remove liveness analysis

theory/Sound_Semantics.thy
@@ -9,8 +9,8 @@ fun value_to_abstract_value :: "val \<Rightarrow> abstract_value" ("|_|" [0]61) 
   "|VClosure p \<rho>| = ^p"
 
 
-inductive maybe_static_eval_value :: "abstract_value_env \<times> abstract_value_env \<Rightarrow> val \<Rightarrow> bool" (infix "\<Turnstile>\<^sub>\<omega>" 55)
-and  maybe_static_eval_env :: "abstract_value_env \<times> abstract_value_env \<Rightarrow> val_env \<Rightarrow> bool" (infix "\<Turnstile>\<^sub>\<rho>" 55) 
+inductive may_be_static_eval_value :: "abstract_value_env \<times> abstract_value_env \<Rightarrow> val \<Rightarrow> bool" (infix "\<Turnstile>\<^sub>\<omega>" 55)
+and  may_be_static_eval_env :: "abstract_value_env \<times> abstract_value_env \<Rightarrow> val_env \<Rightarrow> bool" (infix "\<Turnstile>\<^sub>\<rho>" 55) 
 where
   Unit: "
     (\<V>, \<C>) \<Turnstile>\<^sub>\<omega> VUnit
@@ -69,7 +69,7 @@ where
   "
 
 
-inductive maybe_static_eval_stack :: "abstract_value_env \<times> abstract_value_env \<Rightarrow> abstract_value set \<Rightarrow> cont list \<Rightarrow> bool" ("_ \<Turnstile>\<^sub>\<kappa> _ \<Rrightarrow> _" [56,0,56]55) where
+inductive may_be_static_eval_stack :: "abstract_value_env \<times> abstract_value_env \<Rightarrow> abstract_value set \<Rightarrow> cont list \<Rightarrow> bool" ("_ \<Turnstile>\<^sub>\<kappa> _ \<Rrightarrow> _" [56,0,56]55) where
   Empty: "(\<V>, \<C>) \<Turnstile>\<^sub>\<kappa> \<W> \<Rrightarrow> []" |
   Nonempty: "
     \<lbrakk> 
@@ -82,7 +82,7 @@ inductive maybe_static_eval_stack :: "abstract_value_env \<times> abstract_value
   "
 
 
-inductive maybe_static_eval_state :: "abstract_value_env \<times> abstract_value_env \<Rightarrow> state \<Rightarrow> bool" (infix "\<Turnstile>\<^sub>\<sigma>" 55)  where
+inductive may_be_static_eval_state :: "abstract_value_env \<times> abstract_value_env \<Rightarrow> state \<Rightarrow> bool" (infix "\<Turnstile>\<^sub>\<sigma>" 55)  where
   Any: "
     \<lbrakk>
       (\<V>, \<C>) \<Turnstile>\<^sub>e e;
@@ -92,24 +92,24 @@ inductive maybe_static_eval_state :: "abstract_value_env \<times> abstract_value
     (\<V>, \<C>) \<Turnstile>\<^sub>\<sigma> \<langle>e; \<rho>; \<kappa>\<rangle>
   "
 
-inductive maybe_static_eval_pool :: "abstract_value_env \<times> abstract_value_env \<Rightarrow> trace_pool \<Rightarrow> bool" (infix "\<Turnstile>\<^sub>\<E>" 55) where
+inductive may_be_static_eval_pool :: "abstract_value_env \<times> abstract_value_env \<Rightarrow> trace_pool \<Rightarrow> bool" (infix "\<Turnstile>\<^sub>\<E>" 55) where
   Any: "
     (\<forall> \<pi> \<sigma> . \<E> \<pi> = Some \<sigma> \<longrightarrow> (\<V>, \<C>) \<Turnstile>\<^sub>\<sigma> \<sigma>)
     \<Longrightarrow> 
     (\<V>, \<C>) \<Turnstile>\<^sub>\<E> \<E>
   "
 
-lemma maybe_static_eval_state_to_exp_result: "
+lemma may_be_static_eval_state_to_exp_result: "
   (\<V>, \<C>) \<Turnstile>\<^sub>\<sigma> \<langle>RESULT x;\<rho>;\<langle>x\<^sub>\<kappa>,e\<^sub>\<kappa>,\<rho>\<^sub>\<kappa>\<rangle> # \<kappa>\<rangle> \<Longrightarrow> (\<V>, \<C>) \<Turnstile>\<^sub>e e\<^sub>\<kappa>
 "
 proof -
  assume "(\<V>, \<C>) \<Turnstile>\<^sub>\<sigma> \<langle>RESULT x;\<rho>;\<langle>x\<^sub>\<kappa>,e\<^sub>\<kappa>,\<rho>\<^sub>\<kappa>\<rangle> # \<kappa>\<rangle>" then
- have "(\<V>, \<C>) \<Turnstile>\<^sub>\<kappa> \<V> x \<Rrightarrow> \<langle>x\<^sub>\<kappa>,e\<^sub>\<kappa>,\<rho>\<^sub>\<kappa>\<rangle> # \<kappa>" by (simp add: maybe_static_eval_state.simps) then
- show "(\<V>, \<C>) \<Turnstile>\<^sub>e e\<^sub>\<kappa>" by (rule maybe_static_eval_stack.cases; auto)
+ have "(\<V>, \<C>) \<Turnstile>\<^sub>\<kappa> \<V> x \<Rrightarrow> \<langle>x\<^sub>\<kappa>,e\<^sub>\<kappa>,\<rho>\<^sub>\<kappa>\<rangle> # \<kappa>" by (simp add: may_be_static_eval_state.simps) then
+ show "(\<V>, \<C>) \<Turnstile>\<^sub>e e\<^sub>\<kappa>" by (rule may_be_static_eval_stack.cases; auto)
 qed
 
 
-lemma maybe_static_eval_state_to_exp_let_case_left: "
+lemma may_be_static_eval_state_to_exp_let_case_left: "
   (\<V>, \<C>) \<Turnstile>\<^sub>\<sigma> \<langle>LET x = CASE x\<^sub>s LEFT x\<^sub>l |> e\<^sub>l RIGHT x\<^sub>r |> e\<^sub>r in e; \<rho>; \<kappa>\<rangle> \<Longrightarrow> 
   \<rho> x\<^sub>s = Some (VClosure (Left x\<^sub>l') \<rho>\<^sub>l) \<Longrightarrow> 
   (\<V>, \<C>) \<Turnstile>\<^sub>e e\<^sub>l
@@ -119,8 +119,8 @@ proof -
   assume "(\<V>, \<C>) \<Turnstile>\<^sub>\<sigma> \<langle>LET x = CASE x\<^sub>s LEFT x\<^sub>l |> e\<^sub>l RIGHT x\<^sub>r |> e\<^sub>r in e; \<rho>; \<kappa>\<rangle>" then
   have "(\<V>, \<C>) \<Turnstile>\<^sub>e LET x = CASE x\<^sub>s LEFT x\<^sub>l |> e\<^sub>l RIGHT x\<^sub>r |> e\<^sub>r in e"  
   and "(\<V>, \<C>) \<Turnstile>\<^sub>\<rho> \<rho>"
-  by (simp add: maybe_static_eval_state.simps)+ then
-  have "\<forall>x \<omega>. \<rho> x = Some \<omega> \<longrightarrow> {|\<omega>|} \<subseteq> \<V> x" by (simp add: maybe_static_eval_env.simps)
+  by (simp add: may_be_static_eval_state.simps)+ then
+  have "\<forall>x \<omega>. \<rho> x = Some \<omega> \<longrightarrow> {|\<omega>|} \<subseteq> \<V> x" by (simp add: may_be_static_eval_env.simps)
   with `\<rho> x\<^sub>s = Some (VClosure (Left x\<^sub>l') \<rho>\<^sub>l)`
   have "^prim.Left x\<^sub>l' \<in> \<V> x\<^sub>s" by fastforce
   with `(\<V>, \<C>) \<Turnstile>\<^sub>e LET x = CASE x\<^sub>s LEFT x\<^sub>l |> e\<^sub>l RIGHT x\<^sub>r |> e\<^sub>r in e`
@@ -135,7 +135,7 @@ proof -
 qed
 
 
-lemma maybe_static_eval_state_to_exp_let_case_right: "
+lemma may_be_static_eval_state_to_exp_let_case_right: "
   (\<V>, \<C>) \<Turnstile>\<^sub>\<sigma> \<langle>LET x = CASE x\<^sub>s LEFT x\<^sub>l |> e\<^sub>l RIGHT x\<^sub>r |> e\<^sub>r in e; \<rho>; \<kappa>\<rangle> \<Longrightarrow> 
   \<rho> x\<^sub>s = Some (VClosure (Right x\<^sub>r') \<rho>\<^sub>r) \<Longrightarrow> 
   (\<V>, \<C>) \<Turnstile>\<^sub>e e\<^sub>r
@@ -145,8 +145,8 @@ proof -
   assume "(\<V>, \<C>) \<Turnstile>\<^sub>\<sigma> \<langle>LET x = CASE x\<^sub>s LEFT x\<^sub>l |> e\<^sub>l RIGHT x\<^sub>r |> e\<^sub>r in e; \<rho>; \<kappa>\<rangle>" then
   have "(\<V>, \<C>) \<Turnstile>\<^sub>e LET x = CASE x\<^sub>s LEFT x\<^sub>l |> e\<^sub>l RIGHT x\<^sub>r |> e\<^sub>r in e"  
   and "(\<V>, \<C>) \<Turnstile>\<^sub>\<rho> \<rho>" 
-    by (simp add: maybe_static_eval_state.simps)+ then
-  have "\<forall>x \<omega>. \<rho> x = Some \<omega> \<longrightarrow> {|\<omega>|} \<subseteq> \<V> x" by (simp add: maybe_static_eval_env.simps)
+    by (simp add: may_be_static_eval_state.simps)+ then
+  have "\<forall>x \<omega>. \<rho> x = Some \<omega> \<longrightarrow> {|\<omega>|} \<subseteq> \<V> x" by (simp add: may_be_static_eval_env.simps)
   with `\<rho> x\<^sub>s = Some (VClosure (Right x\<^sub>r') \<rho>\<^sub>r)`
   have "^prim.Right x\<^sub>r' \<in> \<V> x\<^sub>s" by fastforce
   with `(\<V>, \<C>) \<Turnstile>\<^sub>e LET x = CASE x\<^sub>s LEFT x\<^sub>l |> e\<^sub>l RIGHT x\<^sub>r |> e\<^sub>r in e`
@@ -161,17 +161,17 @@ proof -
 qed
 
 
-lemma maybe_static_eval_state_to_exp_let: "
+lemma may_be_static_eval_state_to_exp_let: "
   (\<V>, \<C>) \<Turnstile>\<^sub>\<sigma> \<langle>LET x = b in e; \<rho>; \<kappa>\<rangle> \<Longrightarrow> (\<V>, \<C>) \<Turnstile>\<^sub>e e
 "
 proof -
  assume "(\<V>, \<C>) \<Turnstile>\<^sub>\<sigma> \<langle>LET x = b in e; \<rho>; \<kappa>\<rangle>" then
- have "(\<V>, \<C>) \<Turnstile>\<^sub>e LET x = b in e" by (simp add: maybe_static_eval_state.simps) then
- show "(\<V>, \<C>) \<Turnstile>\<^sub>e e" by (rule maybe_static_eval.cases; auto)
+ have "(\<V>, \<C>) \<Turnstile>\<^sub>e LET x = b in e" by (simp add: may_be_static_eval_state.simps) then
+ show "(\<V>, \<C>) \<Turnstile>\<^sub>e e" by (rule may_be_static_eval.cases; auto)
 qed
 
 
-lemma maybe_static_eval_state_to_exp_let_app: "
+lemma may_be_static_eval_state_to_exp_let_app: "
  (\<V>, \<C>) \<Turnstile>\<^sub>\<sigma> \<langle>LET x = APP f x\<^sub>a in e; \<rho>; \<kappa>\<rangle> \<Longrightarrow> 
  \<rho> f = Some (VClosure (Abs f' x\<^sub>p e\<^sub>b) \<rho>') \<Longrightarrow>
  (\<V>, \<C>) \<Turnstile>\<^sub>e e\<^sub>b
@@ -180,14 +180,14 @@ lemma maybe_static_eval_state_to_exp_let_app: "
 proof -
   assume "\<rho> f = Some (VClosure (Abs f' x\<^sub>p e\<^sub>b) \<rho>')"
   assume "(\<V>, \<C>) \<Turnstile>\<^sub>\<sigma> \<langle>LET x = APP f x\<^sub>a in e; \<rho>; \<kappa>\<rangle>" then
-  have "(\<V>, \<C>) \<Turnstile>\<^sub>\<rho> \<rho>" by (simp add: maybe_static_eval_state.simps) then
-  have "\<forall>x \<omega>. \<rho> x = Some \<omega> \<longrightarrow> {|\<omega>|} \<subseteq> \<V> x \<and> (\<V>, \<C>) \<Turnstile>\<^sub>\<omega> \<omega>" by (simp add: maybe_static_eval_env.simps)
+  have "(\<V>, \<C>) \<Turnstile>\<^sub>\<rho> \<rho>" by (simp add: may_be_static_eval_state.simps) then
+  have "\<forall>x \<omega>. \<rho> x = Some \<omega> \<longrightarrow> {|\<omega>|} \<subseteq> \<V> x \<and> (\<V>, \<C>) \<Turnstile>\<^sub>\<omega> \<omega>" by (simp add: may_be_static_eval_env.simps)
   with `\<rho> f = Some (VClosure (Abs f' x\<^sub>p e\<^sub>b) \<rho>')`
   have "(\<V>, \<C>) \<Turnstile>\<^sub>\<omega> (VClosure (Abs f' x\<^sub>p e\<^sub>b) \<rho>')" by simp then
-  show "(\<V>, \<C>) \<Turnstile>\<^sub>e e\<^sub>b" by (rule maybe_static_eval_value.cases; auto)
+  show "(\<V>, \<C>) \<Turnstile>\<^sub>e e\<^sub>b" by (rule may_be_static_eval_value.cases; auto)
 qed
 
-lemma maybe_static_eval_state_to_env_result: "
+lemma may_be_static_eval_state_to_env_result: "
   (\<V>, \<C>) \<Turnstile>\<^sub>\<sigma> \<langle>RESULT x; \<rho>; \<langle>x\<^sub>\<kappa>,e\<^sub>\<kappa>,\<rho>\<^sub>\<kappa>\<rangle> # \<kappa>\<rangle> \<Longrightarrow> 
   \<rho> x = Some \<omega> \<Longrightarrow> 
   (\<V>, \<C>) \<Turnstile>\<^sub>\<rho> \<rho>\<^sub>\<kappa>(x\<^sub>\<kappa> \<mapsto> \<omega>)
@@ -196,10 +196,10 @@ proof
  assume "\<rho> x = Some \<omega> "
 
  assume "(\<V>, \<C>) \<Turnstile>\<^sub>\<sigma> \<langle>RESULT x; \<rho>; \<langle>x\<^sub>\<kappa>,e\<^sub>\<kappa>,\<rho>\<^sub>\<kappa>\<rangle> # \<kappa>\<rangle>" then
- have "(\<V>, \<C>) \<Turnstile>\<^sub>\<kappa> \<V> x \<Rrightarrow> \<langle>x\<^sub>\<kappa>,e\<^sub>\<kappa>,\<rho>\<^sub>\<kappa>\<rangle> # \<kappa>" and "(\<V>, \<C>) \<Turnstile>\<^sub>\<rho> \<rho>" by (rule maybe_static_eval_state.cases; auto)+
+ have "(\<V>, \<C>) \<Turnstile>\<^sub>\<kappa> \<V> x \<Rrightarrow> \<langle>x\<^sub>\<kappa>,e\<^sub>\<kappa>,\<rho>\<^sub>\<kappa>\<rangle> # \<kappa>" and "(\<V>, \<C>) \<Turnstile>\<^sub>\<rho> \<rho>" by (rule may_be_static_eval_state.cases; auto)+
 
  from `(\<V>, \<C>) \<Turnstile>\<^sub>\<rho> \<rho>` and `\<rho> x = Some \<omega>`
- have "{|\<omega>|} \<subseteq> \<V> x" "(\<V>, \<C>) \<Turnstile>\<^sub>\<omega> \<omega>" by (simp add: maybe_static_eval_env.simps)+
+ have "{|\<omega>|} \<subseteq> \<V> x" "(\<V>, \<C>) \<Turnstile>\<^sub>\<omega> \<omega>" by (simp add: may_be_static_eval_env.simps)+
 
  from `(\<V>, \<C>) \<Turnstile>\<^sub>\<kappa> \<V> x \<Rrightarrow> \<langle>x\<^sub>\<kappa>,e\<^sub>\<kappa>,\<rho>\<^sub>\<kappa>\<rangle> # \<kappa>`
  show "\<forall>x \<omega>'. (\<rho>\<^sub>\<kappa>(x\<^sub>\<kappa> \<mapsto> \<omega>)) x = Some \<omega>' \<longrightarrow> {|\<omega>'|} \<subseteq> \<V> x \<and> (\<V>, \<C>) \<Turnstile>\<^sub>\<omega> \<omega>'"
@@ -226,7 +226,7 @@ proof
        have "\<rho>\<^sub>\<kappa> x' = Some \<omega>'" by simp 
        with `(\<V>, \<C>) \<Turnstile>\<^sub>\<rho> \<rho>\<^sub>\<kappa>`
        
-       show "{|\<omega>'|} \<subseteq> \<V> x' \<and> (\<V>, \<C>) \<Turnstile>\<^sub>\<omega> \<omega>'" by (simp add: maybe_static_eval_env.simps)+
+       show "{|\<omega>'|} \<subseteq> \<V> x' \<and> (\<V>, \<C>) \<Turnstile>\<^sub>\<omega> \<omega>'" by (simp add: may_be_static_eval_env.simps)+
      qed
    } then
 
@@ -235,7 +235,7 @@ proof
 qed
 
 
-lemma maybe_static_eval_state_to_stack_result: "
+lemma may_be_static_eval_state_to_stack_result: "
   (\<V>, \<C>) \<Turnstile>\<^sub>\<sigma> \<langle>RESULT x; \<rho>; \<langle>x\<^sub>\<kappa>,e\<^sub>\<kappa>,\<rho>\<^sub>\<kappa>\<rangle> # \<kappa>\<rangle> \<Longrightarrow> 
   \<rho> x = Some \<omega> \<Longrightarrow> 
   (\<V>, \<C>) \<Turnstile>\<^sub>\<kappa> \<V> (\<lfloor>e\<^sub>\<kappa>\<rfloor>) \<Rrightarrow> \<kappa>
@@ -243,37 +243,37 @@ lemma maybe_static_eval_state_to_stack_result: "
 proof -
   assume "\<rho> x = Some \<omega>"
   assume "(\<V>, \<C>) \<Turnstile>\<^sub>\<sigma> \<langle>RESULT x; \<rho>; \<langle>x\<^sub>\<kappa>,e\<^sub>\<kappa>,\<rho>\<^sub>\<kappa>\<rangle> # \<kappa>\<rangle>" then
-  have "(\<V>, \<C>) \<Turnstile>\<^sub>\<kappa> \<V> x \<Rrightarrow> \<langle>x\<^sub>\<kappa>,e\<^sub>\<kappa>,\<rho>\<^sub>\<kappa>\<rangle> # \<kappa>" by (simp add: maybe_static_eval_state.simps) then
-  show "(\<V>, \<C>) \<Turnstile>\<^sub>\<kappa> \<V> (\<lfloor>e\<^sub>\<kappa>\<rfloor>) \<Rrightarrow> \<kappa>" by (rule maybe_static_eval_stack.cases; auto)
+  have "(\<V>, \<C>) \<Turnstile>\<^sub>\<kappa> \<V> x \<Rrightarrow> \<langle>x\<^sub>\<kappa>,e\<^sub>\<kappa>,\<rho>\<^sub>\<kappa>\<rangle> # \<kappa>" by (simp add: may_be_static_eval_state.simps) then
+  show "(\<V>, \<C>) \<Turnstile>\<^sub>\<kappa> \<V> (\<lfloor>e\<^sub>\<kappa>\<rfloor>) \<Rrightarrow> \<kappa>" by (rule may_be_static_eval_stack.cases; auto)
 qed
 
 
-lemma maybe_static_eval_state_to_state_result: "
+lemma may_be_static_eval_state_to_state_result: "
   (\<V>, \<C>) \<Turnstile>\<^sub>\<sigma> \<langle>RESULT x; \<rho>; \<langle>x\<^sub>\<kappa>,e\<^sub>\<kappa>,\<rho>\<^sub>\<kappa>\<rangle> # \<kappa>\<rangle> \<Longrightarrow> 
   \<rho> x = Some \<omega> \<Longrightarrow> 
   (\<V>, \<C>) \<Turnstile>\<^sub>\<sigma> \<langle>e\<^sub>\<kappa>; \<rho>\<^sub>\<kappa>(x\<^sub>\<kappa> \<mapsto> \<omega>); \<kappa>\<rangle>
 "
 proof
   assume "\<rho> x = Some \<omega>" "(\<V>, \<C>) \<Turnstile>\<^sub>\<sigma> \<langle>RESULT x; \<rho>; \<langle>x\<^sub>\<kappa>,e\<^sub>\<kappa>,\<rho>\<^sub>\<kappa>\<rangle> # \<kappa>\<rangle>" then
-  show "(\<V>, \<C>) \<Turnstile>\<^sub>\<rho> \<rho>\<^sub>\<kappa>(x\<^sub>\<kappa> \<mapsto> \<omega>)" by (blast intro: maybe_static_eval_state_to_env_result)
+  show "(\<V>, \<C>) \<Turnstile>\<^sub>\<rho> \<rho>\<^sub>\<kappa>(x\<^sub>\<kappa> \<mapsto> \<omega>)" by (blast intro: may_be_static_eval_state_to_env_result)
 
   with `(\<V>, \<C>) \<Turnstile>\<^sub>\<sigma> \<langle>RESULT x; \<rho>; \<langle>x\<^sub>\<kappa>,e\<^sub>\<kappa>,\<rho>\<^sub>\<kappa>\<rangle> # \<kappa>\<rangle>`
-  show "(\<V>, \<C>) \<Turnstile>\<^sub>e e\<^sub>\<kappa>" by (blast intro: maybe_static_eval_state_to_exp_result)
+  show "(\<V>, \<C>) \<Turnstile>\<^sub>e e\<^sub>\<kappa>" by (blast intro: may_be_static_eval_state_to_exp_result)
 
   with `\<rho> x = Some \<omega>` `(\<V>, \<C>) \<Turnstile>\<^sub>\<sigma> \<langle>RESULT x; \<rho>; \<langle>x\<^sub>\<kappa>,e\<^sub>\<kappa>,\<rho>\<^sub>\<kappa>\<rangle> # \<kappa>\<rangle>`
-  show "(\<V>, \<C>) \<Turnstile>\<^sub>\<kappa> \<V> (\<lfloor>e\<^sub>\<kappa>\<rfloor>) \<Rrightarrow> \<kappa>" by (blast intro: maybe_static_eval_state_to_stack_result)
+  show "(\<V>, \<C>) \<Turnstile>\<^sub>\<kappa> \<V> (\<lfloor>e\<^sub>\<kappa>\<rfloor>) \<Rrightarrow> \<kappa>" by (blast intro: may_be_static_eval_state_to_stack_result)
 qed
 
 
-lemma maybe_static_eval_state_to_env_let_unit: "
+lemma may_be_static_eval_state_to_env_let_unit: "
   (\<V>, \<C>) \<Turnstile>\<^sub>\<sigma> \<langle>LET x = \<lparr>\<rparr> in e; \<rho>; \<kappa>\<rangle> \<Longrightarrow> (\<V>, \<C>) \<Turnstile>\<^sub>\<rho> \<rho>(x \<mapsto> VUnit)
 "
 proof
   assume "(\<V>, \<C>) \<Turnstile>\<^sub>\<sigma> \<langle>LET x = \<lparr>\<rparr> in e; \<rho>; \<kappa>\<rangle>" then 
-  have "(\<V>, \<C>) \<Turnstile>\<^sub>e LET x = \<lparr>\<rparr> in e" "(\<V>, \<C>) \<Turnstile>\<^sub>\<rho> \<rho>" by (simp add: maybe_static_eval_state.simps)+ 
+  have "(\<V>, \<C>) \<Turnstile>\<^sub>e LET x = \<lparr>\<rparr> in e" "(\<V>, \<C>) \<Turnstile>\<^sub>\<rho> \<rho>" by (simp add: may_be_static_eval_state.simps)+ 
 
   from `(\<V>, \<C>) \<Turnstile>\<^sub>e LET x = \<lparr>\<rparr> in e`
-  have "{^\<lparr>\<rparr>} \<subseteq> \<V> x" by (rule maybe_static_eval.cases; auto)+
+  have "{^\<lparr>\<rparr>} \<subseteq> \<V> x" by (rule may_be_static_eval.cases; auto)+
   have "(\<V>, \<C>) \<Turnstile>\<^sub>\<omega> VUnit" by (simp add: Unit)
 
   {
@@ -293,7 +293,7 @@ proof
 
       from `(\<V>, \<C>) \<Turnstile>\<^sub>\<rho> \<rho>` `\<rho> x' = Some \<omega>'`
 
-      show "{|\<omega>'|} \<subseteq> \<V> x' \<and> (\<V>, \<C>) \<Turnstile>\<^sub>\<omega> \<omega>'" by (simp add: maybe_static_eval_env.simps)
+      show "{|\<omega>'|} \<subseteq> \<V> x' \<and> (\<V>, \<C>) \<Turnstile>\<^sub>\<omega> \<omega>'" by (simp add: may_be_static_eval_env.simps)
     qed
 
   }
@@ -302,41 +302,41 @@ proof
 qed
 
 
-lemma maybe_static_eval_state_to_stack_let: "
+lemma may_be_static_eval_state_to_stack_let: "
   (\<V>, \<C>) \<Turnstile>\<^sub>\<sigma> \<langle>LET x = b in e; \<rho>; \<kappa>\<rangle> \<Longrightarrow> (\<V>, \<C>) \<Turnstile>\<^sub>\<kappa> \<V> (\<lfloor>e\<rfloor>) \<Rrightarrow> \<kappa>
 "
-by (erule maybe_static_eval_state.cases; auto)
+by (erule may_be_static_eval_state.cases; auto)
 
-lemma maybe_static_eval_state_to_state_let_unit: "
+lemma may_be_static_eval_state_to_state_let_unit: "
   (\<V>, \<C>) \<Turnstile>\<^sub>\<sigma> \<langle>LET x = \<lparr>\<rparr> in e; \<rho>; \<kappa>\<rangle> \<Longrightarrow> (\<V>, \<C>) \<Turnstile>\<^sub>\<sigma> \<langle>e; \<rho>(x \<mapsto> VUnit); \<kappa>\<rangle>
 "
 proof
   assume "(\<V>, \<C>) \<Turnstile>\<^sub>\<sigma> \<langle>LET x = \<lparr>\<rparr> in e; \<rho>; \<kappa>\<rangle>" then
-  show "(\<V>, \<C>) \<Turnstile>\<^sub>e e" by (auto simp: maybe_static_eval_state_to_exp_let)
+  show "(\<V>, \<C>) \<Turnstile>\<^sub>e e" by (auto simp: may_be_static_eval_state_to_exp_let)
 
   from `(\<V>, \<C>) \<Turnstile>\<^sub>\<sigma> \<langle>LET x = \<lparr>\<rparr> in e; \<rho>; \<kappa>\<rangle>` 
-  show "(\<V>, \<C>) \<Turnstile>\<^sub>\<rho> \<rho>(x \<mapsto> VUnit)" by (auto simp: maybe_static_eval_state_to_env_let_unit)
+  show "(\<V>, \<C>) \<Turnstile>\<^sub>\<rho> \<rho>(x \<mapsto> VUnit)" by (auto simp: may_be_static_eval_state_to_env_let_unit)
 
   from `(\<V>, \<C>) \<Turnstile>\<^sub>\<sigma> \<langle>LET x = \<lparr>\<rparr> in e; \<rho>; \<kappa>\<rangle>` 
-  show "(\<V>, \<C>) \<Turnstile>\<^sub>\<kappa> \<V> (\<lfloor>e\<rfloor>) \<Rrightarrow> \<kappa>" by (auto simp: maybe_static_eval_state_to_stack_let)
+  show "(\<V>, \<C>) \<Turnstile>\<^sub>\<kappa> \<V> (\<lfloor>e\<rfloor>) \<Rrightarrow> \<kappa>" by (auto simp: may_be_static_eval_state_to_stack_let)
 
 qed
 
-lemma maybe_static_eval_to_value_let_prim: "
+lemma may_be_static_eval_to_value_let_prim: "
   (\<V>, \<C>) \<Turnstile>\<^sub>e LET x = Prim p in e \<Longrightarrow> (\<V>, \<C>) \<Turnstile>\<^sub>\<rho> \<rho> \<Longrightarrow> (\<V>, \<C>) \<Turnstile>\<^sub>\<omega> (VClosure p \<rho>)
 "
-by (erule maybe_static_eval.cases; auto; rule; auto)
+by (erule may_be_static_eval.cases; auto; rule; auto)
 
-lemma maybe_static_eval_state_to_env_let_prim: "
+lemma may_be_static_eval_state_to_env_let_prim: "
   (\<V>, \<C>) \<Turnstile>\<^sub>\<sigma> \<langle>LET x = Prim p in e; \<rho>; \<kappa>\<rangle> \<Longrightarrow> (\<V>, \<C>) \<Turnstile>\<^sub>\<rho> \<rho>(x \<mapsto> (VClosure p \<rho>))
 "
 proof
   assume "(\<V>, \<C>) \<Turnstile>\<^sub>\<sigma> \<langle>LET x = Prim p in e; \<rho>; \<kappa>\<rangle> " then 
-  have "(\<V>, \<C>) \<Turnstile>\<^sub>e LET x = Prim p in e" "(\<V>, \<C>) \<Turnstile>\<^sub>\<rho> \<rho>" by (simp add: maybe_static_eval_state.simps)+ then
-  have "(\<V>, \<C>) \<Turnstile>\<^sub>\<omega> (VClosure p \<rho>)" by (simp add: maybe_static_eval_to_value_let_prim)
+  have "(\<V>, \<C>) \<Turnstile>\<^sub>e LET x = Prim p in e" "(\<V>, \<C>) \<Turnstile>\<^sub>\<rho> \<rho>" by (simp add: may_be_static_eval_state.simps)+ then
+  have "(\<V>, \<C>) \<Turnstile>\<^sub>\<omega> (VClosure p \<rho>)" by (simp add: may_be_static_eval_to_value_let_prim)
 
   from `(\<V>, \<C>) \<Turnstile>\<^sub>e LET x = Prim p in e`
-  have "{^p} \<subseteq> \<V> x" by (rule maybe_static_eval.cases; auto)+
+  have "{^p} \<subseteq> \<V> x" by (rule may_be_static_eval.cases; auto)+
  
   {
     fix x' \<omega>'
@@ -353,7 +353,7 @@ proof
       have "\<rho> x' = Some \<omega>'" by simp
       with `(\<V>, \<C>) \<Turnstile>\<^sub>\<rho> \<rho>` 
   
-      show "{|\<omega>'|} \<subseteq> \<V> x' \<and> (\<V>, \<C>) \<Turnstile>\<^sub>\<omega> \<omega>'" by (simp add: maybe_static_eval_env.simps)
+      show "{|\<omega>'|} \<subseteq> \<V> x' \<and> (\<V>, \<C>) \<Turnstile>\<^sub>\<omega> \<omega>'" by (simp add: may_be_static_eval_env.simps)
     qed
 
   } then
@@ -361,23 +361,23 @@ proof
   show "\<forall>x' \<omega>'. (\<rho>(x \<mapsto> (VClosure p \<rho>))) x' = Some \<omega>' \<longrightarrow> {|\<omega>'|} \<subseteq> \<V> x' \<and> (\<V>, \<C>) \<Turnstile>\<^sub>\<omega> \<omega>'" by auto
 qed
 
-lemma maybe_static_eval_state_to_state_let_prim: "
+lemma may_be_static_eval_state_to_state_let_prim: "
   (\<V>, \<C>) \<Turnstile>\<^sub>\<sigma> \<langle>LET x = Prim p in e; \<rho>; \<kappa>\<rangle> \<Longrightarrow> (\<V>, \<C>) \<Turnstile>\<^sub>\<sigma> \<langle>e; \<rho>(x \<mapsto> (VClosure p \<rho>)); \<kappa>\<rangle>
 "
 proof
   assume "(\<V>, \<C>) \<Turnstile>\<^sub>\<sigma> \<langle>LET x = Prim p in e; \<rho>; \<kappa>\<rangle>" then
-  show "(\<V>, \<C>) \<Turnstile>\<^sub>e e" by (auto simp: maybe_static_eval_state_to_exp_let)
+  show "(\<V>, \<C>) \<Turnstile>\<^sub>e e" by (auto simp: may_be_static_eval_state_to_exp_let)
 
   from `(\<V>, \<C>) \<Turnstile>\<^sub>\<sigma> \<langle>LET x = Prim p in e; \<rho>; \<kappa>\<rangle>` 
-  show "(\<V>, \<C>) \<Turnstile>\<^sub>\<kappa> \<V> (\<lfloor>e\<rfloor>) \<Rrightarrow> \<kappa>" by (auto simp: maybe_static_eval_state_to_stack_let)
+  show "(\<V>, \<C>) \<Turnstile>\<^sub>\<kappa> \<V> (\<lfloor>e\<rfloor>) \<Rrightarrow> \<kappa>" by (auto simp: may_be_static_eval_state_to_stack_let)
 
   from `(\<V>, \<C>) \<Turnstile>\<^sub>\<sigma> \<langle>LET x = Prim p in e; \<rho>; \<kappa>\<rangle>` 
-  show "(\<V>, \<C>) \<Turnstile>\<^sub>\<rho> \<rho>(x \<mapsto> (VClosure p \<rho>))" by (auto simp: maybe_static_eval_state_to_env_let_prim)
+  show "(\<V>, \<C>) \<Turnstile>\<^sub>\<rho> \<rho>(x \<mapsto> (VClosure p \<rho>))" by (auto simp: may_be_static_eval_state_to_env_let_prim)
 
 qed
 
 
-lemma maybe_static_eval_state_to_env_let_case_left: "
+lemma may_be_static_eval_state_to_env_let_case_left: "
   (\<V>, \<C>) \<Turnstile>\<^sub>\<sigma> \<langle>LET x = CASE x\<^sub>s LEFT x\<^sub>l |> e\<^sub>l RIGHT x\<^sub>r |> e\<^sub>r in e; \<rho>; \<kappa>\<rangle> \<Longrightarrow> 
   \<rho> x\<^sub>s = Some (VClosure (Left x\<^sub>l') \<rho>\<^sub>l) \<Longrightarrow> \<rho>\<^sub>l x\<^sub>l' = Some \<omega>\<^sub>l \<Longrightarrow> 
   (\<V>, \<C>) \<Turnstile>\<^sub>\<rho> \<rho>(x\<^sub>l \<mapsto> \<omega>\<^sub>l)
@@ -386,17 +386,17 @@ lemma maybe_static_eval_state_to_env_let_case_left: "
 proof
   assume "\<rho> x\<^sub>s = Some (VClosure (Left x\<^sub>l') \<rho>\<^sub>l)" "\<rho>\<^sub>l x\<^sub>l' = Some \<omega>\<^sub>l"
   assume "(\<V>, \<C>) \<Turnstile>\<^sub>\<sigma> \<langle>LET x = CASE x\<^sub>s LEFT x\<^sub>l |> e\<^sub>l RIGHT x\<^sub>r |> e\<^sub>r in e; \<rho>; \<kappa>\<rangle>" then 
-  have "(\<V>, \<C>) \<Turnstile>\<^sub>e LET x = CASE x\<^sub>s LEFT x\<^sub>l |> e\<^sub>l RIGHT x\<^sub>r |> e\<^sub>r in e" "(\<V>, \<C>) \<Turnstile>\<^sub>\<rho> \<rho>" by (simp add: maybe_static_eval_state.simps)+
+  have "(\<V>, \<C>) \<Turnstile>\<^sub>e LET x = CASE x\<^sub>s LEFT x\<^sub>l |> e\<^sub>l RIGHT x\<^sub>r |> e\<^sub>r in e" "(\<V>, \<C>) \<Turnstile>\<^sub>\<rho> \<rho>" by (simp add: may_be_static_eval_state.simps)+
 
   from `(\<V>, \<C>) \<Turnstile>\<^sub>\<rho> \<rho>` `\<rho> x\<^sub>s = Some (VClosure (Left x\<^sub>l') \<rho>\<^sub>l)`
-  have "(\<V>, \<C>) \<Turnstile>\<^sub>\<omega> (VClosure (Left x\<^sub>l') \<rho>\<^sub>l)" by (blast intro: maybe_static_eval_env.cases) then
-  have "(\<V>, \<C>) \<Turnstile>\<^sub>\<rho> \<rho>\<^sub>l" by (blast intro: maybe_static_eval_value.cases)
+  have "(\<V>, \<C>) \<Turnstile>\<^sub>\<omega> (VClosure (Left x\<^sub>l') \<rho>\<^sub>l)" by (blast intro: may_be_static_eval_env.cases) then
+  have "(\<V>, \<C>) \<Turnstile>\<^sub>\<rho> \<rho>\<^sub>l" by (blast intro: may_be_static_eval_value.cases)
 
   from `(\<V>, \<C>) \<Turnstile>\<^sub>\<rho> \<rho>\<^sub>l` `\<rho>\<^sub>l x\<^sub>l' = Some \<omega>\<^sub>l`
-  have "{|\<omega>\<^sub>l|} \<subseteq> \<V> x\<^sub>l'" "(\<V>, \<C>) \<Turnstile>\<^sub>\<omega> \<omega>\<^sub>l" by (blast intro: maybe_static_eval_env.cases)+
+  have "{|\<omega>\<^sub>l|} \<subseteq> \<V> x\<^sub>l'" "(\<V>, \<C>) \<Turnstile>\<^sub>\<omega> \<omega>\<^sub>l" by (blast intro: may_be_static_eval_env.cases)+
 
   from `(\<V>, \<C>) \<Turnstile>\<^sub>\<rho> \<rho>` `\<rho> x\<^sub>s = Some (VClosure (Left x\<^sub>l') \<rho>\<^sub>l)`
-  have " | (VClosure (Left x\<^sub>l') \<rho>\<^sub>l) | \<in> \<V> x\<^sub>s" by (blast intro: maybe_static_eval_env.cases) then
+  have " | (VClosure (Left x\<^sub>l') \<rho>\<^sub>l) | \<in> \<V> x\<^sub>s" by (blast intro: may_be_static_eval_env.cases) then
   have "^prim.Left x\<^sub>l' \<in> \<V> x\<^sub>s" by simp
 
   from  `(\<V>, \<C>) \<Turnstile>\<^sub>e LET x = CASE x\<^sub>s LEFT x\<^sub>l |> e\<^sub>l RIGHT x\<^sub>r |> e\<^sub>r in e`
@@ -416,7 +416,7 @@ proof
     assume "(\<rho>(x\<^sub>l \<mapsto> \<omega>\<^sub>l)) x' = Some \<omega>'" "x' \<noteq> x\<^sub>l" then
     have "\<rho> x' = Some \<omega>'" by simp
     with `(\<V>, \<C>) \<Turnstile>\<^sub>\<rho> \<rho>` 
-    have "{|\<omega>'|} \<subseteq> \<V> x' \<and> (\<V>, \<C>) \<Turnstile>\<^sub>\<omega> \<omega>'" by (simp add: maybe_static_eval_env.simps)
+    have "{|\<omega>'|} \<subseteq> \<V> x' \<and> (\<V>, \<C>) \<Turnstile>\<^sub>\<omega> \<omega>'" by (simp add: may_be_static_eval_env.simps)
    
   }
   with `{|\<omega>\<^sub>l|} \<subseteq> \<V> x\<^sub>l` `(\<V>, \<C>) \<Turnstile>\<^sub>\<omega> \<omega>\<^sub>l`
@@ -424,7 +424,7 @@ proof
 qed
 
 
-lemma maybe_static_eval_state_to_stack_let_case_left: "
+lemma may_be_static_eval_state_to_stack_let_case_left: "
   (\<V>, \<C>) \<Turnstile>\<^sub>\<sigma> \<langle>LET x = CASE x\<^sub>s LEFT x\<^sub>l |> e\<^sub>l RIGHT x\<^sub>r |> e\<^sub>r in e; \<rho>; \<kappa>\<rangle> \<Longrightarrow>
   \<rho> x\<^sub>s = Some (VClosure (Left x\<^sub>l') \<rho>\<^sub>l) \<Longrightarrow> \<rho>\<^sub>l x\<^sub>l' = Some \<omega>\<^sub>l \<Longrightarrow> 
   (\<V>, \<C>) \<Turnstile>\<^sub>\<kappa> \<V> (\<lfloor>e\<^sub>l\<rfloor>) \<Rrightarrow> \<langle>x,e,\<rho>\<rangle> # \<kappa>
@@ -435,10 +435,10 @@ proof
   assume "\<rho> x\<^sub>s = Some (VClosure (Left x\<^sub>l') \<rho>\<^sub>l)" "\<rho>\<^sub>l x\<^sub>l' = Some \<omega>\<^sub>l"
 
   from `(\<V>, \<C>) \<Turnstile>\<^sub>\<sigma> \<langle>LET x = CASE x\<^sub>s LEFT x\<^sub>l |> e\<^sub>l RIGHT x\<^sub>r |> e\<^sub>r in e;\<rho>;\<kappa>\<rangle>`
-  have "(\<V>, \<C>) \<Turnstile>\<^sub>e LET x = CASE x\<^sub>s LEFT x\<^sub>l |> e\<^sub>l RIGHT x\<^sub>r |> e\<^sub>r in e" "(\<V>, \<C>) \<Turnstile>\<^sub>\<rho> \<rho>" by (blast intro: maybe_static_eval_state.cases)+
+  have "(\<V>, \<C>) \<Turnstile>\<^sub>e LET x = CASE x\<^sub>s LEFT x\<^sub>l |> e\<^sub>l RIGHT x\<^sub>r |> e\<^sub>r in e" "(\<V>, \<C>) \<Turnstile>\<^sub>\<rho> \<rho>" by (blast intro: may_be_static_eval_state.cases)+
   
   from `(\<V>, \<C>) \<Turnstile>\<^sub>\<rho> \<rho>` `\<rho> x\<^sub>s = Some (VClosure (Left x\<^sub>l') \<rho>\<^sub>l)`
-  have " | (VClosure (Left x\<^sub>l') \<rho>\<^sub>l) | \<in> \<V> x\<^sub>s" by (blast intro: maybe_static_eval_env.cases) then
+  have " | (VClosure (Left x\<^sub>l') \<rho>\<^sub>l) | \<in> \<V> x\<^sub>s" by (blast intro: may_be_static_eval_env.cases) then
   have "^prim.Left x\<^sub>l' \<in> \<V> x\<^sub>s" by simp
 
   from `(\<V>, \<C>) \<Turnstile>\<^sub>e LET x = CASE x\<^sub>s LEFT x\<^sub>l |> e\<^sub>l RIGHT x\<^sub>r |> e\<^sub>r in e`
@@ -451,18 +451,18 @@ proof
   qed
 
   from `(\<V>, \<C>) \<Turnstile>\<^sub>\<sigma> \<langle>LET x = CASE x\<^sub>s LEFT x\<^sub>l |> e\<^sub>l RIGHT x\<^sub>r |> e\<^sub>r in e;\<rho>;\<kappa>\<rangle>`
-  show "(\<V>, \<C>) \<Turnstile>\<^sub>e e" by (blast intro: maybe_static_eval_state_to_exp_let)
+  show "(\<V>, \<C>) \<Turnstile>\<^sub>e e" by (blast intro: may_be_static_eval_state_to_exp_let)
 
   from `(\<V>, \<C>) \<Turnstile>\<^sub>\<sigma> \<langle>LET x = CASE x\<^sub>s LEFT x\<^sub>l |> e\<^sub>l RIGHT x\<^sub>r |> e\<^sub>r in e;\<rho>;\<kappa>\<rangle>`
-  show "(\<V>, \<C>) \<Turnstile>\<^sub>\<rho> \<rho>" by (blast intro: maybe_static_eval_state.cases)
+  show "(\<V>, \<C>) \<Turnstile>\<^sub>\<rho> \<rho>" by (blast intro: may_be_static_eval_state.cases)
 
   from `(\<V>, \<C>) \<Turnstile>\<^sub>\<sigma> \<langle>LET x = CASE x\<^sub>s LEFT x\<^sub>l |> e\<^sub>l RIGHT x\<^sub>r |> e\<^sub>r in e;\<rho>;\<kappa>\<rangle>`
-  show "(\<V>, \<C>) \<Turnstile>\<^sub>\<kappa> \<V> (\<lfloor>e\<rfloor>) \<Rrightarrow> \<kappa>" by (blast intro: maybe_static_eval_state_to_stack_let)
+  show "(\<V>, \<C>) \<Turnstile>\<^sub>\<kappa> \<V> (\<lfloor>e\<rfloor>) \<Rrightarrow> \<kappa>" by (blast intro: may_be_static_eval_state_to_stack_let)
   
 qed
 
 
-lemma maybe_static_eval_state_to_state_let_case_left: "
+lemma may_be_static_eval_state_to_state_let_case_left: "
   (\<V>, \<C>) \<Turnstile>\<^sub>\<sigma> \<langle>LET x = CASE x\<^sub>s LEFT x\<^sub>l |> e\<^sub>l RIGHT x\<^sub>r |> e\<^sub>r in e; \<rho>; \<kappa>\<rangle> \<Longrightarrow> 
   \<rho> x\<^sub>s = Some (VClosure (Left x\<^sub>l') \<rho>\<^sub>l) \<Longrightarrow> 
   \<rho>\<^sub>l x\<^sub>l' = Some \<omega>\<^sub>l \<Longrightarrow> 
@@ -470,20 +470,20 @@ lemma maybe_static_eval_state_to_state_let_case_left: "
 "
 proof
   assume "(\<V>, \<C>) \<Turnstile>\<^sub>\<sigma> \<langle>LET x = CASE x\<^sub>s LEFT x\<^sub>l |> e\<^sub>l RIGHT x\<^sub>r |> e\<^sub>r in e; \<rho>; \<kappa>\<rangle>" and "\<rho> x\<^sub>s = Some (VClosure (Left x\<^sub>l') \<rho>\<^sub>l)" then
-  show "(\<V>, \<C>) \<Turnstile>\<^sub>e e\<^sub>l" by (simp add: maybe_static_eval_state_to_exp_let_case_left)
+  show "(\<V>, \<C>) \<Turnstile>\<^sub>e e\<^sub>l" by (simp add: may_be_static_eval_state_to_exp_let_case_left)
 
   assume "\<rho>\<^sub>l x\<^sub>l' = Some \<omega>\<^sub>l"
   with `(\<V>, \<C>) \<Turnstile>\<^sub>\<sigma> \<langle>LET x = CASE x\<^sub>s LEFT x\<^sub>l |> e\<^sub>l RIGHT x\<^sub>r |> e\<^sub>r in e; \<rho>; \<kappa>\<rangle>` and `\<rho> x\<^sub>s = Some (VClosure (Left x\<^sub>l') \<rho>\<^sub>l)` 
-  show "(\<V>, \<C>) \<Turnstile>\<^sub>\<rho> \<rho>(x\<^sub>l \<mapsto> \<omega>\<^sub>l)" by (simp add: maybe_static_eval_state_to_env_let_case_left)
+  show "(\<V>, \<C>) \<Turnstile>\<^sub>\<rho> \<rho>(x\<^sub>l \<mapsto> \<omega>\<^sub>l)" by (simp add: may_be_static_eval_state_to_env_let_case_left)
 
   from `\<rho>\<^sub>l x\<^sub>l' = Some \<omega>\<^sub>l`  
   and `(\<V>, \<C>) \<Turnstile>\<^sub>\<sigma> \<langle>LET x = CASE x\<^sub>s LEFT x\<^sub>l |> e\<^sub>l RIGHT x\<^sub>r |> e\<^sub>r in e; \<rho>; \<kappa>\<rangle>` 
   and `\<rho> x\<^sub>s = Some (VClosure (Left x\<^sub>l') \<rho>\<^sub>l)` 
-  show "(\<V>, \<C>) \<Turnstile>\<^sub>\<kappa> \<V> (\<lfloor>e\<^sub>l\<rfloor>) \<Rrightarrow> \<langle>x,e,\<rho>\<rangle> # \<kappa>" by (simp add: maybe_static_eval_state_to_stack_let_case_left)
+  show "(\<V>, \<C>) \<Turnstile>\<^sub>\<kappa> \<V> (\<lfloor>e\<^sub>l\<rfloor>) \<Rrightarrow> \<langle>x,e,\<rho>\<rangle> # \<kappa>" by (simp add: may_be_static_eval_state_to_stack_let_case_left)
 qed
 
 
-lemma maybe_static_eval_state_to_env_let_case_right: "
+lemma may_be_static_eval_state_to_env_let_case_right: "
   (\<V>, \<C>) \<Turnstile>\<^sub>\<sigma> \<langle>LET x = CASE x\<^sub>s LEFT x\<^sub>l |> e\<^sub>l RIGHT x\<^sub>r |> e\<^sub>r in e; \<rho>; \<kappa>\<rangle> \<Longrightarrow> 
   \<rho> x\<^sub>s = Some (VClosure (Right x\<^sub>r') \<rho>\<^sub>r) \<Longrightarrow> \<rho>\<^sub>r x\<^sub>r' = Some \<omega>\<^sub>r \<Longrightarrow> 
   (\<V>, \<C>) \<Turnstile>\<^sub>\<rho> \<rho>(x\<^sub>r \<mapsto> \<omega>\<^sub>r)
@@ -492,17 +492,17 @@ lemma maybe_static_eval_state_to_env_let_case_right: "
 proof
   assume "\<rho> x\<^sub>s = Some (VClosure (Right x\<^sub>r') \<rho>\<^sub>r)" "\<rho>\<^sub>r x\<^sub>r' = Some \<omega>\<^sub>r"
   assume "(\<V>, \<C>) \<Turnstile>\<^sub>\<sigma> \<langle>LET x = CASE x\<^sub>s LEFT x\<^sub>l |> e\<^sub>l RIGHT x\<^sub>r |> e\<^sub>r in e; \<rho>; \<kappa>\<rangle>" then 
-  have "(\<V>, \<C>) \<Turnstile>\<^sub>e LET x = CASE x\<^sub>s LEFT x\<^sub>l |> e\<^sub>l RIGHT x\<^sub>r |> e\<^sub>r in e" "(\<V>, \<C>) \<Turnstile>\<^sub>\<rho> \<rho>" by (simp add: maybe_static_eval_state.simps)+
+  have "(\<V>, \<C>) \<Turnstile>\<^sub>e LET x = CASE x\<^sub>s LEFT x\<^sub>l |> e\<^sub>l RIGHT x\<^sub>r |> e\<^sub>r in e" "(\<V>, \<C>) \<Turnstile>\<^sub>\<rho> \<rho>" by (simp add: may_be_static_eval_state.simps)+
 
   from `(\<V>, \<C>) \<Turnstile>\<^sub>\<rho> \<rho>` `\<rho> x\<^sub>s = Some (VClosure (Right x\<^sub>r') \<rho>\<^sub>r)`
-  have "(\<V>, \<C>) \<Turnstile>\<^sub>\<omega> (VClosure (Right x\<^sub>r') \<rho>\<^sub>r)" by (blast intro: maybe_static_eval_env.cases) then
-  have "(\<V>, \<C>) \<Turnstile>\<^sub>\<rho> \<rho>\<^sub>r" by (blast intro: maybe_static_eval_value.cases)
+  have "(\<V>, \<C>) \<Turnstile>\<^sub>\<omega> (VClosure (Right x\<^sub>r') \<rho>\<^sub>r)" by (blast intro: may_be_static_eval_env.cases) then
+  have "(\<V>, \<C>) \<Turnstile>\<^sub>\<rho> \<rho>\<^sub>r" by (blast intro: may_be_static_eval_value.cases)
 
   from `(\<V>, \<C>) \<Turnstile>\<^sub>\<rho> \<rho>\<^sub>r` `\<rho>\<^sub>r x\<^sub>r' = Some \<omega>\<^sub>r`
-  have "{|\<omega>\<^sub>r|} \<subseteq> \<V> x\<^sub>r'" "(\<V>, \<C>) \<Turnstile>\<^sub>\<omega> \<omega>\<^sub>r" by (blast intro: maybe_static_eval_env.cases)+
+  have "{|\<omega>\<^sub>r|} \<subseteq> \<V> x\<^sub>r'" "(\<V>, \<C>) \<Turnstile>\<^sub>\<omega> \<omega>\<^sub>r" by (blast intro: may_be_static_eval_env.cases)+
 
   from `(\<V>, \<C>) \<Turnstile>\<^sub>\<rho> \<rho>` `\<rho> x\<^sub>s = Some (VClosure (Right x\<^sub>r') \<rho>\<^sub>r)`
-  have " | (VClosure (Right x\<^sub>r') \<rho>\<^sub>r) | \<in> \<V> x\<^sub>s" by (blast intro: maybe_static_eval_env.cases) then
+  have " | (VClosure (Right x\<^sub>r') \<rho>\<^sub>r) | \<in> \<V> x\<^sub>s" by (blast intro: may_be_static_eval_env.cases) then
   have "^prim.Right x\<^sub>r' \<in> \<V> x\<^sub>s" by simp
 
   from  `(\<V>, \<C>) \<Turnstile>\<^sub>e LET x = CASE x\<^sub>s LEFT x\<^sub>l |> e\<^sub>l RIGHT x\<^sub>r |> e\<^sub>r in e`
@@ -522,14 +522,14 @@ proof
     assume "(\<rho>(x\<^sub>r \<mapsto> \<omega>\<^sub>r)) x' = Some \<omega>'" "x' \<noteq> x\<^sub>r" then
     have "\<rho> x' = Some \<omega>'" by simp
     with `(\<V>, \<C>) \<Turnstile>\<^sub>\<rho> \<rho>` 
-    have "{|\<omega>'|} \<subseteq> \<V> x' \<and> (\<V>, \<C>) \<Turnstile>\<^sub>\<omega> \<omega>'" by (simp add: maybe_static_eval_env.simps)
+    have "{|\<omega>'|} \<subseteq> \<V> x' \<and> (\<V>, \<C>) \<Turnstile>\<^sub>\<omega> \<omega>'" by (simp add: may_be_static_eval_env.simps)
    
   }
   with `{|\<omega>\<^sub>r|} \<subseteq> \<V> x\<^sub>r` `(\<V>, \<C>) \<Turnstile>\<^sub>\<omega> \<omega>\<^sub>r`
   show "\<forall>x' \<omega>'. (\<rho>(x\<^sub>r \<mapsto> \<omega>\<^sub>r)) x' = Some \<omega>' \<longrightarrow> {|\<omega>'|} \<subseteq> \<V> x' \<and> (\<V>, \<C>) \<Turnstile>\<^sub>\<omega> \<omega>'" by auto
 qed
 
-lemma maybe_static_eval_state_to_stack_let_case_right: "
+lemma may_be_static_eval_state_to_stack_let_case_right: "
   (\<V>, \<C>) \<Turnstile>\<^sub>\<sigma>  \<langle>LET x = CASE x\<^sub>s LEFT x\<^sub>l |> e\<^sub>l RIGHT x\<^sub>r |> e\<^sub>r in e; \<rho>; \<kappa>\<rangle> \<Longrightarrow>
   \<rho> x\<^sub>s = Some (VClosure (Right x\<^sub>r') \<rho>\<^sub>r) \<Longrightarrow> \<rho>\<^sub>r x\<^sub>r' = Some \<omega>\<^sub>r \<Longrightarrow> 
   (\<V>, \<C>) \<Turnstile>\<^sub>\<kappa>  \<V> (\<lfloor>e\<^sub>r\<rfloor>) \<Rrightarrow> \<langle>x,e,\<rho>\<rangle> # \<kappa>
@@ -540,10 +540,10 @@ proof
   assume "\<rho> x\<^sub>s = Some (VClosure (Right x\<^sub>r') \<rho>\<^sub>r)" "\<rho>\<^sub>r x\<^sub>r' = Some \<omega>\<^sub>r"
 
   from `(\<V>, \<C>) \<Turnstile>\<^sub>\<sigma> \<langle>LET x = CASE x\<^sub>s LEFT x\<^sub>l |> e\<^sub>l RIGHT x\<^sub>r |> e\<^sub>r in e;\<rho>;\<kappa>\<rangle>`
-  have "(\<V>, \<C>) \<Turnstile>\<^sub>e LET x = CASE x\<^sub>s LEFT x\<^sub>l |> e\<^sub>l RIGHT x\<^sub>r |> e\<^sub>r in e" "(\<V>, \<C>) \<Turnstile>\<^sub>\<rho> \<rho>" by (blast intro: maybe_static_eval_state.cases)+
+  have "(\<V>, \<C>) \<Turnstile>\<^sub>e LET x = CASE x\<^sub>s LEFT x\<^sub>l |> e\<^sub>l RIGHT x\<^sub>r |> e\<^sub>r in e" "(\<V>, \<C>) \<Turnstile>\<^sub>\<rho> \<rho>" by (blast intro: may_be_static_eval_state.cases)+
   
   from `(\<V>, \<C>) \<Turnstile>\<^sub>\<rho> \<rho>` `\<rho> x\<^sub>s = Some (VClosure (Right x\<^sub>r') \<rho>\<^sub>r)`
-  have " | (VClosure (Right x\<^sub>r') \<rho>\<^sub>r) | \<in> \<V> x\<^sub>s" by (blast intro: maybe_static_eval_env.cases) then
+  have " | (VClosure (Right x\<^sub>r') \<rho>\<^sub>r) | \<in> \<V> x\<^sub>s" by (blast intro: may_be_static_eval_env.cases) then
   have "^prim.Right x\<^sub>r' \<in> \<V> x\<^sub>s" by simp
 
   from `(\<V>, \<C>) \<Turnstile>\<^sub>e LET x = CASE x\<^sub>s LEFT x\<^sub>l |> e\<^sub>l RIGHT x\<^sub>r |> e\<^sub>r in e`
@@ -556,37 +556,37 @@ proof
   qed
 
   from `(\<V>, \<C>) \<Turnstile>\<^sub>\<sigma> \<langle>LET x = CASE x\<^sub>s LEFT x\<^sub>l |> e\<^sub>l RIGHT x\<^sub>r |> e\<^sub>r in e;\<rho>;\<kappa>\<rangle>`
-  show "(\<V>, \<C>) \<Turnstile>\<^sub>e e" by (blast intro: maybe_static_eval_state_to_exp_let)
+  show "(\<V>, \<C>) \<Turnstile>\<^sub>e e" by (blast intro: may_be_static_eval_state_to_exp_let)
 
   from `(\<V>, \<C>) \<Turnstile>\<^sub>\<sigma> \<langle>LET x = CASE x\<^sub>s LEFT x\<^sub>l |> e\<^sub>l RIGHT x\<^sub>r |> e\<^sub>r in e;\<rho>;\<kappa>\<rangle>`
-  show "(\<V>, \<C>) \<Turnstile>\<^sub>\<rho> \<rho>" by (blast intro: maybe_static_eval_state.cases)
+  show "(\<V>, \<C>) \<Turnstile>\<^sub>\<rho> \<rho>" by (blast intro: may_be_static_eval_state.cases)
 
   from `(\<V>, \<C>) \<Turnstile>\<^sub>\<sigma> \<langle>LET x = CASE x\<^sub>s LEFT x\<^sub>l |> e\<^sub>l RIGHT x\<^sub>r |> e\<^sub>r in e;\<rho>;\<kappa>\<rangle>`
-  show "(\<V>, \<C>) \<Turnstile>\<^sub>\<kappa> \<V> (\<lfloor>e\<rfloor>) \<Rrightarrow> \<kappa>" by (blast intro: maybe_static_eval_state_to_stack_let)
+  show "(\<V>, \<C>) \<Turnstile>\<^sub>\<kappa> \<V> (\<lfloor>e\<rfloor>) \<Rrightarrow> \<kappa>" by (blast intro: may_be_static_eval_state_to_stack_let)
   
 qed
 
-lemma maybe_static_eval_state_to_state_let_case_right: "
+lemma may_be_static_eval_state_to_state_let_case_right: "
   (\<V>, \<C>) \<Turnstile>\<^sub>\<sigma> \<langle>LET x = CASE x\<^sub>s LEFT x\<^sub>l |> e\<^sub>l RIGHT x\<^sub>r |> e\<^sub>r in e; \<rho>; \<kappa>\<rangle> \<Longrightarrow> 
   \<rho> x\<^sub>s = Some (VClosure (Right x\<^sub>r') \<rho>\<^sub>r) \<Longrightarrow> 
   \<rho>\<^sub>r x\<^sub>r' = Some \<omega>\<^sub>r \<Longrightarrow> (\<V>, \<C>) \<Turnstile>\<^sub>\<sigma> \<langle>e\<^sub>r; \<rho>(x\<^sub>r \<mapsto> \<omega>\<^sub>r); \<langle>x,e,\<rho>\<rangle> # \<kappa>\<rangle>
 "
 proof
   assume "(\<V>, \<C>) \<Turnstile>\<^sub>\<sigma> \<langle>LET x = CASE x\<^sub>s LEFT x\<^sub>l |> e\<^sub>l RIGHT x\<^sub>r |> e\<^sub>r in e; \<rho>; \<kappa>\<rangle>" and "\<rho> x\<^sub>s = Some (VClosure (Right x\<^sub>r') \<rho>\<^sub>r)" then
-  show "(\<V>, \<C>) \<Turnstile>\<^sub>e e\<^sub>r" by (simp add: maybe_static_eval_state_to_exp_let_case_right)
+  show "(\<V>, \<C>) \<Turnstile>\<^sub>e e\<^sub>r" by (simp add: may_be_static_eval_state_to_exp_let_case_right)
 
   assume "\<rho>\<^sub>r x\<^sub>r' = Some \<omega>\<^sub>r"
   with `(\<V>, \<C>) \<Turnstile>\<^sub>\<sigma> \<langle>LET x = CASE x\<^sub>s LEFT x\<^sub>l |> e\<^sub>l RIGHT x\<^sub>r |> e\<^sub>r in e; \<rho>; \<kappa>\<rangle>` and `\<rho> x\<^sub>s = Some (VClosure (Right x\<^sub>r') \<rho>\<^sub>r)` 
-  show "(\<V>, \<C>) \<Turnstile>\<^sub>\<rho> \<rho>(x\<^sub>r \<mapsto> \<omega>\<^sub>r)" by (simp add: maybe_static_eval_state_to_env_let_case_right)
+  show "(\<V>, \<C>) \<Turnstile>\<^sub>\<rho> \<rho>(x\<^sub>r \<mapsto> \<omega>\<^sub>r)" by (simp add: may_be_static_eval_state_to_env_let_case_right)
 
   from `\<rho>\<^sub>r x\<^sub>r' = Some \<omega>\<^sub>r`  
   and `(\<V>, \<C>) \<Turnstile>\<^sub>\<sigma> \<langle>LET x = CASE x\<^sub>s LEFT x\<^sub>l |> e\<^sub>l RIGHT x\<^sub>r |> e\<^sub>r in e; \<rho>; \<kappa>\<rangle>` 
   and `\<rho> x\<^sub>s = Some (VClosure (Right x\<^sub>r') \<rho>\<^sub>r)` 
-  show "(\<V>, \<C>) \<Turnstile>\<^sub>\<kappa> \<V> (\<lfloor>e\<^sub>r\<rfloor>) \<Rrightarrow> \<langle>x,e,\<rho>\<rangle> # \<kappa>" by (simp add: maybe_static_eval_state_to_stack_let_case_right)
+  show "(\<V>, \<C>) \<Turnstile>\<^sub>\<kappa> \<V> (\<lfloor>e\<^sub>r\<rfloor>) \<Rrightarrow> \<langle>x,e,\<rho>\<rangle> # \<kappa>" by (simp add: may_be_static_eval_state_to_stack_let_case_right)
 qed
 
 
-lemma maybe_static_eval_state_to_env_let_fst: "
+lemma may_be_static_eval_state_to_env_let_fst: "
   (\<V>, \<C>) \<Turnstile>\<^sub>\<sigma> \<langle>LET x = FST x\<^sub>p in e; \<rho>; \<kappa>\<rangle> \<Longrightarrow> 
   \<rho> x\<^sub>p = Some (VClosure (Pair x\<^sub>1 x\<^sub>2) \<rho>\<^sub>p) \<Longrightarrow> \<rho>\<^sub>p x\<^sub>1 = Some \<omega> \<Longrightarrow> 
   (\<V>, \<C>) \<Turnstile>\<^sub>\<rho> \<rho>(x \<mapsto> \<omega>)
@@ -594,19 +594,19 @@ lemma maybe_static_eval_state_to_env_let_fst: "
 proof
   assume "\<rho> x\<^sub>p = Some (VClosure (Pair x\<^sub>1 x\<^sub>2) \<rho>\<^sub>p)" and "\<rho>\<^sub>p x\<^sub>1 = Some \<omega>"
   assume "(\<V>, \<C>) \<Turnstile>\<^sub>\<sigma> \<langle>LET x = FST x\<^sub>p in e; \<rho>; \<kappa>\<rangle>" then
-  have "(\<V>, \<C>) \<Turnstile>\<^sub>e LET x = FST x\<^sub>p in e" "(\<V>, \<C>) \<Turnstile>\<^sub>\<rho> \<rho>" by (simp add: maybe_static_eval_state.simps)+
+  have "(\<V>, \<C>) \<Turnstile>\<^sub>e LET x = FST x\<^sub>p in e" "(\<V>, \<C>) \<Turnstile>\<^sub>\<rho> \<rho>" by (simp add: may_be_static_eval_state.simps)+
 
-  thm maybe_static_eval_state.simps
+  thm may_be_static_eval_state.simps
 
   from `(\<V>, \<C>) \<Turnstile>\<^sub>\<rho> \<rho>` `\<rho> x\<^sub>p = Some (VClosure (Pair x\<^sub>1 x\<^sub>2) \<rho>\<^sub>p)`
-  have "(\<V>, \<C>) \<Turnstile>\<^sub>\<omega> (VClosure (Pair x\<^sub>1 x\<^sub>2) \<rho>\<^sub>p)" by (blast intro: maybe_static_eval_env.cases) then
-  have "(\<V>, \<C>) \<Turnstile>\<^sub>\<rho> \<rho>\<^sub>p" by (blast intro: maybe_static_eval_value.cases)
+  have "(\<V>, \<C>) \<Turnstile>\<^sub>\<omega> (VClosure (Pair x\<^sub>1 x\<^sub>2) \<rho>\<^sub>p)" by (blast intro: may_be_static_eval_env.cases) then
+  have "(\<V>, \<C>) \<Turnstile>\<^sub>\<rho> \<rho>\<^sub>p" by (blast intro: may_be_static_eval_value.cases)
 
   from `(\<V>, \<C>) \<Turnstile>\<^sub>\<rho> \<rho>\<^sub>p` `\<rho>\<^sub>p x\<^sub>1 = Some \<omega>`
-  have "{|\<omega>|} \<subseteq> \<V> x\<^sub>1" "(\<V>, \<C>) \<Turnstile>\<^sub>\<omega> \<omega>" by (blast intro: maybe_static_eval_env.cases)+
+  have "{|\<omega>|} \<subseteq> \<V> x\<^sub>1" "(\<V>, \<C>) \<Turnstile>\<^sub>\<omega> \<omega>" by (blast intro: may_be_static_eval_env.cases)+
 
   from `(\<V>, \<C>) \<Turnstile>\<^sub>\<rho> \<rho>` `\<rho> x\<^sub>p = Some (VClosure (Pair x\<^sub>1 x\<^sub>2) \<rho>\<^sub>p)`
-  have " | (VClosure (Pair x\<^sub>1 x\<^sub>2) \<rho>\<^sub>p) | \<in> \<V> x\<^sub>p" by (blast intro: maybe_static_eval_env.cases) then
+  have " | (VClosure (Pair x\<^sub>1 x\<^sub>2) \<rho>\<^sub>p) | \<in> \<V> x\<^sub>p" by (blast intro: may_be_static_eval_env.cases) then
   have "^prim.Pair x\<^sub>1 x\<^sub>2 \<in> \<V> x\<^sub>p" by simp
 
   from  `(\<V>, \<C>) \<Turnstile>\<^sub>e LET x = FST x\<^sub>p in e`
@@ -626,7 +626,7 @@ proof
     assume "(\<rho>(x \<mapsto> \<omega>)) x' = Some \<omega>'" "x' \<noteq> x" then
     have "\<rho> x' = Some \<omega>'" by simp
     with `(\<V>, \<C>) \<Turnstile>\<^sub>\<rho> \<rho>` 
-    have "{|\<omega>'|} \<subseteq> \<V> x' \<and> (\<V>, \<C>) \<Turnstile>\<^sub>\<omega> \<omega>'" by (simp add: maybe_static_eval_env.simps)
+    have "{|\<omega>'|} \<subseteq> \<V> x' \<and> (\<V>, \<C>) \<Turnstile>\<^sub>\<omega> \<omega>'" by (simp add: may_be_static_eval_env.simps)
   }
   with `{|\<omega>|} \<subseteq> \<V> x` `(\<V>, \<C>) \<Turnstile>\<^sub>\<omega> \<omega>`
   show "\<forall>x' \<omega>'. (\<rho>(x \<mapsto> \<omega>)) x' = Some \<omega>' \<longrightarrow> {|\<omega>'|} \<subseteq> \<V> x' \<and> (\<V>, \<C>) \<Turnstile>\<^sub>\<omega> \<omega>'" by auto
@@ -634,42 +634,42 @@ qed
 
 
 
-lemma maybe_static_eval_state_to_state_let_fst: "
+lemma may_be_static_eval_state_to_state_let_fst: "
   (\<V>, \<C>) \<Turnstile>\<^sub>\<sigma> \<langle>LET x = FST x\<^sub>p in e; \<rho>; \<kappa>\<rangle> \<Longrightarrow>
   \<rho> x\<^sub>p = Some (VClosure (Pair x\<^sub>1 x\<^sub>2) \<rho>\<^sub>p) \<Longrightarrow> \<rho>\<^sub>p x\<^sub>1 = Some \<omega> \<Longrightarrow> 
   (\<V>, \<C>) \<Turnstile>\<^sub>\<sigma> \<langle>e; \<rho>(x \<mapsto> \<omega>); \<kappa>\<rangle>
 "
 proof
   assume "(\<V>, \<C>) \<Turnstile>\<^sub>\<sigma> \<langle>LET x = FST x\<^sub>p in e; \<rho>; \<kappa>\<rangle>" then
-  show "(\<V>, \<C>) \<Turnstile>\<^sub>e e" by (simp add: maybe_static_eval_state_to_exp_let)
+  show "(\<V>, \<C>) \<Turnstile>\<^sub>e e" by (simp add: may_be_static_eval_state_to_exp_let)
 
   assume "\<rho> x\<^sub>p = Some (VClosure (Pair x\<^sub>1 x\<^sub>2) \<rho>\<^sub>p)" and "\<rho>\<^sub>p x\<^sub>1 = Some \<omega>"
   with `(\<V>, \<C>) \<Turnstile>\<^sub>\<sigma> \<langle>LET x = FST x\<^sub>p in e; \<rho>; \<kappa>\<rangle>`
-  show "(\<V>, \<C>) \<Turnstile>\<^sub>\<rho> \<rho>(x \<mapsto> \<omega>)"  by (simp add: maybe_static_eval_state_to_env_let_fst)
+  show "(\<V>, \<C>) \<Turnstile>\<^sub>\<rho> \<rho>(x \<mapsto> \<omega>)"  by (simp add: may_be_static_eval_state_to_env_let_fst)
 
   from `\<rho> x\<^sub>p = Some (VClosure (Pair x\<^sub>1 x\<^sub>2) \<rho>\<^sub>p)` and `\<rho>\<^sub>p x\<^sub>1 = Some \<omega>`
   and `(\<V>, \<C>) \<Turnstile>\<^sub>\<sigma> \<langle>LET x = FST x\<^sub>p in e; \<rho>; \<kappa>\<rangle>`
-  show "(\<V>, \<C>) \<Turnstile>\<^sub>\<kappa> \<V> (\<lfloor>e\<rfloor>) \<Rrightarrow> \<kappa>" by (simp add: maybe_static_eval_state_to_stack_let)
+  show "(\<V>, \<C>) \<Turnstile>\<^sub>\<kappa> \<V> (\<lfloor>e\<rfloor>) \<Rrightarrow> \<kappa>" by (simp add: may_be_static_eval_state_to_stack_let)
 qed
 
 
-lemma maybe_static_eval_state_to_env_let_snd: "
+lemma may_be_static_eval_state_to_env_let_snd: "
   (\<V>, \<C>) \<Turnstile>\<^sub>\<sigma> \<langle>LET x = SND x\<^sub>p in e; \<rho>; \<kappa>\<rangle> \<Longrightarrow> \<rho> x\<^sub>p = Some (VClosure (Pair x\<^sub>1 x\<^sub>2) \<rho>\<^sub>p) \<Longrightarrow> \<rho>\<^sub>p x\<^sub>2 = Some \<omega> \<Longrightarrow> (\<V>, \<C>) \<Turnstile>\<^sub>\<rho> \<rho>(x \<mapsto> \<omega>)
 "
 proof
   assume "\<rho> x\<^sub>p = Some (VClosure (Pair x\<^sub>1 x\<^sub>2) \<rho>\<^sub>p)" and "\<rho>\<^sub>p x\<^sub>2 = Some \<omega>"
   assume "(\<V>, \<C>) \<Turnstile>\<^sub>\<sigma> \<langle>LET x = SND x\<^sub>p in e; \<rho>; \<kappa>\<rangle>" then
-  have "(\<V>, \<C>) \<Turnstile>\<^sub>e LET x = SND x\<^sub>p in e" "(\<V>, \<C>) \<Turnstile>\<^sub>\<rho> \<rho>" by (simp add: maybe_static_eval_state.simps)+
+  have "(\<V>, \<C>) \<Turnstile>\<^sub>e LET x = SND x\<^sub>p in e" "(\<V>, \<C>) \<Turnstile>\<^sub>\<rho> \<rho>" by (simp add: may_be_static_eval_state.simps)+
 
   from `(\<V>, \<C>) \<Turnstile>\<^sub>\<rho> \<rho>` `\<rho> x\<^sub>p = Some (VClosure (Pair x\<^sub>1 x\<^sub>2) \<rho>\<^sub>p)`
-  have "(\<V>, \<C>) \<Turnstile>\<^sub>\<omega> (VClosure (Pair x\<^sub>1 x\<^sub>2) \<rho>\<^sub>p)" by (blast intro: maybe_static_eval_env.cases) then
-  have "(\<V>, \<C>) \<Turnstile>\<^sub>\<rho> \<rho>\<^sub>p" by (blast intro: maybe_static_eval_value.cases)
+  have "(\<V>, \<C>) \<Turnstile>\<^sub>\<omega> (VClosure (Pair x\<^sub>1 x\<^sub>2) \<rho>\<^sub>p)" by (blast intro: may_be_static_eval_env.cases) then
+  have "(\<V>, \<C>) \<Turnstile>\<^sub>\<rho> \<rho>\<^sub>p" by (blast intro: may_be_static_eval_value.cases)
 
   from `(\<V>, \<C>) \<Turnstile>\<^sub>\<rho> \<rho>\<^sub>p` `\<rho>\<^sub>p x\<^sub>2 = Some \<omega>`
-  have "{|\<omega>|} \<subseteq> \<V> x\<^sub>2" "(\<V>, \<C>) \<Turnstile>\<^sub>\<omega> \<omega>" by (blast intro: maybe_static_eval_env.cases)+
+  have "{|\<omega>|} \<subseteq> \<V> x\<^sub>2" "(\<V>, \<C>) \<Turnstile>\<^sub>\<omega> \<omega>" by (blast intro: may_be_static_eval_env.cases)+
 
   from `(\<V>, \<C>) \<Turnstile>\<^sub>\<rho> \<rho>` `\<rho> x\<^sub>p = Some (VClosure (Pair x\<^sub>1 x\<^sub>2) \<rho>\<^sub>p)`
-  have " | (VClosure (Pair x\<^sub>1 x\<^sub>2) \<rho>\<^sub>p) | \<in> \<V> x\<^sub>p" by (blast intro: maybe_static_eval_env.cases) then
+  have " | (VClosure (Pair x\<^sub>1 x\<^sub>2) \<rho>\<^sub>p) | \<in> \<V> x\<^sub>p" by (blast intro: may_be_static_eval_env.cases) then
   have "^prim.Pair x\<^sub>1 x\<^sub>2 \<in> \<V> x\<^sub>p" by simp
 
   from  `(\<V>, \<C>) \<Turnstile>\<^sub>e LET x = SND x\<^sub>p in e`
@@ -690,33 +690,33 @@ proof
     assume "(\<rho>(x \<mapsto> \<omega>)) x' = Some \<omega>'" "x' \<noteq> x" then
     have "\<rho> x' = Some \<omega>'" by simp
     with `(\<V>, \<C>) \<Turnstile>\<^sub>\<rho> \<rho>` 
-    have "{|\<omega>'|} \<subseteq> \<V> x' \<and> (\<V>, \<C>) \<Turnstile>\<^sub>\<omega> \<omega>'" by (simp add: maybe_static_eval_env.simps)
+    have "{|\<omega>'|} \<subseteq> \<V> x' \<and> (\<V>, \<C>) \<Turnstile>\<^sub>\<omega> \<omega>'" by (simp add: may_be_static_eval_env.simps)
   }
   with \<open>{|\<omega>|} \<subseteq> \<V> x\<close> \<open>(\<V>, \<C>) \<Turnstile>\<^sub>\<omega> \<omega>\<close> 
   show "\<forall>x' \<omega>'. (\<rho>(x \<mapsto> \<omega>)) x' = Some \<omega>' \<longrightarrow> {|\<omega>'|} \<subseteq> \<V> x' \<and> (\<V>, \<C>) \<Turnstile>\<^sub>\<omega> \<omega>'" by simp
 qed
 
 
-lemma maybe_static_eval_state_to_state_let_snd: "
+lemma may_be_static_eval_state_to_state_let_snd: "
   (\<V>, \<C>) \<Turnstile>\<^sub>\<sigma> \<langle>LET x = SND x\<^sub>p in e; \<rho>; \<kappa>\<rangle> \<Longrightarrow>
   \<rho> x\<^sub>p = Some (VClosure (Pair x\<^sub>1 x\<^sub>2) \<rho>\<^sub>p) \<Longrightarrow> \<rho>\<^sub>p x\<^sub>2 = Some \<omega> \<Longrightarrow> 
   (\<V>, \<C>) \<Turnstile>\<^sub>\<sigma> \<langle>e; \<rho>(x \<mapsto> \<omega>); \<kappa>\<rangle>
 "
 proof
   assume "(\<V>, \<C>) \<Turnstile>\<^sub>\<sigma> \<langle>LET x = SND x\<^sub>p in e; \<rho>; \<kappa>\<rangle>" then
-  show "(\<V>, \<C>) \<Turnstile>\<^sub>e e" by (simp add: maybe_static_eval_state_to_exp_let)
+  show "(\<V>, \<C>) \<Turnstile>\<^sub>e e" by (simp add: may_be_static_eval_state_to_exp_let)
 
   assume "\<rho> x\<^sub>p = Some (VClosure (Pair x\<^sub>1 x\<^sub>2) \<rho>\<^sub>p)" and "\<rho>\<^sub>p x\<^sub>2 = Some \<omega>"
   with `(\<V>, \<C>) \<Turnstile>\<^sub>\<sigma> \<langle>LET x = SND x\<^sub>p in e; \<rho>; \<kappa>\<rangle>`
-  show "(\<V>, \<C>) \<Turnstile>\<^sub>\<rho> \<rho>(x \<mapsto> \<omega>)" by (simp add: maybe_static_eval_state_to_env_let_snd)
+  show "(\<V>, \<C>) \<Turnstile>\<^sub>\<rho> \<rho>(x \<mapsto> \<omega>)" by (simp add: may_be_static_eval_state_to_env_let_snd)
 
   from `\<rho> x\<^sub>p = Some (VClosure (Pair x\<^sub>1 x\<^sub>2) \<rho>\<^sub>p)` and `\<rho>\<^sub>p x\<^sub>2 = Some \<omega>`
   and `(\<V>, \<C>) \<Turnstile>\<^sub>\<sigma> \<langle>LET x = SND x\<^sub>p in e; \<rho>; \<kappa>\<rangle>`
-  show "(\<V>, \<C>) \<Turnstile>\<^sub>\<kappa> \<V> (\<lfloor>e\<rfloor>) \<Rrightarrow> \<kappa>" by (simp add: maybe_static_eval_state_to_stack_let)
+  show "(\<V>, \<C>) \<Turnstile>\<^sub>\<kappa> \<V> (\<lfloor>e\<rfloor>) \<Rrightarrow> \<kappa>" by (simp add: may_be_static_eval_state_to_stack_let)
 qed
 
 
-lemma maybe_static_eval_state_to_env_let_app: "
+lemma may_be_static_eval_state_to_env_let_app: "
   (\<V>, \<C>) \<Turnstile>\<^sub>\<sigma> \<langle>LET x = APP f x\<^sub>a in e; \<rho>; \<kappa>\<rangle> \<Longrightarrow> 
   \<rho> f = Some (VClosure (Abs f\<^sub>l x\<^sub>l e\<^sub>l) \<rho>\<^sub>l) \<Longrightarrow> \<rho> x\<^sub>a = Some \<omega>\<^sub>a \<Longrightarrow> 
   (\<V>, \<C>) \<Turnstile>\<^sub>\<rho> \<rho>\<^sub>l(f\<^sub>l \<mapsto> (VClosure (Abs f\<^sub>l x\<^sub>l e\<^sub>l) \<rho>\<^sub>l), x\<^sub>l \<mapsto> \<omega>\<^sub>a)
@@ -724,19 +724,19 @@ lemma maybe_static_eval_state_to_env_let_app: "
 proof
   assume "\<rho> f = Some (VClosure (Abs f\<^sub>l x\<^sub>l e\<^sub>l) \<rho>\<^sub>l)" "\<rho> x\<^sub>a = Some \<omega>\<^sub>a"
   assume "(\<V>, \<C>) \<Turnstile>\<^sub>\<sigma> \<langle>LET x = APP f x\<^sub>a in e; \<rho>; \<kappa>\<rangle>" then
-  have "(\<V>, \<C>) \<Turnstile>\<^sub>e LET x = APP f x\<^sub>a in e" "(\<V>, \<C>) \<Turnstile>\<^sub>\<rho> \<rho>" by (simp add: maybe_static_eval_state.simps)+
+  have "(\<V>, \<C>) \<Turnstile>\<^sub>e LET x = APP f x\<^sub>a in e" "(\<V>, \<C>) \<Turnstile>\<^sub>\<rho> \<rho>" by (simp add: may_be_static_eval_state.simps)+
 
   from `(\<V>, \<C>) \<Turnstile>\<^sub>\<rho> \<rho>` and `\<rho> x\<^sub>a = Some \<omega>\<^sub>a`
-  have "{|\<omega>\<^sub>a|} \<subseteq> \<V> x\<^sub>a" "(\<V>, \<C>) \<Turnstile>\<^sub>\<omega> \<omega>\<^sub>a" by (blast intro: maybe_static_eval_env.cases)+
+  have "{|\<omega>\<^sub>a|} \<subseteq> \<V> x\<^sub>a" "(\<V>, \<C>) \<Turnstile>\<^sub>\<omega> \<omega>\<^sub>a" by (blast intro: may_be_static_eval_env.cases)+
 
   from `(\<V>, \<C>) \<Turnstile>\<^sub>\<rho> \<rho>` and `\<rho> f = Some (VClosure (Abs f\<^sub>l x\<^sub>l e\<^sub>l) \<rho>\<^sub>l)`
-  have "{|(VClosure (Abs f\<^sub>l x\<^sub>l e\<^sub>l) \<rho>\<^sub>l)|} \<subseteq> \<V> f" "(\<V>, \<C>) \<Turnstile>\<^sub>\<omega> (VClosure (Abs f\<^sub>l x\<^sub>l e\<^sub>l) \<rho>\<^sub>l)" by (blast intro: maybe_static_eval_env.cases)+
+  have "{|(VClosure (Abs f\<^sub>l x\<^sub>l e\<^sub>l) \<rho>\<^sub>l)|} \<subseteq> \<V> f" "(\<V>, \<C>) \<Turnstile>\<^sub>\<omega> (VClosure (Abs f\<^sub>l x\<^sub>l e\<^sub>l) \<rho>\<^sub>l)" by (blast intro: may_be_static_eval_env.cases)+
 
   from `{|(VClosure (Abs f\<^sub>l x\<^sub>l e\<^sub>l) \<rho>\<^sub>l)|} \<subseteq> \<V> f`
   have "^Abs f\<^sub>l x\<^sub>l e\<^sub>l \<in> \<V> f" by simp
 
   from `(\<V>, \<C>) \<Turnstile>\<^sub>\<omega> (VClosure (Abs f\<^sub>l x\<^sub>l e\<^sub>l) \<rho>\<^sub>l)`
-  have "{|(VClosure (Abs f\<^sub>l x\<^sub>l e\<^sub>l) \<rho>\<^sub>l)|} \<subseteq> \<V> f\<^sub>l" "(\<V>, \<C>) \<Turnstile>\<^sub>\<rho> \<rho>\<^sub>l" by (rule maybe_static_eval_value.cases; auto)+
+  have "{|(VClosure (Abs f\<^sub>l x\<^sub>l e\<^sub>l) \<rho>\<^sub>l)|} \<subseteq> \<V> f\<^sub>l" "(\<V>, \<C>) \<Turnstile>\<^sub>\<rho> \<rho>\<^sub>l" by (rule may_be_static_eval_value.cases; auto)+
 
 
   with `(\<V>, \<C>) \<Turnstile>\<^sub>e LET x = APP f x\<^sub>a in e`
@@ -757,14 +757,14 @@ proof
     assume "(\<rho>\<^sub>l(f\<^sub>l \<mapsto> (VClosure (Abs f\<^sub>l x\<^sub>l e\<^sub>l) \<rho>\<^sub>l), x\<^sub>l \<mapsto> \<omega>\<^sub>a)) x' = Some \<omega>'" "x' \<noteq> x\<^sub>l" "x' \<noteq> f\<^sub>l" then
     have "\<rho>\<^sub>l x' = Some \<omega>'" by simp
     with `(\<V>, \<C>) \<Turnstile>\<^sub>\<rho> \<rho>\<^sub>l` 
-    have "{|\<omega>'|} \<subseteq> \<V> x' \<and> (\<V>, \<C>) \<Turnstile>\<^sub>\<omega> \<omega>'" by (simp add: maybe_static_eval_env.simps)
+    have "{|\<omega>'|} \<subseteq> \<V> x' \<and> (\<V>, \<C>) \<Turnstile>\<^sub>\<omega> \<omega>'" by (simp add: may_be_static_eval_env.simps)
   }
   with \<open>{|(VClosure (Abs f\<^sub>l x\<^sub>l e\<^sub>l) \<rho>\<^sub>l)|} \<subseteq> \<V> f\<^sub>l\<close> \<open>(\<V>, \<C>) \<Turnstile>\<^sub>\<omega> (VClosure (Abs f\<^sub>l x\<^sub>l e\<^sub>l) \<rho>\<^sub>l)\<close> \<open>(\<V>, \<C>) \<Turnstile>\<^sub>\<omega> \<omega>\<^sub>a\<close> \<open>{|\<omega>\<^sub>a|} \<subseteq> \<V> x\<^sub>l\<close>
   show "\<forall>x \<omega>. (\<rho>\<^sub>l(f\<^sub>l \<mapsto> (VClosure (Abs f\<^sub>l x\<^sub>l e\<^sub>l) \<rho>\<^sub>l), x\<^sub>l \<mapsto> \<omega>\<^sub>a)) x = Some \<omega> \<longrightarrow> {|\<omega>|} \<subseteq> \<V> x \<and> (\<V>, \<C>) \<Turnstile>\<^sub>\<omega> \<omega>" by auto
 
 qed
 
-lemma maybe_static_eval_state_to_stack_let_app: "
+lemma may_be_static_eval_state_to_stack_let_app: "
   (\<V>, \<C>) \<Turnstile>\<^sub>\<sigma> \<langle>LET x = APP f x\<^sub>a in e; \<rho>; \<kappa>\<rangle> \<Longrightarrow> 
   \<rho> f = Some (VClosure (Abs f' x\<^sub>p e\<^sub>b) \<rho>') \<Longrightarrow> \<rho> x\<^sub>a = Some \<omega>\<^sub>a \<Longrightarrow> 
   (\<V>, \<C>) \<Turnstile>\<^sub>\<kappa> \<V> (\<lfloor>e\<^sub>b\<rfloor>) \<Rrightarrow> \<langle>x,e,\<rho>\<rangle> # \<kappa>
@@ -772,10 +772,10 @@ lemma maybe_static_eval_state_to_stack_let_app: "
 proof
   assume "\<rho> f = Some (VClosure (Abs f' x\<^sub>p e\<^sub>b) \<rho>')" and "\<rho> x\<^sub>a = Some \<omega>\<^sub>a"
   assume "(\<V>, \<C>) \<Turnstile>\<^sub>\<sigma> \<langle>LET x = APP f x\<^sub>a in e; \<rho>; \<kappa>\<rangle>" then
-  have "(\<V>, \<C>) \<Turnstile>\<^sub>e LET x = APP f x\<^sub>a in e"  "(\<V>, \<C>) \<Turnstile>\<^sub>\<rho> \<rho>" by (blast intro: maybe_static_eval_state.cases)+
+  have "(\<V>, \<C>) \<Turnstile>\<^sub>e LET x = APP f x\<^sub>a in e"  "(\<V>, \<C>) \<Turnstile>\<^sub>\<rho> \<rho>" by (blast intro: may_be_static_eval_state.cases)+
 
   from `(\<V>, \<C>) \<Turnstile>\<^sub>\<rho> \<rho>` and `\<rho> f = Some (VClosure (Abs f' x\<^sub>p e\<^sub>b) \<rho>')`
-  have " {|(VClosure (Abs f' x\<^sub>p e\<^sub>b) \<rho>')|} \<subseteq> \<V> f" by (blast intro: maybe_static_eval_env.cases) then
+  have " {|(VClosure (Abs f' x\<^sub>p e\<^sub>b) \<rho>')|} \<subseteq> \<V> f" by (blast intro: may_be_static_eval_env.cases) then
   have " ^Abs f' x\<^sub>p e\<^sub>b \<in> \<V> f" by simp
 
   from `(\<V>, \<C>) \<Turnstile>\<^sub>e LET x = APP f x\<^sub>a in e`
@@ -788,34 +788,34 @@ proof
   qed
 
   from `(\<V>, \<C>) \<Turnstile>\<^sub>\<sigma> \<langle>LET x = APP f x\<^sub>a in e; \<rho>; \<kappa>\<rangle>`
-  show "(\<V>, \<C>) \<Turnstile>\<^sub>e e" by (blast intro: maybe_static_eval_state_to_exp_let)
+  show "(\<V>, \<C>) \<Turnstile>\<^sub>e e" by (blast intro: may_be_static_eval_state_to_exp_let)
 
   from `(\<V>, \<C>) \<Turnstile>\<^sub>\<sigma> \<langle>LET x = APP f x\<^sub>a in e; \<rho>; \<kappa>\<rangle>`
-  show "(\<V>, \<C>) \<Turnstile>\<^sub>\<rho> \<rho>" by (blast intro: maybe_static_eval_state.cases)
+  show "(\<V>, \<C>) \<Turnstile>\<^sub>\<rho> \<rho>" by (blast intro: may_be_static_eval_state.cases)
 
   from `(\<V>, \<C>) \<Turnstile>\<^sub>\<sigma> \<langle>LET x = APP f x\<^sub>a in e; \<rho>; \<kappa>\<rangle>`
-  show "(\<V>, \<C>) \<Turnstile>\<^sub>\<kappa> \<V> (\<lfloor>e\<rfloor>) \<Rrightarrow> \<kappa>" by (blast intro: maybe_static_eval_state_to_stack_let)
+  show "(\<V>, \<C>) \<Turnstile>\<^sub>\<kappa> \<V> (\<lfloor>e\<rfloor>) \<Rrightarrow> \<kappa>" by (blast intro: may_be_static_eval_state_to_stack_let)
 qed
 
 
-lemma maybe_static_eval_state_to_state_let_app: "
+lemma may_be_static_eval_state_to_state_let_app: "
   (\<V>, \<C>) \<Turnstile>\<^sub>\<sigma> \<langle>LET x = APP f x\<^sub>a in e; \<rho>; \<kappa>\<rangle> \<Longrightarrow>
   \<rho> f = Some (VClosure (Abs f' x\<^sub>p e\<^sub>b) \<rho>') \<Longrightarrow> \<rho> x\<^sub>a = Some \<omega>\<^sub>a \<Longrightarrow> 
   (\<V>, \<C>) \<Turnstile>\<^sub>\<sigma> \<langle>e\<^sub>b; \<rho>'(f' \<mapsto> (VClosure (Abs f' x\<^sub>p e\<^sub>b) \<rho>'), x\<^sub>p \<mapsto> \<omega>\<^sub>a); \<langle>x,e,\<rho>\<rangle> # \<kappa>\<rangle>
 "
 proof
   assume "(\<V>, \<C>) \<Turnstile>\<^sub>\<sigma> \<langle>LET x = APP f x\<^sub>a in e; \<rho>; \<kappa>\<rangle>" and "\<rho> f = Some (VClosure (Abs f' x\<^sub>p e\<^sub>b) \<rho>')" then
-  show "(\<V>, \<C>) \<Turnstile>\<^sub>e e\<^sub>b" by (blast intro: maybe_static_eval_state_to_exp_let_app)
+  show "(\<V>, \<C>) \<Turnstile>\<^sub>e e\<^sub>b" by (blast intro: may_be_static_eval_state_to_exp_let_app)
 
   assume "\<rho> x\<^sub>a = Some \<omega>\<^sub>a"
   with `(\<V>, \<C>) \<Turnstile>\<^sub>\<sigma> \<langle>LET x = APP f x\<^sub>a in e; \<rho>; \<kappa>\<rangle>` and `\<rho> f = Some (VClosure (Abs f' x\<^sub>p e\<^sub>b) \<rho>')`
-  show "(\<V>, \<C>) \<Turnstile>\<^sub>\<rho> \<rho>'(f' \<mapsto> (VClosure (Abs f' x\<^sub>p e\<^sub>b) \<rho>'), x\<^sub>p \<mapsto> \<omega>\<^sub>a)" by (blast intro: maybe_static_eval_state_to_env_let_app)
+  show "(\<V>, \<C>) \<Turnstile>\<^sub>\<rho> \<rho>'(f' \<mapsto> (VClosure (Abs f' x\<^sub>p e\<^sub>b) \<rho>'), x\<^sub>p \<mapsto> \<omega>\<^sub>a)" by (blast intro: may_be_static_eval_state_to_env_let_app)
 
   from `\<rho> x\<^sub>a = Some \<omega>\<^sub>a` and  `(\<V>, \<C>) \<Turnstile>\<^sub>\<sigma> \<langle>LET x = APP f x\<^sub>a in e; \<rho>; \<kappa>\<rangle>` and `\<rho> f = Some (VClosure (Abs f' x\<^sub>p e\<^sub>b) \<rho>')`
-  show "(\<V>, \<C>) \<Turnstile>\<^sub>\<kappa> \<V> (\<lfloor>e\<^sub>b\<rfloor>) \<Rrightarrow> \<langle>x,e,\<rho>\<rangle> # \<kappa>" by (blast intro: maybe_static_eval_state_to_stack_let_app)
+  show "(\<V>, \<C>) \<Turnstile>\<^sub>\<kappa> \<V> (\<lfloor>e\<^sub>b\<rfloor>) \<Rrightarrow> \<langle>x,e,\<rho>\<rangle> # \<kappa>" by (blast intro: may_be_static_eval_state_to_stack_let_app)
 qed
 
-theorem maybe_static_eval_state_preserved_under_step : "
+theorem may_be_static_eval_state_preserved_under_step : "
   \<lbrakk>
     (\<V>, \<C>) \<Turnstile>\<^sub>\<sigma> \<sigma>; 
     \<sigma> \<hookrightarrow> \<sigma>'
@@ -830,38 +830,38 @@ proof -
     case (Result \<rho> x \<omega> x\<^sub>\<kappa> e\<^sub>\<kappa> \<rho>\<^sub>\<kappa> \<kappa>)
     assume "\<sigma> = \<langle>RESULT x;\<rho>;\<langle>x\<^sub>\<kappa>,e\<^sub>\<kappa>,\<rho>\<^sub>\<kappa>\<rangle> # \<kappa>\<rangle>" and "\<sigma>' = \<langle>e\<^sub>\<kappa>;\<rho>\<^sub>\<kappa> ++ [x\<^sub>\<kappa> \<mapsto> \<omega>];\<kappa>\<rangle>" and "\<rho> x = Some \<omega>" 
     with `(\<V>, \<C>) \<Turnstile>\<^sub>\<sigma> \<sigma>`
-    show "(\<V>, \<C>) \<Turnstile>\<^sub>\<sigma> \<sigma>'" by (simp add: maybe_static_eval_state_to_state_result)
+    show "(\<V>, \<C>) \<Turnstile>\<^sub>\<sigma> \<sigma>'" by (simp add: may_be_static_eval_state_to_state_result)
   next
     case (Let_Unit x e \<rho> \<kappa>)
     assume "\<sigma> = \<langle>LET x = \<lparr>\<rparr> in e;\<rho>;\<kappa>\<rangle>" and "\<sigma>' = \<langle>e;\<rho> ++ [x \<mapsto> VUnit];\<kappa>\<rangle>"
     with `(\<V>, \<C>) \<Turnstile>\<^sub>\<sigma> \<sigma>`
-    show "(\<V>, \<C>) \<Turnstile>\<^sub>\<sigma> \<sigma>'" by (simp add: maybe_static_eval_state_to_state_let_unit)
+    show "(\<V>, \<C>) \<Turnstile>\<^sub>\<sigma> \<sigma>'" by (simp add: may_be_static_eval_state_to_state_let_unit)
   next
     case (Let_Prim x p e \<rho> \<kappa>)
     assume "\<sigma> = \<langle>LET x = Prim p in e;\<rho>;\<kappa>\<rangle>" and "\<sigma>' = \<langle>e;\<rho> ++ [x \<mapsto> (VClosure p \<rho>)];\<kappa>\<rangle>"
     with `(\<V>, \<C>) \<Turnstile>\<^sub>\<sigma> \<sigma>`
-    show "(\<V>, \<C>) \<Turnstile>\<^sub>\<sigma> \<sigma>'" by (simp add: maybe_static_eval_state_to_state_let_prim)
+    show "(\<V>, \<C>) \<Turnstile>\<^sub>\<sigma> \<sigma>'" by (simp add: may_be_static_eval_state_to_state_let_prim)
   next
     case (Let_Fst \<rho> x\<^sub>p x\<^sub>1 x\<^sub>2 \<rho>\<^sub>p \<omega> x e \<kappa>)
     assume "\<sigma> = \<langle>LET x = FST x\<^sub>p in e;\<rho>;\<kappa>\<rangle>"
     and "\<sigma>' = \<langle>e;\<rho> ++ [x \<mapsto> \<omega>];\<kappa>\<rangle>"
     and "\<rho> x\<^sub>p = Some (VClosure (Pair x\<^sub>1 x\<^sub>2) \<rho>\<^sub>p)" and "\<rho>\<^sub>p x\<^sub>1 = Some \<omega>"
     with `(\<V>, \<C>) \<Turnstile>\<^sub>\<sigma> \<sigma>`
-    show "(\<V>, \<C>) \<Turnstile>\<^sub>\<sigma> \<sigma>'" by (simp add: maybe_static_eval_state_to_state_let_fst)
+    show "(\<V>, \<C>) \<Turnstile>\<^sub>\<sigma> \<sigma>'" by (simp add: may_be_static_eval_state_to_state_let_fst)
   next
     case (Let_Snd \<rho> x\<^sub>p x\<^sub>1 x\<^sub>2 \<rho>\<^sub>p \<omega> x e \<kappa>)
     assume "\<sigma> = \<langle>LET x = SND x\<^sub>p in e;\<rho>;\<kappa>\<rangle>"
     and "\<sigma>' = \<langle>e;\<rho> ++ [x \<mapsto> \<omega>];\<kappa>\<rangle>"
     and "\<rho> x\<^sub>p = Some (VClosure (Pair x\<^sub>1 x\<^sub>2) \<rho>\<^sub>p)" and "\<rho>\<^sub>p x\<^sub>2 = Some \<omega>"
     with `(\<V>, \<C>) \<Turnstile>\<^sub>\<sigma> \<sigma>`
-    show "(\<V>, \<C>) \<Turnstile>\<^sub>\<sigma> \<sigma>'" by (simp add: maybe_static_eval_state_to_state_let_snd)
+    show "(\<V>, \<C>) \<Turnstile>\<^sub>\<sigma> \<sigma>'" by (simp add: may_be_static_eval_state_to_state_let_snd)
   next
     case (Let_Case_Left \<rho> x\<^sub>s x\<^sub>l' \<rho>\<^sub>l \<omega>\<^sub>l x x\<^sub>l e\<^sub>l x\<^sub>r e\<^sub>r e \<kappa>)
     assume "\<sigma> = \<langle>LET x = CASE x\<^sub>s LEFT x\<^sub>l |> e\<^sub>l RIGHT x\<^sub>r |> e\<^sub>r in e;\<rho>;\<kappa>\<rangle>"
     and "\<sigma>' = \<langle>e\<^sub>l;\<rho> ++ [x\<^sub>l \<mapsto> \<omega>\<^sub>l];\<langle>x,e,\<rho>\<rangle> # \<kappa>\<rangle>"
     and "\<rho> x\<^sub>s = Some (VClosure (Left x\<^sub>l') \<rho>\<^sub>l)" and "\<rho>\<^sub>l x\<^sub>l' = Some \<omega>\<^sub>l"
     with `(\<V>, \<C>) \<Turnstile>\<^sub>\<sigma> \<sigma>`
-    show "(\<V>, \<C>) \<Turnstile>\<^sub>\<sigma> \<sigma>'" by (simp add: maybe_static_eval_state_to_state_let_case_left)
+    show "(\<V>, \<C>) \<Turnstile>\<^sub>\<sigma> \<sigma>'" by (simp add: may_be_static_eval_state_to_state_let_case_left)
   next
     case (Let_Case_Right \<rho> x\<^sub>s x\<^sub>r' \<rho>\<^sub>r \<omega>\<^sub>r x x\<^sub>l e\<^sub>l x\<^sub>r e\<^sub>r e \<kappa>)
     assume "\<sigma> = \<langle>LET x = CASE x\<^sub>s LEFT x\<^sub>l |> e\<^sub>l RIGHT x\<^sub>r |> e\<^sub>r in e;\<rho>;\<kappa>\<rangle>"
@@ -869,7 +869,7 @@ proof -
     and "\<rho> x\<^sub>s = Some (VClosure (Right x\<^sub>r') \<rho>\<^sub>r)"
     and "\<rho>\<^sub>r x\<^sub>r' = Some \<omega>\<^sub>r"
     with `(\<V>, \<C>) \<Turnstile>\<^sub>\<sigma> \<sigma>`
-    show "(\<V>, \<C>) \<Turnstile>\<^sub>\<sigma> \<sigma>'" by (simp add: maybe_static_eval_state_to_state_let_case_right)
+    show "(\<V>, \<C>) \<Turnstile>\<^sub>\<sigma> \<sigma>'" by (simp add: may_be_static_eval_state_to_state_let_case_right)
   next
     case (Let_App \<rho> f f\<^sub>l x\<^sub>l e\<^sub>l \<rho>\<^sub>l x\<^sub>a \<omega>\<^sub>a x e \<kappa>)
     assume "\<sigma> = \<langle>LET x = APP f x\<^sub>a in e;\<rho>;\<kappa>\<rangle>"
@@ -877,73 +877,73 @@ proof -
     and "\<rho> f = Some (VClosure (Abs f\<^sub>l x\<^sub>l e\<^sub>l) \<rho>\<^sub>l)"
     and "\<rho> x\<^sub>a = Some \<omega>\<^sub>a"
     with `(\<V>, \<C>) \<Turnstile>\<^sub>\<sigma> \<sigma>`
-    show "(\<V>, \<C>) \<Turnstile>\<^sub>\<sigma> \<sigma>'" by (simp add: maybe_static_eval_state_to_state_let_app)
+    show "(\<V>, \<C>) \<Turnstile>\<^sub>\<sigma> \<sigma>'" by (simp add: may_be_static_eval_state_to_state_let_app)
   qed
 
 qed
 
-lemma maybe_static_eval_preserved_under_seq_step_down: "
+lemma may_be_static_eval_preserved_under_seq_step_down: "
   (\<V>, \<C>) \<Turnstile>\<^sub>\<E> \<E> \<Longrightarrow> leaf \<E> \<pi> \<Longrightarrow> \<E> \<pi> = Some (\<langle>RESULT x; \<rho>; \<langle>x\<^sub>\<kappa>, e\<^sub>\<kappa>, \<rho>\<^sub>\<kappa>\<rangle> # \<kappa>\<rangle>) \<Longrightarrow> 
   \<langle>RESULT x; \<rho>; \<langle>x\<^sub>\<kappa>, e\<^sub>\<kappa>, \<rho>\<^sub>\<kappa>\<rangle> # \<kappa>\<rangle> \<hookrightarrow> \<sigma>' \<Longrightarrow> (\<V>, \<C>) \<Turnstile>\<^sub>\<E> \<E>(\<pi> ;;(LReturn x\<^sub>\<kappa>) \<mapsto> \<sigma>')
 "
 proof
   
   assume "(\<V>, \<C>) \<Turnstile>\<^sub>\<E> \<E>" and "\<E> \<pi> = Some (\<langle>RESULT x; \<rho>; \<langle>x\<^sub>\<kappa>, e\<^sub>\<kappa>, \<rho>\<^sub>\<kappa>\<rangle> # \<kappa>\<rangle>)" then
-  have "(\<V>, \<C>) \<Turnstile>\<^sub>\<sigma> \<langle>RESULT x; \<rho>; \<langle>x\<^sub>\<kappa>, e\<^sub>\<kappa>, \<rho>\<^sub>\<kappa>\<rangle> # \<kappa>\<rangle>" by (simp add: maybe_static_eval_pool.simps)
+  have "(\<V>, \<C>) \<Turnstile>\<^sub>\<sigma> \<langle>RESULT x; \<rho>; \<langle>x\<^sub>\<kappa>, e\<^sub>\<kappa>, \<rho>\<^sub>\<kappa>\<rangle> # \<kappa>\<rangle>" by (simp add: may_be_static_eval_pool.simps)
   
   assume "\<langle>RESULT x; \<rho>; \<langle>x\<^sub>\<kappa>, e\<^sub>\<kappa>, \<rho>\<^sub>\<kappa>\<rangle> # \<kappa>\<rangle> \<hookrightarrow> \<sigma>'" with `(\<V>, \<C>) \<Turnstile>\<^sub>\<sigma> \<langle>RESULT x; \<rho>; \<langle>x\<^sub>\<kappa>, e\<^sub>\<kappa>, \<rho>\<^sub>\<kappa>\<rangle> # \<kappa>\<rangle>`
-  have "(\<V>, \<C>) \<Turnstile>\<^sub>\<sigma> \<sigma>'" by (simp add: maybe_static_eval_state_preserved_under_step)
+  have "(\<V>, \<C>) \<Turnstile>\<^sub>\<sigma> \<sigma>'" by (simp add: may_be_static_eval_state_preserved_under_step)
 
   from \<open>(\<V>, \<C>) \<Turnstile>\<^sub>\<E> \<E>\<close> \<open>(\<V>, \<C>) \<Turnstile>\<^sub>\<sigma> \<sigma>'\<close>
-  show "\<forall>\<pi>' \<sigma>. (\<E>(\<pi> ;;(LReturn x\<^sub>\<kappa>) \<mapsto> \<sigma>')) \<pi>' = Some \<sigma> \<longrightarrow> (\<V>, \<C>) \<Turnstile>\<^sub>\<sigma> \<sigma>" by (simp add: maybe_static_eval_pool.simps)
+  show "\<forall>\<pi>' \<sigma>. (\<E>(\<pi> ;;(LReturn x\<^sub>\<kappa>) \<mapsto> \<sigma>')) \<pi>' = Some \<sigma> \<longrightarrow> (\<V>, \<C>) \<Turnstile>\<^sub>\<sigma> \<sigma>" by (simp add: may_be_static_eval_pool.simps)
 
 qed
 
 
-lemma maybe_static_eval_preserved_under_seq_step_up: "
+lemma may_be_static_eval_preserved_under_seq_step_up: "
   (\<V>, \<C>) \<Turnstile>\<^sub>\<E> \<E> \<Longrightarrow> leaf \<E> \<pi> \<Longrightarrow> \<E> \<pi> = Some (\<langle>LET x = b in e; \<rho>; \<kappa>\<rangle>) \<Longrightarrow> 
   \<langle>LET x = b in e; \<rho>; \<kappa>\<rangle> \<hookrightarrow> \<sigma>' \<Longrightarrow> (\<V>, \<C>) \<Turnstile>\<^sub>\<E> \<E>(\<pi>;;(LCall x) \<mapsto> \<sigma>')
 "
 proof
   assume "(\<V>, \<C>) \<Turnstile>\<^sub>\<E> \<E>" and "\<E> \<pi> = Some (\<langle>LET x = b in e; \<rho>; \<kappa>\<rangle>)" then
-  have "(\<V>, \<C>) \<Turnstile>\<^sub>\<sigma> \<langle>LET x = b in e; \<rho>; \<kappa>\<rangle>" by (simp add: maybe_static_eval_pool.simps)
+  have "(\<V>, \<C>) \<Turnstile>\<^sub>\<sigma> \<langle>LET x = b in e; \<rho>; \<kappa>\<rangle>" by (simp add: may_be_static_eval_pool.simps)
 
   assume "\<langle>LET x = b in e; \<rho>; \<kappa>\<rangle> \<hookrightarrow> \<sigma>'" with `(\<V>, \<C>) \<Turnstile>\<^sub>\<sigma> \<langle>LET x = b in e; \<rho>; \<kappa>\<rangle>`
-  have "(\<V>, \<C>) \<Turnstile>\<^sub>\<sigma> \<sigma>'" by (simp add: maybe_static_eval_state_preserved_under_step)
+  have "(\<V>, \<C>) \<Turnstile>\<^sub>\<sigma> \<sigma>'" by (simp add: may_be_static_eval_state_preserved_under_step)
 
   from \<open>(\<V>, \<C>) \<Turnstile>\<^sub>\<E> \<E>\<close> \<open>(\<V>, \<C>) \<Turnstile>\<^sub>\<sigma> \<sigma>'\<close>
-  show "\<forall>\<pi>' \<sigma>. (\<E>(\<pi> ;;(LCall x) \<mapsto> \<sigma>')) \<pi>' = Some \<sigma> \<longrightarrow> (\<V>, \<C>) \<Turnstile>\<^sub>\<sigma> \<sigma>" by (simp add: maybe_static_eval_pool.simps)
+  show "\<forall>\<pi>' \<sigma>. (\<E>(\<pi> ;;(LCall x) \<mapsto> \<sigma>')) \<pi>' = Some \<sigma> \<longrightarrow> (\<V>, \<C>) \<Turnstile>\<^sub>\<sigma> \<sigma>" by (simp add: may_be_static_eval_pool.simps)
 qed
 
 
-lemma maybe_static_eval_preserved_under_seq_step: "
+lemma may_be_static_eval_preserved_under_seq_step: "
   (\<V>, \<C>) \<Turnstile>\<^sub>\<E> \<E> \<Longrightarrow> leaf \<E> \<pi> \<Longrightarrow> \<E> \<pi> = Some (\<langle>LET x = b in e; \<rho>; \<kappa>\<rangle>) \<Longrightarrow> 
   \<langle>LET x = b in e; \<rho>; \<kappa>\<rangle> \<hookrightarrow> \<sigma>' \<Longrightarrow> (\<V>, \<C>) \<Turnstile>\<^sub>\<E> \<E>(\<pi> ;;(LNext x) \<mapsto> \<sigma>')
 "
 proof
   assume "(\<V>, \<C>) \<Turnstile>\<^sub>\<E> \<E>" and "\<E> \<pi> = Some (\<langle>LET x = b in e; \<rho>; \<kappa>\<rangle>)" then
-  have "(\<V>, \<C>) \<Turnstile>\<^sub>\<sigma> \<langle>LET x = b in e; \<rho>; \<kappa>\<rangle>" by (simp add: maybe_static_eval_pool.simps)
+  have "(\<V>, \<C>) \<Turnstile>\<^sub>\<sigma> \<langle>LET x = b in e; \<rho>; \<kappa>\<rangle>" by (simp add: may_be_static_eval_pool.simps)
 
   assume "\<langle>LET x = b in e; \<rho>; \<kappa>\<rangle> \<hookrightarrow> \<sigma>'" with `(\<V>, \<C>) \<Turnstile>\<^sub>\<sigma> \<langle>LET x = b in e; \<rho>; \<kappa>\<rangle>`
-  have "(\<V>, \<C>) \<Turnstile>\<^sub>\<sigma> \<sigma>'" by (simp add: maybe_static_eval_state_preserved_under_step)
+  have "(\<V>, \<C>) \<Turnstile>\<^sub>\<sigma> \<sigma>'" by (simp add: may_be_static_eval_state_preserved_under_step)
 
   from \<open>(\<V>, \<C>) \<Turnstile>\<^sub>\<E> \<E>\<close> \<open>(\<V>, \<C>) \<Turnstile>\<^sub>\<sigma> \<sigma>'\<close>
-  show "\<forall>\<pi>' \<sigma>. (\<E>(\<pi> ;;(LNext x) \<mapsto> \<sigma>')) \<pi>' = Some \<sigma> \<longrightarrow> (\<V>, \<C>) \<Turnstile>\<^sub>\<sigma> \<sigma>" by (simp add: maybe_static_eval_pool.simps)
+  show "\<forall>\<pi>' \<sigma>. (\<E>(\<pi> ;;(LNext x) \<mapsto> \<sigma>')) \<pi>' = Some \<sigma> \<longrightarrow> (\<V>, \<C>) \<Turnstile>\<^sub>\<sigma> \<sigma>" by (simp add: may_be_static_eval_pool.simps)
 qed
 
-lemma maybe_static_eval_pool_to_exp_let: "
+lemma may_be_static_eval_pool_to_exp_let: "
   (\<V>, \<C>) \<Turnstile>\<^sub>\<E> \<E> \<Longrightarrow>
   \<E> \<pi> = Some (\<langle>LET x = b in e; \<rho>; \<kappa>\<rangle>) \<Longrightarrow>
   (\<V>, \<C>) \<Turnstile>\<^sub>e e
 "
 proof -
  assume "(\<V>, \<C>) \<Turnstile>\<^sub>\<E> \<E>" and "\<E> \<pi> = Some (\<langle>LET x = b in e; \<rho>; \<kappa>\<rangle>)" then
- have "(\<V>, \<C>) \<Turnstile>\<^sub>\<sigma> \<langle>LET x = b in e; \<rho>; \<kappa>\<rangle>" by (simp add: maybe_static_eval_pool.simps) then
- show "(\<V>, \<C>) \<Turnstile>\<^sub>e e " by (blast intro: maybe_static_eval_state_to_exp_let)
+ have "(\<V>, \<C>) \<Turnstile>\<^sub>\<sigma> \<langle>LET x = b in e; \<rho>; \<kappa>\<rangle>" by (simp add: may_be_static_eval_pool.simps) then
+ show "(\<V>, \<C>) \<Turnstile>\<^sub>e e " by (blast intro: may_be_static_eval_state_to_exp_let)
 qed
 
 
-lemma maybe_static_eval_pool_let_sync_send_values_relate: "
+lemma may_be_static_eval_pool_let_sync_send_values_relate: "
   (\<V>, \<C>) \<Turnstile>\<^sub>\<E> \<E> \<Longrightarrow>
   \<E> \<pi>\<^sub>s = Some (\<langle>LET x\<^sub>s = SYNC x\<^sub>s\<^sub>e in e\<^sub>s; \<rho>\<^sub>s; \<kappa>\<^sub>s\<rangle>) \<Longrightarrow>
   \<rho>\<^sub>s x\<^sub>s\<^sub>e = Some (VClosure (Send_Evt x\<^sub>s\<^sub>c x\<^sub>m) \<rho>\<^sub>s\<^sub>e) \<Longrightarrow>
@@ -957,19 +957,19 @@ proof -
   and "\<rho>\<^sub>s\<^sub>e x\<^sub>s\<^sub>c = Some (VChan (Ch \<pi>\<^sub>c x\<^sub>c))"
 
   from `(\<V>, \<C>) \<Turnstile>\<^sub>\<E> \<E>` and `\<E> \<pi>\<^sub>s = Some (\<langle>LET x\<^sub>s = SYNC x\<^sub>s\<^sub>e in e\<^sub>s; \<rho>\<^sub>s; \<kappa>\<^sub>s\<rangle>)`
-  have "(\<V>, \<C>) \<Turnstile>\<^sub>\<sigma> \<langle>LET x\<^sub>s = SYNC x\<^sub>s\<^sub>e in e\<^sub>s; \<rho>\<^sub>s; \<kappa>\<^sub>s\<rangle>" by (simp add: maybe_static_eval_pool.simps) then
-  have "(\<V>, \<C>) \<Turnstile>\<^sub>e LET x\<^sub>s = SYNC x\<^sub>s\<^sub>e in e\<^sub>s" "(\<V>, \<C>) \<Turnstile>\<^sub>\<rho> \<rho>\<^sub>s" by (simp add: maybe_static_eval_state.simps)+
+  have "(\<V>, \<C>) \<Turnstile>\<^sub>\<sigma> \<langle>LET x\<^sub>s = SYNC x\<^sub>s\<^sub>e in e\<^sub>s; \<rho>\<^sub>s; \<kappa>\<^sub>s\<rangle>" by (simp add: may_be_static_eval_pool.simps) then
+  have "(\<V>, \<C>) \<Turnstile>\<^sub>e LET x\<^sub>s = SYNC x\<^sub>s\<^sub>e in e\<^sub>s" "(\<V>, \<C>) \<Turnstile>\<^sub>\<rho> \<rho>\<^sub>s" by (simp add: may_be_static_eval_state.simps)+
 
   from `(\<V>, \<C>) \<Turnstile>\<^sub>\<rho> \<rho>\<^sub>s` and `\<rho>\<^sub>s x\<^sub>s\<^sub>e = Some (VClosure (Send_Evt x\<^sub>s\<^sub>c x\<^sub>m) \<rho>\<^sub>s\<^sub>e)`
-  have "{|(VClosure (Send_Evt x\<^sub>s\<^sub>c x\<^sub>m) \<rho>\<^sub>s\<^sub>e)|} \<subseteq> \<V> x\<^sub>s\<^sub>e" and "(\<V>, \<C>) \<Turnstile>\<^sub>\<omega> (VClosure (Send_Evt x\<^sub>s\<^sub>c x\<^sub>m) \<rho>\<^sub>s\<^sub>e)" by (blast intro: maybe_static_eval_env.cases)+
+  have "{|(VClosure (Send_Evt x\<^sub>s\<^sub>c x\<^sub>m) \<rho>\<^sub>s\<^sub>e)|} \<subseteq> \<V> x\<^sub>s\<^sub>e" and "(\<V>, \<C>) \<Turnstile>\<^sub>\<omega> (VClosure (Send_Evt x\<^sub>s\<^sub>c x\<^sub>m) \<rho>\<^sub>s\<^sub>e)" by (blast intro: may_be_static_eval_env.cases)+
 
   from `{|(VClosure (Send_Evt x\<^sub>s\<^sub>c x\<^sub>m) \<rho>\<^sub>s\<^sub>e)|} \<subseteq> \<V> x\<^sub>s\<^sub>e`
   have "^Send_Evt x\<^sub>s\<^sub>c x\<^sub>m \<in> \<V> x\<^sub>s\<^sub>e" by simp
 
   from `(\<V>, \<C>) \<Turnstile>\<^sub>\<omega> (VClosure (Send_Evt x\<^sub>s\<^sub>c x\<^sub>m) \<rho>\<^sub>s\<^sub>e)`
-  have "(\<V>, \<C>) \<Turnstile>\<^sub>\<rho> \<rho>\<^sub>s\<^sub>e" by (blast intro: maybe_static_eval_value.cases)
+  have "(\<V>, \<C>) \<Turnstile>\<^sub>\<rho> \<rho>\<^sub>s\<^sub>e" by (blast intro: may_be_static_eval_value.cases)
   with `\<rho>\<^sub>s\<^sub>e x\<^sub>s\<^sub>c = Some (VChan (Ch \<pi>\<^sub>c x\<^sub>c))`
-  have "{|(VChan (Ch \<pi>\<^sub>c x\<^sub>c))|} \<subseteq> \<V> x\<^sub>s\<^sub>c" by (blast intro: maybe_static_eval_env.cases) then
+  have "{|(VChan (Ch \<pi>\<^sub>c x\<^sub>c))|} \<subseteq> \<V> x\<^sub>s\<^sub>c" by (blast intro: may_be_static_eval_env.cases) then
   have "{^Chan x\<^sub>c} \<subseteq> \<V> x\<^sub>s\<^sub>c" by simp then
   have "^Chan x\<^sub>c \<in> \<V> x\<^sub>s\<^sub>c" by auto
   
@@ -984,7 +984,7 @@ proof -
 
 qed
 
-lemma maybe_static_eval_pool_let_sync_send_message_relate: "
+lemma may_be_static_eval_pool_let_sync_send_message_relate: "
   (\<V>, \<C>) \<Turnstile>\<^sub>\<E> \<E> \<Longrightarrow>
   \<E> \<pi>\<^sub>s = Some (\<langle>LET x\<^sub>s = SYNC x\<^sub>s\<^sub>e in e\<^sub>s; \<rho>\<^sub>s; \<kappa>\<^sub>s\<rangle>) \<Longrightarrow>
   \<rho>\<^sub>s x\<^sub>s\<^sub>e = Some (VClosure (Send_Evt x\<^sub>s\<^sub>c x\<^sub>m) \<rho>\<^sub>s\<^sub>e) \<Longrightarrow>
@@ -998,16 +998,16 @@ proof -
   and "\<rho>\<^sub>s\<^sub>e x\<^sub>m = Some \<omega>\<^sub>m"
 
   from `(\<V>, \<C>) \<Turnstile>\<^sub>\<E> \<E>` and `\<E> \<pi>\<^sub>s = Some (\<langle>LET x\<^sub>s = SYNC x\<^sub>s\<^sub>e in e\<^sub>s; \<rho>\<^sub>s; \<kappa>\<^sub>s\<rangle>)`
-  have "(\<V>, \<C>) \<Turnstile>\<^sub>\<sigma> \<langle>LET x\<^sub>s = SYNC x\<^sub>s\<^sub>e in e\<^sub>s; \<rho>\<^sub>s; \<kappa>\<^sub>s\<rangle>" by (simp add: maybe_static_eval_pool.simps) then
-  have "(\<V>, \<C>) \<Turnstile>\<^sub>\<rho> \<rho>\<^sub>s" by (simp add: maybe_static_eval_state.simps)
+  have "(\<V>, \<C>) \<Turnstile>\<^sub>\<sigma> \<langle>LET x\<^sub>s = SYNC x\<^sub>s\<^sub>e in e\<^sub>s; \<rho>\<^sub>s; \<kappa>\<^sub>s\<rangle>" by (simp add: may_be_static_eval_pool.simps) then
+  have "(\<V>, \<C>) \<Turnstile>\<^sub>\<rho> \<rho>\<^sub>s" by (simp add: may_be_static_eval_state.simps)
   with `\<rho>\<^sub>s x\<^sub>s\<^sub>e = Some (VClosure (Send_Evt x\<^sub>s\<^sub>c x\<^sub>m) \<rho>\<^sub>s\<^sub>e)`
-  have "(\<V>, \<C>) \<Turnstile>\<^sub>\<omega> (VClosure (Send_Evt x\<^sub>s\<^sub>c x\<^sub>m) \<rho>\<^sub>s\<^sub>e)" by (blast intro: maybe_static_eval_env.cases) then
-  have "(\<V>, \<C>) \<Turnstile>\<^sub>\<rho> \<rho>\<^sub>s\<^sub>e" by (blast intro: maybe_static_eval_value.cases)
+  have "(\<V>, \<C>) \<Turnstile>\<^sub>\<omega> (VClosure (Send_Evt x\<^sub>s\<^sub>c x\<^sub>m) \<rho>\<^sub>s\<^sub>e)" by (blast intro: may_be_static_eval_env.cases) then
+  have "(\<V>, \<C>) \<Turnstile>\<^sub>\<rho> \<rho>\<^sub>s\<^sub>e" by (blast intro: may_be_static_eval_value.cases)
   with `\<rho>\<^sub>s\<^sub>e x\<^sub>m = Some \<omega>\<^sub>m`
-  show "{|\<omega>\<^sub>m|} \<subseteq> \<V> x\<^sub>m \<and> (\<V>, \<C>) \<Turnstile>\<^sub>\<omega> \<omega>\<^sub>m" by (blast intro: maybe_static_eval_env.cases)
+  show "{|\<omega>\<^sub>m|} \<subseteq> \<V> x\<^sub>m \<and> (\<V>, \<C>) \<Turnstile>\<^sub>\<omega> \<omega>\<^sub>m" by (blast intro: may_be_static_eval_env.cases)
 qed
 
-lemma maybe_static_eval_pool_to_env_let_sync_send: "
+lemma may_be_static_eval_pool_to_env_let_sync_send: "
   (\<V>, \<C>) \<Turnstile>\<^sub>\<E> \<E> \<Longrightarrow>
   \<E> \<pi>\<^sub>s = Some (\<langle>LET x\<^sub>s = SYNC x\<^sub>s\<^sub>e in e\<^sub>s; \<rho>\<^sub>s; \<kappa>\<^sub>s\<rangle>) \<Longrightarrow>
   \<rho>\<^sub>s x\<^sub>s\<^sub>e = Some (VClosure (Send_Evt x\<^sub>s\<^sub>c x\<^sub>m) \<rho>\<^sub>s\<^sub>e) \<Longrightarrow>
@@ -1021,8 +1021,8 @@ proof
   and "\<rho>\<^sub>s x\<^sub>s\<^sub>e = Some (VClosure (Send_Evt x\<^sub>s\<^sub>c x\<^sub>m) \<rho>\<^sub>s\<^sub>e)"
 
   from `(\<V>, \<C>) \<Turnstile>\<^sub>\<E> \<E>` and `\<E> \<pi>\<^sub>s = Some (\<langle>LET x\<^sub>s = SYNC x\<^sub>s\<^sub>e in e\<^sub>s; \<rho>\<^sub>s; \<kappa>\<^sub>s\<rangle>)`
-  have "(\<V>, \<C>) \<Turnstile>\<^sub>\<sigma> \<langle>LET x\<^sub>s = SYNC x\<^sub>s\<^sub>e in e\<^sub>s; \<rho>\<^sub>s; \<kappa>\<^sub>s\<rangle>" by (simp add: maybe_static_eval_pool.simps) then
-  have "(\<V>, \<C>) \<Turnstile>\<^sub>\<rho> \<rho>\<^sub>s" by (simp add: maybe_static_eval_state.simps)+
+  have "(\<V>, \<C>) \<Turnstile>\<^sub>\<sigma> \<langle>LET x\<^sub>s = SYNC x\<^sub>s\<^sub>e in e\<^sub>s; \<rho>\<^sub>s; \<kappa>\<^sub>s\<rangle>" by (simp add: may_be_static_eval_pool.simps) then
+  have "(\<V>, \<C>) \<Turnstile>\<^sub>\<rho> \<rho>\<^sub>s" by (simp add: may_be_static_eval_state.simps)+
 
   have "{^\<lparr>\<rparr>} \<subseteq> \<V> x\<^sub>s"
   proof (cases c)
@@ -1032,7 +1032,7 @@ proof
     and  `(\<V>, \<C>) \<Turnstile>\<^sub>\<E> \<E>`
     and `\<E> \<pi>\<^sub>s = Some (\<langle>LET x\<^sub>s = SYNC x\<^sub>s\<^sub>e in e\<^sub>s; \<rho>\<^sub>s; \<kappa>\<^sub>s\<rangle>)`
     and `\<rho>\<^sub>s x\<^sub>s\<^sub>e = Some (VClosure (Send_Evt x\<^sub>s\<^sub>c x\<^sub>m) \<rho>\<^sub>s\<^sub>e)`
-    show "{^\<lparr>\<rparr>} \<subseteq> \<V> x\<^sub>s" using maybe_static_eval_pool_let_sync_send_values_relate by simp
+    show "{^\<lparr>\<rparr>} \<subseteq> \<V> x\<^sub>s" using may_be_static_eval_pool_let_sync_send_values_relate by simp
   qed
   
   have "(\<V>, \<C>) \<Turnstile>\<^sub>\<omega> VUnit" by (simp add: Unit)
@@ -1041,14 +1041,14 @@ proof
     assume "(\<rho>\<^sub>s(x\<^sub>s \<mapsto> VUnit)) x' = Some \<omega>'" "x' \<noteq> x\<^sub>s" then
     have "\<rho>\<^sub>s x' = Some \<omega>'" by simp
     with `(\<V>, \<C>) \<Turnstile>\<^sub>\<rho> \<rho>\<^sub>s` 
-    have "{|\<omega>'|} \<subseteq> \<V> x' \<and> (\<V>, \<C>) \<Turnstile>\<^sub>\<omega> \<omega>'" by (simp add: maybe_static_eval_env.simps)
+    have "{|\<omega>'|} \<subseteq> \<V> x' \<and> (\<V>, \<C>) \<Turnstile>\<^sub>\<omega> \<omega>'" by (simp add: may_be_static_eval_env.simps)
   }
   with \<open>{^\<lparr>\<rparr>} \<subseteq> \<V> x\<^sub>s\<close> \<open>(\<V>, \<C>) \<Turnstile>\<^sub>\<omega> VUnit\<close> 
   show "\<forall>x \<omega>. (\<rho>\<^sub>s(x\<^sub>s \<mapsto> VUnit)) x = Some \<omega> \<longrightarrow> {|\<omega>|} \<subseteq> \<V> x \<and> (\<V>, \<C>) \<Turnstile>\<^sub>\<omega> \<omega>" by simp
 qed
 
 
-lemma maybe_static_eval_pool_let_sync_recv_values_relate: "
+lemma may_be_static_eval_pool_let_sync_recv_values_relate: "
   (\<V>, \<C>) \<Turnstile>\<^sub>\<E> \<E> \<Longrightarrow>
   \<E> \<pi>\<^sub>r = Some (\<langle>LET x\<^sub>r = SYNC x\<^sub>r\<^sub>e in e\<^sub>r; \<rho>\<^sub>r; \<kappa>\<^sub>r\<rangle>) \<Longrightarrow>
   \<rho>\<^sub>r x\<^sub>r\<^sub>e = Some (VClosure (Recv_Evt x\<^sub>r\<^sub>c) \<rho>\<^sub>r\<^sub>e) \<Longrightarrow>
@@ -1062,19 +1062,19 @@ proof -
   and "\<rho>\<^sub>r\<^sub>e x\<^sub>r\<^sub>c = Some (VChan (Ch \<pi>\<^sub>c x\<^sub>c))"
 
   from `(\<V>, \<C>) \<Turnstile>\<^sub>\<E> \<E>` and `\<E> \<pi>\<^sub>r = Some (\<langle>LET x\<^sub>r = SYNC x\<^sub>r\<^sub>e in e\<^sub>r; \<rho>\<^sub>r; \<kappa>\<^sub>r\<rangle>)`
-  have "(\<V>, \<C>) \<Turnstile>\<^sub>\<sigma> \<langle>LET x\<^sub>r = SYNC x\<^sub>r\<^sub>e in e\<^sub>r; \<rho>\<^sub>r; \<kappa>\<^sub>r\<rangle>" by (simp add: maybe_static_eval_pool.simps) then
-  have "(\<V>, \<C>) \<Turnstile>\<^sub>e LET x\<^sub>r = SYNC x\<^sub>r\<^sub>e in e\<^sub>r" "(\<V>, \<C>) \<Turnstile>\<^sub>\<rho> \<rho>\<^sub>r" by (simp add: maybe_static_eval_state.simps)+
+  have "(\<V>, \<C>) \<Turnstile>\<^sub>\<sigma> \<langle>LET x\<^sub>r = SYNC x\<^sub>r\<^sub>e in e\<^sub>r; \<rho>\<^sub>r; \<kappa>\<^sub>r\<rangle>" by (simp add: may_be_static_eval_pool.simps) then
+  have "(\<V>, \<C>) \<Turnstile>\<^sub>e LET x\<^sub>r = SYNC x\<^sub>r\<^sub>e in e\<^sub>r" "(\<V>, \<C>) \<Turnstile>\<^sub>\<rho> \<rho>\<^sub>r" by (simp add: may_be_static_eval_state.simps)+
 
   from `(\<V>, \<C>) \<Turnstile>\<^sub>\<rho> \<rho>\<^sub>r` and `\<rho>\<^sub>r x\<^sub>r\<^sub>e = Some (VClosure (Recv_Evt x\<^sub>r\<^sub>c) \<rho>\<^sub>r\<^sub>e)`
-  have "{|(VClosure (Recv_Evt x\<^sub>r\<^sub>c) \<rho>\<^sub>r\<^sub>e)|} \<subseteq> \<V> x\<^sub>r\<^sub>e" and "(\<V>, \<C>) \<Turnstile>\<^sub>\<omega> (VClosure (Recv_Evt x\<^sub>r\<^sub>c) \<rho>\<^sub>r\<^sub>e)" by (blast intro: maybe_static_eval_env.cases)+
+  have "{|(VClosure (Recv_Evt x\<^sub>r\<^sub>c) \<rho>\<^sub>r\<^sub>e)|} \<subseteq> \<V> x\<^sub>r\<^sub>e" and "(\<V>, \<C>) \<Turnstile>\<^sub>\<omega> (VClosure (Recv_Evt x\<^sub>r\<^sub>c) \<rho>\<^sub>r\<^sub>e)" by (blast intro: may_be_static_eval_env.cases)+
 
   from `{|(VClosure (Recv_Evt x\<^sub>r\<^sub>c) \<rho>\<^sub>r\<^sub>e)|} \<subseteq> \<V> x\<^sub>r\<^sub>e`
   have "^Recv_Evt x\<^sub>r\<^sub>c \<in> \<V> x\<^sub>r\<^sub>e" by simp
 
   from `(\<V>, \<C>) \<Turnstile>\<^sub>\<omega> (VClosure (Recv_Evt x\<^sub>r\<^sub>c) \<rho>\<^sub>r\<^sub>e)`
-  have "(\<V>, \<C>) \<Turnstile>\<^sub>\<rho> \<rho>\<^sub>r\<^sub>e" by (blast intro: maybe_static_eval_value.cases)
+  have "(\<V>, \<C>) \<Turnstile>\<^sub>\<rho> \<rho>\<^sub>r\<^sub>e" by (blast intro: may_be_static_eval_value.cases)
   with `\<rho>\<^sub>r\<^sub>e x\<^sub>r\<^sub>c = Some (VChan (Ch \<pi>\<^sub>c x\<^sub>c))`
-  have "{|(VChan (Ch \<pi>\<^sub>c x\<^sub>c))|} \<subseteq> \<V> x\<^sub>r\<^sub>c" by (blast intro: maybe_static_eval_env.cases) then
+  have "{|(VChan (Ch \<pi>\<^sub>c x\<^sub>c))|} \<subseteq> \<V> x\<^sub>r\<^sub>c" by (blast intro: may_be_static_eval_env.cases) then
   have "{^Chan x\<^sub>c} \<subseteq> \<V> x\<^sub>r\<^sub>c" by simp then
   have "^Chan x\<^sub>c \<in> \<V> x\<^sub>r\<^sub>c" by auto
   
@@ -1089,18 +1089,18 @@ proof -
 qed
 
 
-lemma maybe_static_eval_pool_to_stack_let: "
+lemma may_be_static_eval_pool_to_stack_let: "
   (\<V>, \<C>) \<Turnstile>\<^sub>\<E> \<E> \<Longrightarrow>
   \<E> \<pi> = Some (\<langle>LET x = b in e; \<rho>; \<kappa>\<rangle>) \<Longrightarrow>
   (\<V>, \<C>) \<Turnstile>\<^sub>\<kappa> \<V> (\<lfloor>e\<rfloor>) \<Rrightarrow> \<kappa>
 "
 proof -
   assume "(\<V>, \<C>) \<Turnstile>\<^sub>\<E> \<E>" and "\<E> \<pi> = Some (\<langle>LET x = b in e; \<rho>; \<kappa>\<rangle>)" then
-  have "(\<V>, \<C>) \<Turnstile>\<^sub>\<sigma> \<langle>LET x = b in e; \<rho>; \<kappa>\<rangle>" by (simp add: maybe_static_eval_pool.simps) then
-  show "(\<V>, \<C>) \<Turnstile>\<^sub>\<kappa> \<V> (\<lfloor>e\<rfloor>) \<Rrightarrow> \<kappa>" by (simp add: maybe_static_eval_state_to_stack_let)
+  have "(\<V>, \<C>) \<Turnstile>\<^sub>\<sigma> \<langle>LET x = b in e; \<rho>; \<kappa>\<rangle>" by (simp add: may_be_static_eval_pool.simps) then
+  show "(\<V>, \<C>) \<Turnstile>\<^sub>\<kappa> \<V> (\<lfloor>e\<rfloor>) \<Rrightarrow> \<kappa>" by (simp add: may_be_static_eval_state_to_stack_let)
 qed
 
-lemma maybe_static_eval_pool_to_env_let_sync_recv: "
+lemma may_be_static_eval_pool_to_env_let_sync_recv: "
   (\<V>, \<C>) \<Turnstile>\<^sub>\<E> \<E> \<Longrightarrow>
   \<E> \<pi>\<^sub>s = Some (\<langle>LET x\<^sub>s = SYNC x\<^sub>s\<^sub>e in e\<^sub>s; \<rho>\<^sub>s; \<kappa>\<^sub>s\<rangle>) \<Longrightarrow>
   \<rho>\<^sub>s x\<^sub>s\<^sub>e = Some (VClosure (Send_Evt x\<^sub>s\<^sub>c x\<^sub>m) \<rho>\<^sub>s\<^sub>e) \<Longrightarrow>
@@ -1116,7 +1116,7 @@ proof
   and "\<E> \<pi>\<^sub>s = Some (\<langle>LET x\<^sub>s = SYNC x\<^sub>s\<^sub>e in e\<^sub>s; \<rho>\<^sub>s; \<kappa>\<^sub>s\<rangle>)"
   and "\<rho>\<^sub>s x\<^sub>s\<^sub>e = Some (VClosure (Send_Evt x\<^sub>s\<^sub>c x\<^sub>m) \<rho>\<^sub>s\<^sub>e)"
   and "\<rho>\<^sub>s\<^sub>e x\<^sub>m = Some \<omega>\<^sub>m" then
-  have "{|\<omega>\<^sub>m|} \<subseteq> \<V> x\<^sub>m" "(\<V>, \<C>) \<Turnstile>\<^sub>\<omega> \<omega>\<^sub>m" using maybe_static_eval_pool_let_sync_send_message_relate by auto
+  have "{|\<omega>\<^sub>m|} \<subseteq> \<V> x\<^sub>m" "(\<V>, \<C>) \<Turnstile>\<^sub>\<omega> \<omega>\<^sub>m" using may_be_static_eval_pool_let_sync_send_message_relate by auto
 
   assume "\<rho>\<^sub>s\<^sub>e x\<^sub>s\<^sub>c = Some (VChan c)"
   and "\<E> \<pi>\<^sub>r = Some (\<langle>LET x\<^sub>r = SYNC x\<^sub>r\<^sub>e in e\<^sub>r; \<rho>\<^sub>r; \<kappa>\<^sub>r\<rangle>)"
@@ -1124,8 +1124,8 @@ proof
   and "\<rho>\<^sub>r\<^sub>e x\<^sub>r\<^sub>c = Some (VChan c)"
 
   from `(\<V>, \<C>) \<Turnstile>\<^sub>\<E> \<E>` and `\<E> \<pi>\<^sub>r = Some (\<langle>LET x\<^sub>r = SYNC x\<^sub>r\<^sub>e in e\<^sub>r; \<rho>\<^sub>r; \<kappa>\<^sub>r\<rangle>)`
-  have "(\<V>, \<C>) \<Turnstile>\<^sub>\<sigma> \<langle>LET x\<^sub>r = SYNC x\<^sub>r\<^sub>e in e\<^sub>r; \<rho>\<^sub>r; \<kappa>\<^sub>r\<rangle>" by (simp add: maybe_static_eval_pool.simps) then
-  have "(\<V>, \<C>) \<Turnstile>\<^sub>\<rho> \<rho>\<^sub>r" by (simp add: maybe_static_eval_state.simps)+
+  have "(\<V>, \<C>) \<Turnstile>\<^sub>\<sigma> \<langle>LET x\<^sub>r = SYNC x\<^sub>r\<^sub>e in e\<^sub>r; \<rho>\<^sub>r; \<kappa>\<^sub>r\<rangle>" by (simp add: may_be_static_eval_pool.simps) then
+  have "(\<V>, \<C>) \<Turnstile>\<^sub>\<rho> \<rho>\<^sub>r" by (simp add: may_be_static_eval_state.simps)+
 
 
   have "\<V> x\<^sub>m \<subseteq> \<V> x\<^sub>r"
@@ -1139,14 +1139,14 @@ proof
     and `\<rho>\<^sub>s x\<^sub>s\<^sub>e = Some (VClosure (Send_Evt x\<^sub>s\<^sub>c x\<^sub>m) \<rho>\<^sub>s\<^sub>e)`
     and `\<E> \<pi>\<^sub>s = Some (\<langle>LET x\<^sub>s = SYNC x\<^sub>s\<^sub>e in e\<^sub>s; \<rho>\<^sub>s; \<kappa>\<^sub>s\<rangle>)`
     and `\<rho>\<^sub>s\<^sub>e x\<^sub>m = Some \<omega>\<^sub>m`
-    have "\<V> x\<^sub>m \<subseteq> \<C> x\<^sub>c" using \<open>\<rho>\<^sub>s\<^sub>e x\<^sub>s\<^sub>c = Some (VChan c)\<close> maybe_static_eval_pool_let_sync_send_values_relate by blast
+    have "\<V> x\<^sub>m \<subseteq> \<C> x\<^sub>c" using \<open>\<rho>\<^sub>s\<^sub>e x\<^sub>s\<^sub>c = Some (VChan c)\<close> may_be_static_eval_pool_let_sync_send_values_relate by blast
 
     with `c = Ch \<pi>\<^sub>c x\<^sub>c`
     and `\<rho>\<^sub>r\<^sub>e x\<^sub>r\<^sub>c = Some (VChan c)`
     and `(\<V>, \<C>) \<Turnstile>\<^sub>\<E> \<E>`
     and `\<E> \<pi>\<^sub>r = Some (\<langle>LET x\<^sub>r = SYNC x\<^sub>r\<^sub>e in e\<^sub>r; \<rho>\<^sub>r; \<kappa>\<^sub>r\<rangle>)`
     and `\<rho>\<^sub>r x\<^sub>r\<^sub>e = Some (VClosure (Recv_Evt x\<^sub>r\<^sub>c) \<rho>\<^sub>r\<^sub>e)`
-    have "\<C> x\<^sub>c \<subseteq> \<V> x\<^sub>r" using  maybe_static_eval_pool_let_sync_recv_values_relate by auto
+    have "\<C> x\<^sub>c \<subseteq> \<V> x\<^sub>r" using  may_be_static_eval_pool_let_sync_recv_values_relate by auto
 
     from `\<V> x\<^sub>m \<subseteq> \<C> x\<^sub>c` and `\<C> x\<^sub>c \<subseteq> \<V> x\<^sub>r`
     show "\<V> x\<^sub>m \<subseteq> \<V> x\<^sub>r" by simp
@@ -1156,21 +1156,21 @@ proof
   have "{|\<omega>\<^sub>m|} \<subseteq> \<V> x\<^sub>r" by blast
 
   from `(\<V>, \<C>) \<Turnstile>\<^sub>\<E> \<E>` and `\<E> \<pi>\<^sub>s = Some (\<langle>LET x\<^sub>s = SYNC x\<^sub>s\<^sub>e in e\<^sub>s; \<rho>\<^sub>s; \<kappa>\<^sub>s\<rangle>)`
-  have "(\<V>, \<C>) \<Turnstile>\<^sub>\<sigma> \<langle>LET x\<^sub>s = SYNC x\<^sub>s\<^sub>e in e\<^sub>s; \<rho>\<^sub>s; \<kappa>\<^sub>s\<rangle>" by (simp add: maybe_static_eval_pool.simps) then
-  have "(\<V>, \<C>) \<Turnstile>\<^sub>\<rho> \<rho>\<^sub>s" by (simp add: maybe_static_eval_state.simps)+
+  have "(\<V>, \<C>) \<Turnstile>\<^sub>\<sigma> \<langle>LET x\<^sub>s = SYNC x\<^sub>s\<^sub>e in e\<^sub>s; \<rho>\<^sub>s; \<kappa>\<^sub>s\<rangle>" by (simp add: may_be_static_eval_pool.simps) then
+  have "(\<V>, \<C>) \<Turnstile>\<^sub>\<rho> \<rho>\<^sub>s" by (simp add: may_be_static_eval_state.simps)+
   {
     fix x' \<omega>'
     assume "(\<rho>\<^sub>r(x\<^sub>r \<mapsto> \<omega>\<^sub>m)) x' = Some \<omega>'" "x' \<noteq> x\<^sub>r" then
     have "\<rho>\<^sub>r x' = Some \<omega>'" by simp
     with `(\<V>, \<C>) \<Turnstile>\<^sub>\<rho> \<rho>\<^sub>r` 
-    have "{|\<omega>'|} \<subseteq> \<V> x' \<and> (\<V>, \<C>) \<Turnstile>\<^sub>\<omega> \<omega>'" by (simp add: maybe_static_eval_env.simps)
+    have "{|\<omega>'|} \<subseteq> \<V> x' \<and> (\<V>, \<C>) \<Turnstile>\<^sub>\<omega> \<omega>'" by (simp add: may_be_static_eval_env.simps)
   }
   with `{|\<omega>\<^sub>m|} \<subseteq> \<V> x\<^sub>r` and `(\<V>, \<C>) \<Turnstile>\<^sub>\<omega> \<omega>\<^sub>m`
   show "\<forall>x \<omega>. (\<rho>\<^sub>r(x\<^sub>r \<mapsto> \<omega>\<^sub>m)) x = Some \<omega> \<longrightarrow> {|\<omega>|} \<subseteq> \<V> x \<and> (\<V>, \<C>) \<Turnstile>\<^sub>\<omega> \<omega>" by auto
 qed
 
 
-lemma maybe_static_eval_preserved_under_sync: "
+lemma may_be_static_eval_preserved_under_sync: "
   (\<V>, \<C>) \<Turnstile>\<^sub>\<E> \<E> \<Longrightarrow>
   \<E> \<pi>\<^sub>s = Some (\<langle>LET x\<^sub>s = SYNC x\<^sub>s\<^sub>e in e\<^sub>s; \<rho>\<^sub>s; \<kappa>\<^sub>s\<rangle>) \<Longrightarrow>
   \<rho>\<^sub>s x\<^sub>s\<^sub>e = Some (VClosure (Send_Evt x\<^sub>s\<^sub>c x\<^sub>m) \<rho>\<^sub>s\<^sub>e) \<Longrightarrow>
@@ -1193,20 +1193,20 @@ proof
 
 
   from \<open>(\<V>, \<C>) \<Turnstile>\<^sub>\<E> \<E>\<close> and \<open>\<E> \<pi>\<^sub>s = Some (\<langle>LET x\<^sub>s = SYNC x\<^sub>s\<^sub>e in e\<^sub>s;\<rho>\<^sub>s;\<kappa>\<^sub>s\<rangle>)\<close> 
-  have "(\<V>, \<C>) \<Turnstile>\<^sub>e e\<^sub>s" by (blast intro: maybe_static_eval_pool_to_exp_let)
+  have "(\<V>, \<C>) \<Turnstile>\<^sub>e e\<^sub>s" by (blast intro: may_be_static_eval_pool_to_exp_let)
 
   from \<open>(\<V>, \<C>) \<Turnstile>\<^sub>\<E> \<E>\<close> \<open>\<E> \<pi>\<^sub>s = Some (\<langle>LET x\<^sub>s = SYNC x\<^sub>s\<^sub>e in e\<^sub>s;\<rho>\<^sub>s;\<kappa>\<^sub>s\<rangle>)\<close> 
   and \<open>\<rho>\<^sub>s x\<^sub>s\<^sub>e = Some (VClosure (Send_Evt x\<^sub>s\<^sub>c x\<^sub>m) \<rho>\<^sub>s\<^sub>e)\<close> \<open>\<rho>\<^sub>s\<^sub>e x\<^sub>s\<^sub>c = Some (VChan c)\<close> 
-  have "(\<V>, \<C>) \<Turnstile>\<^sub>\<rho> \<rho>\<^sub>s(x\<^sub>s \<mapsto> VUnit)" by (blast intro: maybe_static_eval_pool_to_env_let_sync_send)
+  have "(\<V>, \<C>) \<Turnstile>\<^sub>\<rho> \<rho>\<^sub>s(x\<^sub>s \<mapsto> VUnit)" by (blast intro: may_be_static_eval_pool_to_env_let_sync_send)
 
   from \<open>(\<V>, \<C>) \<Turnstile>\<^sub>\<E> \<E>\<close> and \<open>\<E> \<pi>\<^sub>s = Some (\<langle>LET x\<^sub>s = SYNC x\<^sub>s\<^sub>e in e\<^sub>s;\<rho>\<^sub>s;\<kappa>\<^sub>s\<rangle>)\<close>
-  have  "(\<V>, \<C>) \<Turnstile>\<^sub>\<kappa> \<V> (\<lfloor>e\<^sub>s\<rfloor>) \<Rrightarrow> \<kappa>\<^sub>s" by (blast intro: maybe_static_eval_pool_to_stack_let)
+  have  "(\<V>, \<C>) \<Turnstile>\<^sub>\<kappa> \<V> (\<lfloor>e\<^sub>s\<rfloor>) \<Rrightarrow> \<kappa>\<^sub>s" by (blast intro: may_be_static_eval_pool_to_stack_let)
 
   from `(\<V>, \<C>) \<Turnstile>\<^sub>e e\<^sub>s` and `(\<V>, \<C>) \<Turnstile>\<^sub>\<rho> \<rho>\<^sub>s(x\<^sub>s \<mapsto> VUnit)` and `(\<V>, \<C>) \<Turnstile>\<^sub>\<kappa> \<V> (\<lfloor>e\<^sub>s\<rfloor>) \<Rrightarrow> \<kappa>\<^sub>s`
-  have "(\<V>, \<C>) \<Turnstile>\<^sub>\<sigma> \<langle>e\<^sub>s;\<rho>\<^sub>s(x\<^sub>s \<mapsto> VUnit);\<kappa>\<^sub>s\<rangle>" by (blast intro: maybe_static_eval_state.intros)
+  have "(\<V>, \<C>) \<Turnstile>\<^sub>\<sigma> \<langle>e\<^sub>s;\<rho>\<^sub>s(x\<^sub>s \<mapsto> VUnit);\<kappa>\<^sub>s\<rangle>" by (blast intro: may_be_static_eval_state.intros)
 
   from \<open>(\<V>, \<C>) \<Turnstile>\<^sub>\<E> \<E>\<close> and \<open>\<E> \<pi>\<^sub>r = Some (\<langle>LET x\<^sub>r = SYNC x\<^sub>r\<^sub>e in e\<^sub>r;\<rho>\<^sub>r;\<kappa>\<^sub>r\<rangle>)\<close> 
-  have "(\<V>, \<C>) \<Turnstile>\<^sub>e e\<^sub>r" by (blast intro: maybe_static_eval_pool_to_exp_let)
+  have "(\<V>, \<C>) \<Turnstile>\<^sub>e e\<^sub>r" by (blast intro: may_be_static_eval_pool_to_exp_let)
 
   from \<open>(\<V>, \<C>) \<Turnstile>\<^sub>\<E> \<E>\<close> 
   and \<open>\<E> \<pi>\<^sub>s = Some (\<langle>LET x\<^sub>s = SYNC x\<^sub>s\<^sub>e in e\<^sub>s;\<rho>\<^sub>s;\<kappa>\<^sub>s\<rangle>)\<close> 
@@ -1214,13 +1214,13 @@ proof
   and \<open>\<rho>\<^sub>s\<^sub>e x\<^sub>m = Some \<omega>\<^sub>m\<close> \<open>\<rho>\<^sub>s\<^sub>e x\<^sub>s\<^sub>c = Some (VChan c)\<close>
   and \<open>\<E> \<pi>\<^sub>r = Some (\<langle>LET x\<^sub>r = SYNC x\<^sub>r\<^sub>e in e\<^sub>r;\<rho>\<^sub>r;\<kappa>\<^sub>r\<rangle>)\<close> 
   and \<open>\<rho>\<^sub>r x\<^sub>r\<^sub>e = Some (VClosure (Recv_Evt x\<^sub>r\<^sub>c) \<rho>\<^sub>r\<^sub>e)\<close> \<open>\<rho>\<^sub>r\<^sub>e x\<^sub>r\<^sub>c = Some (VChan c)\<close> 
-  have "(\<V>, \<C>) \<Turnstile>\<^sub>\<rho> \<rho>\<^sub>r(x\<^sub>r \<mapsto> \<omega>\<^sub>m)" by (blast intro: maybe_static_eval_pool_to_env_let_sync_recv)
+  have "(\<V>, \<C>) \<Turnstile>\<^sub>\<rho> \<rho>\<^sub>r(x\<^sub>r \<mapsto> \<omega>\<^sub>m)" by (blast intro: may_be_static_eval_pool_to_env_let_sync_recv)
 
   from \<open>(\<V>, \<C>) \<Turnstile>\<^sub>\<E> \<E>\<close> and \<open>\<E> \<pi>\<^sub>r = Some (\<langle>LET x\<^sub>r = SYNC x\<^sub>r\<^sub>e in e\<^sub>r;\<rho>\<^sub>r;\<kappa>\<^sub>r\<rangle>)\<close>
-  have  "(\<V>, \<C>) \<Turnstile>\<^sub>\<kappa> \<V> (\<lfloor>e\<^sub>r\<rfloor>) \<Rrightarrow> \<kappa>\<^sub>r" by (blast intro: maybe_static_eval_pool_to_stack_let)
+  have  "(\<V>, \<C>) \<Turnstile>\<^sub>\<kappa> \<V> (\<lfloor>e\<^sub>r\<rfloor>) \<Rrightarrow> \<kappa>\<^sub>r" by (blast intro: may_be_static_eval_pool_to_stack_let)
 
   from `(\<V>, \<C>) \<Turnstile>\<^sub>e e\<^sub>r` and `(\<V>, \<C>) \<Turnstile>\<^sub>\<rho> \<rho>\<^sub>r(x\<^sub>r \<mapsto> \<omega>\<^sub>m)` and `(\<V>, \<C>) \<Turnstile>\<^sub>\<kappa> \<V> (\<lfloor>e\<^sub>r\<rfloor>) \<Rrightarrow> \<kappa>\<^sub>r`
-  have "(\<V>, \<C>) \<Turnstile>\<^sub>\<sigma> \<langle>e\<^sub>r;\<rho>\<^sub>r(x\<^sub>r \<mapsto> \<omega>\<^sub>m);\<kappa>\<^sub>r\<rangle>" by (blast intro: maybe_static_eval_state.intros)
+  have "(\<V>, \<C>) \<Turnstile>\<^sub>\<sigma> \<langle>e\<^sub>r;\<rho>\<^sub>r(x\<^sub>r \<mapsto> \<omega>\<^sub>m);\<kappa>\<^sub>r\<rangle>" by (blast intro: may_be_static_eval_state.intros)
 
   {
     fix \<pi> \<sigma>
@@ -1228,90 +1228,90 @@ proof
     and "(\<E>(\<pi>\<^sub>s ;;(LNext x\<^sub>s) \<mapsto> \<langle>e\<^sub>s;\<rho>\<^sub>s(x\<^sub>s \<mapsto> VUnit);\<kappa>\<^sub>s\<rangle>, \<pi>\<^sub>r ;; (LNext x\<^sub>r) \<mapsto> \<langle>e\<^sub>r;\<rho>\<^sub>r(x\<^sub>r \<mapsto> \<omega>\<^sub>m);\<kappa>\<^sub>r\<rangle>)) \<pi> = Some \<sigma>" then
     have "\<E> \<pi> = Some \<sigma>" by simp
     with \<open>(\<V>, \<C>) \<Turnstile>\<^sub>\<E> \<E>\<close>
-    have "(\<V>, \<C>) \<Turnstile>\<^sub>\<sigma> \<sigma>" by (blast intro: maybe_static_eval_pool.cases)
+    have "(\<V>, \<C>) \<Turnstile>\<^sub>\<sigma> \<sigma>" by (blast intro: may_be_static_eval_pool.cases)
   } with `(\<V>, \<C>) \<Turnstile>\<^sub>\<sigma> \<langle>e\<^sub>r;\<rho>\<^sub>r (x\<^sub>r \<mapsto> \<omega>\<^sub>m);\<kappa>\<^sub>r\<rangle>` `(\<V>, \<C>) \<Turnstile>\<^sub>\<sigma> \<langle>e\<^sub>s;\<rho>\<^sub>s (x\<^sub>s \<mapsto> VUnit);\<kappa>\<^sub>s\<rangle>`
   show "\<forall>\<pi> \<sigma>. (\<E>(\<pi>\<^sub>s ;; (LNext x\<^sub>s) \<mapsto> \<langle>e\<^sub>s;\<rho>\<^sub>s(x\<^sub>s \<mapsto> VUnit);\<kappa>\<^sub>s\<rangle>, \<pi>\<^sub>r ;;(LNext x\<^sub>r) \<mapsto> \<langle>e\<^sub>r;\<rho>\<^sub>r(x\<^sub>r \<mapsto> \<omega>\<^sub>m);\<kappa>\<^sub>r\<rangle>)) \<pi> = Some \<sigma> \<longrightarrow> (\<V>, \<C>) \<Turnstile>\<^sub>\<sigma> \<sigma>" by simp
 
 qed
 
 
-lemma maybe_static_eval_pool_to_env_let_chan: "
+lemma may_be_static_eval_pool_to_env_let_chan: "
   (\<V>, \<C>) \<Turnstile>\<^sub>\<E> \<E> \<Longrightarrow>
   \<E> \<pi> = Some (\<langle>LET x = CHAN \<lparr>\<rparr> in e; \<rho>; \<kappa>\<rangle>) \<Longrightarrow> 
   (\<V>, \<C>) \<Turnstile>\<^sub>\<rho> \<rho>(x \<mapsto> (VChan (Ch \<pi> x)))
 "
 proof
   assume "(\<V>, \<C>) \<Turnstile>\<^sub>\<E> \<E>" and "\<E> \<pi> = Some (\<langle>LET x = CHAN \<lparr>\<rparr> in e; \<rho>; \<kappa>\<rangle>)" then
-  have "(\<V>, \<C>) \<Turnstile>\<^sub>\<sigma> \<langle>LET x = CHAN \<lparr>\<rparr> in e; \<rho>; \<kappa>\<rangle>" by (blast intro: maybe_static_eval_pool.cases) then
-  have "(\<V>, \<C>) \<Turnstile>\<^sub>e LET x = CHAN \<lparr>\<rparr> in e" by (blast intro: maybe_static_eval_state.cases) then
-  have "{^Chan x} \<subseteq> \<V> x"  by (blast intro: maybe_static_eval.cases)
+  have "(\<V>, \<C>) \<Turnstile>\<^sub>\<sigma> \<langle>LET x = CHAN \<lparr>\<rparr> in e; \<rho>; \<kappa>\<rangle>" by (blast intro: may_be_static_eval_pool.cases) then
+  have "(\<V>, \<C>) \<Turnstile>\<^sub>e LET x = CHAN \<lparr>\<rparr> in e" by (blast intro: may_be_static_eval_state.cases) then
+  have "{^Chan x} \<subseteq> \<V> x"  by (blast intro: may_be_static_eval.cases)
   have "(\<V>, \<C>) \<Turnstile>\<^sub>\<omega> (VChan (Ch \<pi> x))" by (simp add: Chan)
 
   from `(\<V>, \<C>) \<Turnstile>\<^sub>\<sigma> \<langle>LET x = CHAN \<lparr>\<rparr> in e; \<rho>; \<kappa>\<rangle>` 
-  have "(\<V>, \<C>) \<Turnstile>\<^sub>\<rho> \<rho>" by (simp add: maybe_static_eval_state.simps)+
+  have "(\<V>, \<C>) \<Turnstile>\<^sub>\<rho> \<rho>" by (simp add: may_be_static_eval_state.simps)+
   {
     fix x' \<omega>'
     assume "(\<rho>(x \<mapsto> (VChan (Ch \<pi> x)))) x' = Some \<omega>'" and "x \<noteq> x'"then
     have "\<rho> x' = Some \<omega>'" by simp with `(\<V>, \<C>) \<Turnstile>\<^sub>\<rho> \<rho>`
-    have "{|\<omega>'|} \<subseteq> \<V> x' \<and> (\<V>, \<C>) \<Turnstile>\<^sub>\<omega> \<omega>'" by (simp add: maybe_static_eval_env.simps)
+    have "{|\<omega>'|} \<subseteq> \<V> x' \<and> (\<V>, \<C>) \<Turnstile>\<^sub>\<omega> \<omega>'" by (simp add: may_be_static_eval_env.simps)
   } with `{^Chan x} \<subseteq> \<V> x` and `(\<V>, \<C>) \<Turnstile>\<^sub>\<omega> (VChan (Ch \<pi> x))`
   show "\<forall>x' \<omega>'. (\<rho>(x \<mapsto> (VChan (Ch \<pi> x)))) x' = Some \<omega>' \<longrightarrow> {|\<omega>'|} \<subseteq> \<V> x' \<and> (\<V>, \<C>) \<Turnstile>\<^sub>\<omega> \<omega>'" by simp
 qed
 
 
-lemma maybe_static_eval_preserved_under_chan: "
+lemma may_be_static_eval_preserved_under_chan: "
   (\<V>, \<C>) \<Turnstile>\<^sub>\<E> \<E> \<Longrightarrow>
   \<E> \<pi> = Some (\<langle>LET x = CHAN \<lparr>\<rparr> in e; \<rho>; \<kappa>\<rangle>) \<Longrightarrow> 
   (\<V>, \<C>) \<Turnstile>\<^sub>\<E> \<E>(\<pi> ;;(LNext x) \<mapsto> \<langle>e; \<rho>(x \<mapsto> (VChan (Ch \<pi> x))); \<kappa>\<rangle>)
 "
 proof
   assume "(\<V>, \<C>) \<Turnstile>\<^sub>\<E> \<E>" and "\<E> \<pi> = Some (\<langle>LET x = CHAN \<lparr>\<rparr> in e; \<rho>; \<kappa>\<rangle>)" then
-  have "(\<V>, \<C>) \<Turnstile>\<^sub>e e" by (blast intro: maybe_static_eval_pool_to_exp_let)
+  have "(\<V>, \<C>) \<Turnstile>\<^sub>e e" by (blast intro: may_be_static_eval_pool_to_exp_let)
 
   from `(\<V>, \<C>) \<Turnstile>\<^sub>\<E> \<E>` and `\<E> \<pi> = Some (\<langle>LET x = CHAN \<lparr>\<rparr> in e; \<rho>; \<kappa>\<rangle>)`
-  have "(\<V>, \<C>) \<Turnstile>\<^sub>\<rho> \<rho>(x \<mapsto> (VChan (Ch \<pi> x)))" by (blast intro: maybe_static_eval_pool_to_env_let_chan )
+  have "(\<V>, \<C>) \<Turnstile>\<^sub>\<rho> \<rho>(x \<mapsto> (VChan (Ch \<pi> x)))" by (blast intro: may_be_static_eval_pool_to_env_let_chan )
 
   from `(\<V>, \<C>) \<Turnstile>\<^sub>\<E> \<E>` and `\<E> \<pi> = Some (\<langle>LET x = CHAN \<lparr>\<rparr> in e; \<rho>; \<kappa>\<rangle>)`
-  have "(\<V>, \<C>) \<Turnstile>\<^sub>\<kappa> \<V> (\<lfloor>e\<rfloor>) \<Rrightarrow> \<kappa>" by (blast intro: maybe_static_eval_pool_to_stack_let)
+  have "(\<V>, \<C>) \<Turnstile>\<^sub>\<kappa> \<V> (\<lfloor>e\<rfloor>) \<Rrightarrow> \<kappa>" by (blast intro: may_be_static_eval_pool_to_stack_let)
 
   from `(\<V>, \<C>) \<Turnstile>\<^sub>e e` and `(\<V>, \<C>) \<Turnstile>\<^sub>\<rho> \<rho>(x \<mapsto> (VChan (Ch \<pi> x)))` and `(\<V>, \<C>) \<Turnstile>\<^sub>\<kappa> \<V> (\<lfloor>e\<rfloor>) \<Rrightarrow> \<kappa>`
-  have "(\<V>, \<C>) \<Turnstile>\<^sub>\<sigma> \<langle>e;\<rho>(x \<mapsto> (VChan (Ch \<pi> x)));\<kappa>\<rangle>" by (blast intro: maybe_static_eval_state.intros)
+  have "(\<V>, \<C>) \<Turnstile>\<^sub>\<sigma> \<langle>e;\<rho>(x \<mapsto> (VChan (Ch \<pi> x)));\<kappa>\<rangle>" by (blast intro: may_be_static_eval_state.intros)
   {
     fix \<pi>' \<sigma>'
     assume "(\<E>(\<pi> ;;(LNext x) \<mapsto> \<langle>e;\<rho>(x \<mapsto> (VChan (Ch \<pi> x)));\<kappa>\<rangle>)) \<pi>' = Some \<sigma>'" 
     and "\<pi>' \<noteq> \<pi> ;;(LNext x)" then
     have "\<E> \<pi>' = Some \<sigma>'" by simp with `(\<V>, \<C>) \<Turnstile>\<^sub>\<E> \<E>`
-    have "(\<V>, \<C>) \<Turnstile>\<^sub>\<sigma> \<sigma>'" by (simp add: maybe_static_eval_pool.simps)
+    have "(\<V>, \<C>) \<Turnstile>\<^sub>\<sigma> \<sigma>'" by (simp add: may_be_static_eval_pool.simps)
   } with `(\<V>, \<C>) \<Turnstile>\<^sub>\<sigma> \<langle>e;\<rho>(x \<mapsto> (VChan (Ch \<pi> x)));\<kappa>\<rangle>`
   show "\<forall>\<pi>' \<sigma>'. (\<E>(\<pi> ;;(LNext x) \<mapsto> \<langle>e;\<rho>(x \<mapsto> (VChan (Ch \<pi> x)));\<kappa>\<rangle>)) \<pi>' = Some \<sigma>' \<longrightarrow> (\<V>, \<C>) \<Turnstile>\<^sub>\<sigma> \<sigma>'" by simp
 qed
 
 
-lemma maybe_static_eval_pool_to_env_let_spawn: "
+lemma may_be_static_eval_pool_to_env_let_spawn: "
   (\<V>, \<C>) \<Turnstile>\<^sub>\<E> \<E> \<Longrightarrow>
   \<E> \<pi> = Some (\<langle>LET x = SPAWN e\<^sub>c in e; \<rho>; \<kappa>\<rangle>) \<Longrightarrow> 
   (\<V>, \<C>) \<Turnstile>\<^sub>\<rho> \<rho>(x \<mapsto> VUnit)"
 proof
 
   assume "(\<V>, \<C>) \<Turnstile>\<^sub>\<E> \<E>" and "\<E> \<pi> = Some (\<langle>LET x = SPAWN e\<^sub>c in e; \<rho>; \<kappa>\<rangle>)" then
-  have "(\<V>, \<C>) \<Turnstile>\<^sub>\<sigma> \<langle>LET x = SPAWN e\<^sub>c in e; \<rho>; \<kappa>\<rangle>" by (simp add: maybe_static_eval_pool.simps) then
-  have "(\<V>, \<C>) \<Turnstile>\<^sub>e LET x = SPAWN e\<^sub>c in e" by (blast intro: maybe_static_eval_state.cases) then
-  have "{^\<lparr>\<rparr>} \<subseteq> \<V> x"  by (blast intro: maybe_static_eval.cases) then
+  have "(\<V>, \<C>) \<Turnstile>\<^sub>\<sigma> \<langle>LET x = SPAWN e\<^sub>c in e; \<rho>; \<kappa>\<rangle>" by (simp add: may_be_static_eval_pool.simps) then
+  have "(\<V>, \<C>) \<Turnstile>\<^sub>e LET x = SPAWN e\<^sub>c in e" by (blast intro: may_be_static_eval_state.cases) then
+  have "{^\<lparr>\<rparr>} \<subseteq> \<V> x"  by (blast intro: may_be_static_eval.cases) then
   have "(\<V>, \<C>) \<Turnstile>\<^sub>\<omega> VUnit" by (simp add: Unit)
 
   from `(\<V>, \<C>) \<Turnstile>\<^sub>\<sigma> \<langle>LET x = SPAWN e\<^sub>c in e; \<rho>; \<kappa>\<rangle>` 
-  have "(\<V>, \<C>) \<Turnstile>\<^sub>\<rho> \<rho>" by (simp add: maybe_static_eval_state.simps)
+  have "(\<V>, \<C>) \<Turnstile>\<^sub>\<rho> \<rho>" by (simp add: may_be_static_eval_state.simps)
 
   {
     fix x' \<omega>'
     assume "(\<rho>(x \<mapsto> VUnit)) x' = Some \<omega>'" and "x \<noteq> x'" then
     have "\<rho> x' = Some \<omega>'" by simp with `(\<V>, \<C>) \<Turnstile>\<^sub>\<rho> \<rho>`
-    have "{|\<omega>'|} \<subseteq> \<V> x' \<and> (\<V>, \<C>) \<Turnstile>\<^sub>\<omega> \<omega>'" by (blast intro: maybe_static_eval_env.cases)
+    have "{|\<omega>'|} \<subseteq> \<V> x' \<and> (\<V>, \<C>) \<Turnstile>\<^sub>\<omega> \<omega>'" by (blast intro: may_be_static_eval_env.cases)
   } with `{^\<lparr>\<rparr>} \<subseteq> \<V> x` and `(\<V>, \<C>) \<Turnstile>\<^sub>\<omega> VUnit`
   show "\<forall>x' \<omega>'. (\<rho>(x \<mapsto> VUnit)) x' = Some \<omega>' \<longrightarrow> {|\<omega>'|} \<subseteq> \<V> x' \<and> (\<V>, \<C>) \<Turnstile>\<^sub>\<omega> \<omega>'" by simp
 qed
 
-lemma maybe_static_eval_preserved_under_spawn: "
+lemma may_be_static_eval_preserved_under_spawn: "
   (\<V>, \<C>) \<Turnstile>\<^sub>\<E> \<E> \<Longrightarrow>
   \<E> \<pi> = Some (\<langle>LET x = SPAWN e\<^sub>c in e; \<rho>; \<kappa>\<rangle>) \<Longrightarrow> 
   (\<V>, \<C>) \<Turnstile>\<^sub>\<E> \<E>(\<pi> ;;(LNext x) \<mapsto> \<langle>e; \<rho>(x \<mapsto> VUnit); \<kappa>\<rangle>, \<pi>;;(LSpawn x) \<mapsto> \<langle>e\<^sub>c; \<rho>; []\<rangle>)
@@ -1321,40 +1321,40 @@ proof
   assume "(\<V>, \<C>) \<Turnstile>\<^sub>\<E> \<E>" and "\<E> \<pi> = Some (\<langle>LET x = SPAWN e\<^sub>c in e; \<rho>; \<kappa>\<rangle>)"
 
   from `(\<V>, \<C>) \<Turnstile>\<^sub>\<E> \<E>` and `\<E> \<pi> = Some (\<langle>LET x = SPAWN e\<^sub>c in e; \<rho>; \<kappa>\<rangle>)`
-  have "(\<V>, \<C>) \<Turnstile>\<^sub>e e" by (blast intro: maybe_static_eval_pool_to_exp_let)
+  have "(\<V>, \<C>) \<Turnstile>\<^sub>e e" by (blast intro: may_be_static_eval_pool_to_exp_let)
 
   from `(\<V>, \<C>) \<Turnstile>\<^sub>\<E> \<E>` and `\<E> \<pi> = Some (\<langle>LET x = SPAWN e\<^sub>c in e; \<rho>; \<kappa>\<rangle>)`
-  have "(\<V>, \<C>) \<Turnstile>\<^sub>\<rho> \<rho>(x \<mapsto> VUnit)" by (blast intro: maybe_static_eval_pool_to_env_let_spawn)
+  have "(\<V>, \<C>) \<Turnstile>\<^sub>\<rho> \<rho>(x \<mapsto> VUnit)" by (blast intro: may_be_static_eval_pool_to_env_let_spawn)
 
   from `(\<V>, \<C>) \<Turnstile>\<^sub>\<E> \<E>` and `\<E> \<pi> = Some (\<langle>LET x = SPAWN e\<^sub>c in e; \<rho>; \<kappa>\<rangle>)`
-  have "(\<V>, \<C>) \<Turnstile>\<^sub>\<kappa> \<V> (\<lfloor>e\<rfloor>) \<Rrightarrow> \<kappa>" by (blast intro: maybe_static_eval_pool_to_stack_let)
+  have "(\<V>, \<C>) \<Turnstile>\<^sub>\<kappa> \<V> (\<lfloor>e\<rfloor>) \<Rrightarrow> \<kappa>" by (blast intro: may_be_static_eval_pool_to_stack_let)
 
   from \<open>(\<V>, \<C>) \<Turnstile>\<^sub>\<kappa> \<V> (\<lfloor>e\<rfloor>) \<Rrightarrow> \<kappa>\<close> \<open>(\<V>, \<C>) \<Turnstile>\<^sub>\<rho> \<rho>(x \<mapsto> VUnit)\<close> \<open>(\<V>, \<C>) \<Turnstile>\<^sub>e e\<close>
-  have "(\<V>, \<C>) \<Turnstile>\<^sub>\<sigma> \<langle>e;\<rho>(x \<mapsto> VUnit);\<kappa>\<rangle>" by (simp add: maybe_static_eval_state.intros)
+  have "(\<V>, \<C>) \<Turnstile>\<^sub>\<sigma> \<langle>e;\<rho>(x \<mapsto> VUnit);\<kappa>\<rangle>" by (simp add: may_be_static_eval_state.intros)
 
   from `(\<V>, \<C>) \<Turnstile>\<^sub>\<E> \<E>` and `\<E> \<pi> = Some (\<langle>LET x = SPAWN e\<^sub>c in e; \<rho>; \<kappa>\<rangle>)`
-  have "(\<V>, \<C>) \<Turnstile>\<^sub>\<sigma> \<langle>LET x = SPAWN e\<^sub>c in e; \<rho>; \<kappa>\<rangle>" by (simp add: maybe_static_eval_pool.simps) then
-  have "(\<V>, \<C>) \<Turnstile>\<^sub>e LET x = SPAWN e\<^sub>c in e" and "(\<V>, \<C>) \<Turnstile>\<^sub>\<rho> \<rho>" by (simp add: maybe_static_eval_state.simps)+
+  have "(\<V>, \<C>) \<Turnstile>\<^sub>\<sigma> \<langle>LET x = SPAWN e\<^sub>c in e; \<rho>; \<kappa>\<rangle>" by (simp add: may_be_static_eval_pool.simps) then
+  have "(\<V>, \<C>) \<Turnstile>\<^sub>e LET x = SPAWN e\<^sub>c in e" and "(\<V>, \<C>) \<Turnstile>\<^sub>\<rho> \<rho>" by (simp add: may_be_static_eval_state.simps)+
   
   from `(\<V>, \<C>) \<Turnstile>\<^sub>e LET x = SPAWN e\<^sub>c in e`
-  have "(\<V>, \<C>) \<Turnstile>\<^sub>e e\<^sub>c" by (blast intro: maybe_static_eval.cases)
+  have "(\<V>, \<C>) \<Turnstile>\<^sub>e e\<^sub>c" by (blast intro: may_be_static_eval.cases)
 
-  have "(\<V>, \<C>) \<Turnstile>\<^sub>\<kappa> \<V> (\<lfloor>e\<^sub>c\<rfloor>) \<Rrightarrow> []" by (simp add: maybe_static_eval_stack.Empty)
+  have "(\<V>, \<C>) \<Turnstile>\<^sub>\<kappa> \<V> (\<lfloor>e\<^sub>c\<rfloor>) \<Rrightarrow> []" by (simp add: may_be_static_eval_stack.Empty)
   from \<open>(\<V>, \<C>) \<Turnstile>\<^sub>\<kappa> \<V> (\<lfloor>e\<^sub>c\<rfloor>) \<Rrightarrow> []\<close> \<open>(\<V>, \<C>) \<Turnstile>\<^sub>\<rho> \<rho>\<close> \<open>(\<V>, \<C>) \<Turnstile>\<^sub>e e\<^sub>c\<close> 
-  have "(\<V>, \<C>) \<Turnstile>\<^sub>\<sigma> \<langle>e\<^sub>c;\<rho>;[]\<rangle>" by (simp add: maybe_static_eval_state.intros)
+  have "(\<V>, \<C>) \<Turnstile>\<^sub>\<sigma> \<langle>e\<^sub>c;\<rho>;[]\<rangle>" by (simp add: may_be_static_eval_state.intros)
 
   {
     fix \<pi>' \<sigma>'
     assume "(\<E>(\<pi> ;;(LNext x) \<mapsto> \<langle>e;\<rho>(x \<mapsto> VUnit);\<kappa>\<rangle>, \<pi> ;; (LSpawn x) \<mapsto> \<langle>e\<^sub>c;\<rho>;[]\<rangle>)) \<pi>' = Some \<sigma>'"
     and "\<pi>' \<noteq> \<pi> ;; (LNext x)" and " \<pi>' \<noteq> \<pi> ;; (LSpawn x)" then
     have "\<E> \<pi>' = Some \<sigma>'" by simp with `(\<V>, \<C>) \<Turnstile>\<^sub>\<E> \<E>`
-    have "(\<V>, \<C>) \<Turnstile>\<^sub>\<sigma> \<sigma>'" by (blast intro: maybe_static_eval_pool.cases)
+    have "(\<V>, \<C>) \<Turnstile>\<^sub>\<sigma> \<sigma>'" by (blast intro: may_be_static_eval_pool.cases)
   } with `(\<V>, \<C>) \<Turnstile>\<^sub>\<sigma> \<langle>e;\<rho>(x \<mapsto> VUnit);\<kappa>\<rangle>` and `(\<V>, \<C>) \<Turnstile>\<^sub>\<sigma> \<langle>e\<^sub>c;\<rho>;[]\<rangle>`
   show "\<forall>\<pi>' \<sigma>'. (\<E>(\<pi> ;; (LNext x) \<mapsto> \<langle>e;\<rho>(x \<mapsto> VUnit);\<kappa>\<rangle>, \<pi> ;; (LSpawn x) \<mapsto> \<langle>e\<^sub>c;\<rho>;[]\<rangle>)) \<pi>' = Some \<sigma>' \<longrightarrow> (\<V>, \<C>) \<Turnstile>\<^sub>\<sigma> \<sigma>'" by simp
 qed
 
 
-theorem maybe_static_eval_preserved_under_concur_step : "
+theorem may_be_static_eval_preserved_under_concur_step : "
   \<lbrakk>
     (\<V>, \<C>) \<Turnstile>\<^sub>\<E> \<E>; 
     \<E> \<rightarrow> \<E>'
@@ -1371,7 +1371,7 @@ proof -
     assume "leaf \<E> \<pi>" and "\<E> \<pi> = Some (\<langle>RESULT x;\<rho>;\<langle>x\<^sub>\<kappa>,e\<^sub>\<kappa>,\<rho>\<^sub>\<kappa>\<rangle> # \<kappa>\<rangle>)"
     and "\<langle>RESULT x;\<rho>;\<langle>x\<^sub>\<kappa>,e\<^sub>\<kappa>,\<rho>\<^sub>\<kappa>\<rangle> # \<kappa>\<rangle> \<hookrightarrow> \<sigma>'"
     with \<open>(\<V>, \<C>) \<Turnstile>\<^sub>\<E> \<E>\<close>
-    have "(\<V>, \<C>) \<Turnstile>\<^sub>\<E> \<E>(\<pi> ;; (LReturn x\<^sub>\<kappa>) \<mapsto> \<sigma>')" by (simp add:  maybe_static_eval_preserved_under_seq_step_down)
+    have "(\<V>, \<C>) \<Turnstile>\<^sub>\<E> \<E>(\<pi> ;; (LReturn x\<^sub>\<kappa>) \<mapsto> \<sigma>')" by (simp add:  may_be_static_eval_preserved_under_seq_step_down)
     with `\<E>' = \<E> ++ [\<pi> ;; (LReturn x\<^sub>\<kappa>) \<mapsto> \<sigma>']`
     show "(\<V>, \<C>) \<Turnstile>\<^sub>\<E> \<E>'" by simp
   next
@@ -1380,7 +1380,7 @@ proof -
     assume "leaf \<E> \<pi>" and "\<E> \<pi> = Some (\<langle>LET x = b in e;\<rho>;\<kappa>\<rangle>)"
     and "\<langle>LET x = b in e;\<rho>;\<kappa>\<rangle> \<hookrightarrow> \<langle>e';\<rho>';\<kappa>\<rangle>"
     with \<open>(\<V>, \<C>) \<Turnstile>\<^sub>\<E> \<E>\<close>
-    have "(\<V>, \<C>) \<Turnstile>\<^sub>\<E> \<E>(\<pi> ;; (LNext x) \<mapsto> \<langle>e';\<rho>';\<kappa>\<rangle>)" by (simp add: maybe_static_eval_preserved_under_seq_step)
+    have "(\<V>, \<C>) \<Turnstile>\<^sub>\<E> \<E>(\<pi> ;; (LNext x) \<mapsto> \<langle>e';\<rho>';\<kappa>\<rangle>)" by (simp add: may_be_static_eval_preserved_under_seq_step)
     with \<open>\<E>' = \<E> ++ [\<pi> ;; (LNext x) \<mapsto> \<langle>e';\<rho>';\<kappa>\<rangle>]\<close>
     show "(\<V>, \<C>) \<Turnstile>\<^sub>\<E> \<E>'" by simp
   next
@@ -1389,7 +1389,7 @@ proof -
     assume "leaf \<E> \<pi>" and "\<E> \<pi> = Some (\<langle>LET x = b in e;\<rho>;\<kappa>\<rangle>)"
     and "\<langle>LET x = b in e;\<rho>;\<kappa>\<rangle> \<hookrightarrow> \<langle>e';\<rho>';\<langle>x,e,\<rho>\<rangle> # \<kappa>\<rangle>"
     with \<open>(\<V>, \<C>) \<Turnstile>\<^sub>\<E> \<E>\<close>
-    have "(\<V>, \<C>) \<Turnstile>\<^sub>\<E> \<E>(\<pi> ;; (LCall) x \<mapsto> \<langle>e';\<rho>';\<langle>x,e,\<rho>\<rangle> # \<kappa>\<rangle>)" by (simp add: maybe_static_eval_preserved_under_seq_step_up)
+    have "(\<V>, \<C>) \<Turnstile>\<^sub>\<E> \<E>(\<pi> ;; (LCall) x \<mapsto> \<langle>e';\<rho>';\<langle>x,e,\<rho>\<rangle> # \<kappa>\<rangle>)" by (simp add: may_be_static_eval_preserved_under_seq_step_up)
     with \<open>\<E>' = \<E> ++ [\<pi> ;; (LCall x) \<mapsto> \<langle>e';\<rho>';\<langle>x,e,\<rho>\<rangle> # \<kappa>\<rangle>]\<close>
     show "(\<V>, \<C>) \<Turnstile>\<^sub>\<E> \<E>'" by simp
   next
@@ -1397,7 +1397,7 @@ proof -
     assume "\<E>' = \<E> ++ [\<pi> ;; (LNext x) \<mapsto> \<langle>e;\<rho> ++ [x \<mapsto> (VChan (Ch \<pi> x))];\<kappa>\<rangle>]"
     assume "leaf \<E> \<pi>" and "\<E> \<pi> = Some (\<langle>LET x = CHAN \<lparr>\<rparr> in e;\<rho>;\<kappa>\<rangle>)"
     with \<open>(\<V>, \<C>) \<Turnstile>\<^sub>\<E> \<E>\<close>
-    have "(\<V>, \<C>) \<Turnstile>\<^sub>\<E> \<E>(\<pi> ;; (LNext x) \<mapsto> \<langle>e;\<rho> ++ [x \<mapsto> (VChan (Ch \<pi> x))];\<kappa>\<rangle>)" by (simp add: maybe_static_eval_preserved_under_chan)
+    have "(\<V>, \<C>) \<Turnstile>\<^sub>\<E> \<E>(\<pi> ;; (LNext x) \<mapsto> \<langle>e;\<rho> ++ [x \<mapsto> (VChan (Ch \<pi> x))];\<kappa>\<rangle>)" by (simp add: may_be_static_eval_preserved_under_chan)
     with \<open>\<E>' = \<E> ++ [\<pi> ;; (LNext x) \<mapsto> \<langle>e;\<rho> ++ [x \<mapsto> (VChan (Ch \<pi> x))];\<kappa>\<rangle>]\<close>
     show "(\<V>, \<C>) \<Turnstile>\<^sub>\<E> \<E>'" by simp
   next
@@ -1405,7 +1405,7 @@ proof -
     assume "\<E>' = \<E> ++ [\<pi> ;; (LNext x) \<mapsto> \<langle>e;\<rho> ++ [x \<mapsto> VUnit];\<kappa>\<rangle>, \<pi> ;; (LSpawn x) \<mapsto> \<langle>e\<^sub>c;\<rho>;[]\<rangle>]"
     assume "leaf \<E> \<pi>" and "\<E> \<pi> = Some (\<langle>LET x = SPAWN e\<^sub>c in e;\<rho>;\<kappa>\<rangle>)"
     with \<open>(\<V>, \<C>) \<Turnstile>\<^sub>\<E> \<E>\<close>
-    have "(\<V>, \<C>) \<Turnstile>\<^sub>\<E> \<E>(\<pi> ;; (LNext x) \<mapsto> \<langle>e;\<rho> ++ [x \<mapsto> VUnit];\<kappa>\<rangle>, \<pi> ;; (LSpawn x) \<mapsto> \<langle>e\<^sub>c;\<rho>;[]\<rangle>)" by (simp add: maybe_static_eval_preserved_under_spawn)
+    have "(\<V>, \<C>) \<Turnstile>\<^sub>\<E> \<E>(\<pi> ;; (LNext x) \<mapsto> \<langle>e;\<rho> ++ [x \<mapsto> VUnit];\<kappa>\<rangle>, \<pi> ;; (LSpawn x) \<mapsto> \<langle>e\<^sub>c;\<rho>;[]\<rangle>)" by (simp add: may_be_static_eval_preserved_under_spawn)
     with \<open>\<E>' = \<E> ++ [\<pi> ;; (LNext x) \<mapsto> \<langle>e;\<rho> ++ [x \<mapsto> VUnit];\<kappa>\<rangle>, \<pi> ;; (LSpawn x) \<mapsto> \<langle>e\<^sub>c;\<rho>;[]\<rangle>]\<close>
     show "(\<V>, \<C>) \<Turnstile>\<^sub>\<E> \<E>'" by simp
   next
@@ -1422,14 +1422,14 @@ proof -
     and "\<rho>\<^sub>r\<^sub>e x\<^sub>r\<^sub>c = Some (VChan c)"
     and "\<rho>\<^sub>s\<^sub>e x\<^sub>m = Some \<omega>\<^sub>m"
     with \<open>(\<V>, \<C>) \<Turnstile>\<^sub>\<E> \<E>\<close>
-    have "(\<V>, \<C>) \<Turnstile>\<^sub>\<E> \<E>(\<pi>\<^sub>s ;; (LNext x\<^sub>s) \<mapsto> \<langle>e\<^sub>s;\<rho>\<^sub>s ++ [x\<^sub>s \<mapsto> VUnit];\<kappa>\<^sub>s\<rangle>, \<pi>\<^sub>r ;; (LNext x\<^sub>r) \<mapsto> \<langle>e\<^sub>r;\<rho>\<^sub>r ++ [x\<^sub>r \<mapsto> \<omega>\<^sub>m];\<kappa>\<^sub>r\<rangle>)" by (simp add: maybe_static_eval_preserved_under_sync)
+    have "(\<V>, \<C>) \<Turnstile>\<^sub>\<E> \<E>(\<pi>\<^sub>s ;; (LNext x\<^sub>s) \<mapsto> \<langle>e\<^sub>s;\<rho>\<^sub>s ++ [x\<^sub>s \<mapsto> VUnit];\<kappa>\<^sub>s\<rangle>, \<pi>\<^sub>r ;; (LNext x\<^sub>r) \<mapsto> \<langle>e\<^sub>r;\<rho>\<^sub>r ++ [x\<^sub>r \<mapsto> \<omega>\<^sub>m];\<kappa>\<^sub>r\<rangle>)" by (simp add: may_be_static_eval_preserved_under_sync)
     with \<open>\<E>' = \<E> ++ [\<pi>\<^sub>s ;; (LNext x\<^sub>s) \<mapsto> \<langle>e\<^sub>s;\<rho>\<^sub>s ++ [x\<^sub>s \<mapsto> VUnit];\<kappa>\<^sub>s\<rangle>, \<pi>\<^sub>r ;; (LNext x\<^sub>r) \<mapsto> \<langle>e\<^sub>r;\<rho>\<^sub>r ++ [x\<^sub>r \<mapsto> \<omega>\<^sub>m];\<kappa>\<^sub>r\<rangle>]\<close>
     show "(\<V>, \<C>) \<Turnstile>\<^sub>\<E> \<E>'" by simp
   qed
 qed
 
 
-theorem maybe_static_eval_preserved_under_concur_step_star : "
+theorem may_be_static_eval_preserved_under_concur_step_star : "
   \<lbrakk>
     (\<V>, \<C>) \<Turnstile>\<^sub>\<E> \<E>;  
     \<E> \<rightarrow>* \<E>'
@@ -1447,22 +1447,22 @@ proof -
     case (step \<E> \<E>\<^sub>m \<E>')
     assume " \<E> \<rightarrow> \<E>\<^sub>m"
     and "(\<V>, \<C>) \<Turnstile>\<^sub>\<E> \<E>\<^sub>m \<longrightarrow> (\<V>, \<C>) \<Turnstile>\<^sub>\<E> \<E>'" then
-    show "(\<V>, \<C>) \<Turnstile>\<^sub>\<E> \<E> \<longrightarrow> (\<V>, \<C>) \<Turnstile>\<^sub>\<E> \<E>'" by (blast intro: maybe_static_eval_preserved_under_concur_step)
+    show "(\<V>, \<C>) \<Turnstile>\<^sub>\<E> \<E> \<longrightarrow> (\<V>, \<C>) \<Turnstile>\<^sub>\<E> \<E>'" by (blast intro: may_be_static_eval_preserved_under_concur_step)
   qed with `(\<V>, \<C>) \<Turnstile>\<^sub>\<E> \<E>`
   show "(\<V>, \<C>) \<Turnstile>\<^sub>\<E> \<E>'" by blast
 qed
 
-theorem maybe_static_eval_env_to_precise : "
+theorem may_be_static_eval_env_to_precise : "
   \<rho> x = Some \<omega> \<Longrightarrow>
   (\<V>, \<C>) \<Turnstile>\<^sub>\<rho> \<rho> \<Longrightarrow>
   {|\<omega>|} \<subseteq> \<V> x
 "
 proof -
   assume "\<rho> x = Some \<omega>" and "(\<V>, \<C>) \<Turnstile>\<^sub>\<rho> \<rho>" then
-  show "{|\<omega>|} \<subseteq> \<V> x" by (simp add: maybe_static_eval_env.simps)
+  show "{|\<omega>|} \<subseteq> \<V> x" by (simp add: may_be_static_eval_env.simps)
 qed
 
-theorem maybe_static_eval_pool_to_precise : "
+theorem may_be_static_eval_pool_to_precise : "
   \<rho> x = Some \<omega> \<Longrightarrow>
   \<E> \<pi> = Some (\<langle>e; \<rho>; \<kappa>\<rangle>) \<Longrightarrow>
   (\<V>, \<C>) \<Turnstile>\<^sub>\<E> \<E> \<Longrightarrow>
@@ -1473,12 +1473,12 @@ proof -
 
   assume "(\<V>, \<C>) \<Turnstile>\<^sub>\<E> \<E>" and "\<E> \<pi> = Some (\<langle>e; \<rho>; \<kappa>\<rangle>)" then
 
-  have "(\<V>, \<C>) \<Turnstile>\<^sub>\<sigma> \<langle>e; \<rho>; \<kappa>\<rangle>" by (simp add: maybe_static_eval_pool.simps) then
+  have "(\<V>, \<C>) \<Turnstile>\<^sub>\<sigma> \<langle>e; \<rho>; \<kappa>\<rangle>" by (simp add: may_be_static_eval_pool.simps) then
 
-  have "(\<V>, \<C>) \<Turnstile>\<^sub>\<rho> \<rho>" by (simp add: maybe_static_eval_state.simps) 
+  have "(\<V>, \<C>) \<Turnstile>\<^sub>\<rho> \<rho>" by (simp add: may_be_static_eval_state.simps) 
   with `\<rho> x = Some \<omega>`
 
-  show "{|\<omega>|} \<subseteq> \<V> x" by (simp add: maybe_static_eval_env.simps)
+  show "{|\<omega>|} \<subseteq> \<V> x" by (simp add: may_be_static_eval_env.simps)
 qed
 
 theorem values_not_bound_pool_sound : "
@@ -1491,13 +1491,13 @@ theorem values_not_bound_pool_sound : "
 proof -
   assume "\<rho>' x = Some \<omega>"
   assume "(\<V>, \<C>) \<Turnstile>\<^sub>\<E> \<E>" and "\<E> \<rightarrow>* \<E>'" and "\<E>' \<pi> = Some (\<langle>e'; \<rho>'; \<kappa>'\<rangle>)" then
-  have "(\<V>, \<C>) \<Turnstile>\<^sub>\<E> \<E>'" by (blast intro: maybe_static_eval_preserved_under_concur_step_star)
+  have "(\<V>, \<C>) \<Turnstile>\<^sub>\<E> \<E>'" by (blast intro: may_be_static_eval_preserved_under_concur_step_star)
   with \<open>\<E>' \<pi> = Some (\<langle>e';\<rho>';\<kappa>'\<rangle>)\<close> and `\<rho>' x = Some \<omega>`
-  show "{|\<omega>|} \<subseteq> \<V> x" using maybe_static_eval_pool_to_precise by auto
+  show "{|\<omega>|} \<subseteq> \<V> x" using may_be_static_eval_pool_to_precise by auto
 qed
 
 
-lemma maybe_static_eval_to_pool: "
+lemma may_be_static_eval_to_pool: "
   \<lbrakk>
     (\<V>, \<C>) \<Turnstile>\<^sub>e e
   \<rbrakk> \<Longrightarrow>
@@ -1506,15 +1506,15 @@ lemma maybe_static_eval_to_pool: "
 proof -
   assume "(\<V>, \<C>) \<Turnstile>\<^sub>e e"
 
-  have "(\<V>, \<C>) \<Turnstile>\<^sub>\<rho> empty" by (simp add: maybe_static_eval_value_maybe_static_eval_env.Any)
-  have "(\<V>, \<C>) \<Turnstile>\<^sub>\<kappa> \<V> (\<lfloor>e\<rfloor>) \<Rrightarrow> []" by (simp add: maybe_static_eval_stack.Empty)
+  have "(\<V>, \<C>) \<Turnstile>\<^sub>\<rho> empty" by (simp add: may_be_static_eval_value_may_be_static_eval_env.Any)
+  have "(\<V>, \<C>) \<Turnstile>\<^sub>\<kappa> \<V> (\<lfloor>e\<rfloor>) \<Rrightarrow> []" by (simp add: may_be_static_eval_stack.Empty)
 
   from `(\<V>, \<C>) \<Turnstile>\<^sub>e e` and `(\<V>, \<C>) \<Turnstile>\<^sub>\<rho> empty` and `(\<V>, \<C>) \<Turnstile>\<^sub>\<kappa> \<V> (\<lfloor>e\<rfloor>) \<Rrightarrow> []`
-  have "(\<V>, \<C>) \<Turnstile>\<^sub>\<sigma> \<langle>e; empty; []\<rangle>" by (simp add: maybe_static_eval_state.intros)
+  have "(\<V>, \<C>) \<Turnstile>\<^sub>\<sigma> \<langle>e; empty; []\<rangle>" by (simp add: may_be_static_eval_state.intros)
 
   have "[[] \<mapsto> \<langle>e; empty; []\<rangle>] [] = Some (\<langle>e; empty; []\<rangle>)" by simp
   with `(\<V>, \<C>) \<Turnstile>\<^sub>\<sigma> \<langle>e; empty; []\<rangle>`
-  show "(\<V>, \<C>) \<Turnstile>\<^sub>\<E> [[] \<mapsto> \<langle>e; empty; []\<rangle>]" by (simp add: maybe_static_eval_pool.intros)
+  show "(\<V>, \<C>) \<Turnstile>\<^sub>\<E> [[] \<mapsto> \<langle>e; empty; []\<rangle>]" by (simp add: may_be_static_eval_pool.intros)
 qed
 
 
@@ -1531,7 +1531,7 @@ proof -
   and "\<E>' \<pi> = Some (\<langle>e'; \<rho>'; \<kappa>'\<rangle>)"
 
   from `(\<V>, \<C>) \<Turnstile>\<^sub>e e`
-  have "(\<V>, \<C>) \<Turnstile>\<^sub>\<E> [[] \<mapsto> \<langle>e; empty; []\<rangle>]" by (simp add: maybe_static_eval_to_pool)
+  have "(\<V>, \<C>) \<Turnstile>\<^sub>\<E> [[] \<mapsto> \<langle>e; empty; []\<rangle>]" by (simp add: may_be_static_eval_to_pool)
 
   from \<open>(\<V>, \<C>) \<Turnstile>\<^sub>\<E> [[] \<mapsto> \<langle>e;Map.empty;[]\<rangle>]\<close> 
   and \<open>[[] \<mapsto> \<langle>e;Map.empty;[]\<rangle>] \<rightarrow>* \<E>'\<close> 
