theory/Static_Communication_Analysis.thy
@@ -8,235 +8,120 @@ begin
 type_synonym label_map = "node_label \<Rightarrow> var set"
 
 
-inductive static_built_on_chan :: "abstract_value_env \<Rightarrow> label_map \<Rightarrow> var \<Rightarrow> var \<Rightarrow> bool"  where
+inductive 
+  may_be_built_on_abstract_chan :: "abstract_value_env \<Rightarrow> var \<Rightarrow> var \<Rightarrow> bool" and
+  may_be_built_on_abstract_chan_exp :: "abstract_value_env \<Rightarrow> var \<Rightarrow> exp \<Rightarrow> bool"
+where
   Chan: "
     \<lbrakk>
       ^Chan x\<^sub>c \<in> V x 
     \<rbrakk> \<Longrightarrow> 
-    static_built_on_chan V Ln x\<^sub>c x
+    may_be_built_on_abstract_chan V x\<^sub>c x
   " |
   Send_Evt: "
     \<lbrakk>
       ^Send_Evt x\<^sub>s\<^sub>c x\<^sub>m \<in> V x;
-      static_built_on_chan V Ln x\<^sub>c x\<^sub>s\<^sub>c \<or> static_built_on_chan V Ln x\<^sub>c x\<^sub>m 
+      may_be_built_on_abstract_chan V x\<^sub>c x\<^sub>s\<^sub>c \<or> may_be_built_on_abstract_chan V x\<^sub>c x\<^sub>m 
     \<rbrakk> \<Longrightarrow> 
-    static_built_on_chan V Ln x\<^sub>c x
+    may_be_built_on_abstract_chan V x\<^sub>c x
   " |
   Recv_Evt: "
     \<lbrakk>
       ^Recv_Evt x\<^sub>r\<^sub>c \<in> V x;
-      static_built_on_chan V Ln x\<^sub>c x\<^sub>r\<^sub>c
+      may_be_built_on_abstract_chan V x\<^sub>c x\<^sub>r\<^sub>c
     \<rbrakk> \<Longrightarrow> 
-    static_built_on_chan V Ln x\<^sub>c x
+    may_be_built_on_abstract_chan V x\<^sub>c x
   " |
   Pair: "
     \<lbrakk>
       ^(Pair x\<^sub>1 x\<^sub>2) \<in> V x;
-      static_built_on_chan V Ln x\<^sub>c x\<^sub>1 \<or> static_built_on_chan V Ln x\<^sub>c x\<^sub>2
+      may_be_built_on_abstract_chan V x\<^sub>c x\<^sub>1 \<or> may_be_built_on_abstract_chan V x\<^sub>c x\<^sub>2
     \<rbrakk> \<Longrightarrow> 
-    static_built_on_chan V Ln x\<^sub>c x
+    may_be_built_on_abstract_chan V x\<^sub>c x
   " |
   Left: "
     \<lbrakk>
       ^(Left x\<^sub>a) \<in> V x;
-      static_built_on_chan V Ln x\<^sub>c x\<^sub>a
+      may_be_built_on_abstract_chan V x\<^sub>c x\<^sub>a
     \<rbrakk> \<Longrightarrow> 
-    static_built_on_chan V Ln x\<^sub>c x
+    may_be_built_on_abstract_chan V x\<^sub>c x
   " |
   Right: "
     \<lbrakk>
       ^(Right x\<^sub>a) \<in> V x;
-      static_built_on_chan V Ln x\<^sub>c x\<^sub>a
+      may_be_built_on_abstract_chan V x\<^sub>c x\<^sub>a
     \<rbrakk> \<Longrightarrow> 
-    static_built_on_chan V Ln x\<^sub>c x
+    may_be_built_on_abstract_chan V x\<^sub>c x
   " |
   Abs: "
     ^Abs f x\<^sub>p e\<^sub>b \<in> V x \<Longrightarrow> 
-    \<not> Set.is_empty (Ln (nodeLabel e\<^sub>b)) \<Longrightarrow>
-    static_built_on_chan V Ln x\<^sub>c x
-  "
+    may_be_built_on_abstract_chan_exp V x\<^sub>c e\<^sub>b \<Longrightarrow>
+    may_be_built_on_abstract_chan V x\<^sub>c x
+  " 
 
+  |
 
-fun chanSet :: "abstract_value_env \<Rightarrow> label_map \<Rightarrow> var \<Rightarrow> var \<Rightarrow> var set" where
-  "chanSet V Ln x\<^sub>c x = (if static_built_on_chan V Ln x\<^sub>c x then {x} else {})"
-
-
-inductive static_chan_liveness :: "abstract_value_env \<Rightarrow> label_map \<Rightarrow> label_map \<Rightarrow> var \<Rightarrow> exp \<Rightarrow> bool" where
   Result: "
-    \<lbrakk>
-      chanSet V Ln x\<^sub>c y = Ln (NResult y)
-    \<rbrakk> \<Longrightarrow>
-    static_chan_liveness V Ln Lx x\<^sub>c (RESULT y)
+    may_be_built_on_abstract_chan V x\<^sub>c x \<Longrightarrow>
+    may_be_built_on_abstract_chan_exp V x\<^sub>c (RESULT x)
   " |
-  Let_Unit: "
-    \<lbrakk>
-      static_chan_liveness V Ln Lx x\<^sub>c e;
-      Ln (nodeLabel e) = Lx (NLet x);
-      Lx (NLet x) = Ln (NLet x)
-    \<rbrakk> \<Longrightarrow>
-    static_chan_liveness V Ln Lx x\<^sub>c (LET x = \<lparr>\<rparr> in e)
-  " |
-  Let_Chan: "
-    \<lbrakk>
-      static_chan_liveness V Ln Lx x\<^sub>c e;
-      Ln (nodeLabel e) = Lx (NLet x);
-      (Lx (NLet x) - {x}) = Ln (NLet x)
-    \<rbrakk> \<Longrightarrow>
-    static_chan_liveness V Ln Lx x\<^sub>c (LET x = CHAN \<lparr>\<rparr> in e)
-  " |
-  Let_Send_Evt: "
-    \<lbrakk>
-      static_chan_liveness V Ln Lx x\<^sub>c e;
-      Ln (nodeLabel e) = Lx (NLet x);
-      (Lx (NLet x) - {x}) \<union> chanSet V Ln x\<^sub>c x\<^sub>s\<^sub>c \<union> chanSet V Ln x\<^sub>c x\<^sub>m = Ln (NLet x)
-    \<rbrakk> \<Longrightarrow>
-    static_chan_liveness V Ln Lx x\<^sub>c (LET x = SEND EVT x\<^sub>s\<^sub>c x\<^sub>m in e)
-  " |
-  Let_Recv_Evt: "
-    \<lbrakk>
-      static_chan_liveness V Ln Lx x\<^sub>c e;
-      Ln (nodeLabel e) = Lx (NLet x);
-      (Lx (NLet x) - {x}) \<union> chanSet V Ln x\<^sub>c x\<^sub>r\<^sub>c = Ln (NLet x)
-    \<rbrakk> \<Longrightarrow>
-    static_chan_liveness V Ln Lx x\<^sub>c (LET x = RECV EVT x\<^sub>r\<^sub>c in e)
-  " |
-  Let_Pair: "
-    \<lbrakk>
-      static_chan_liveness V Ln Lx x\<^sub>c e;
-      Ln (nodeLabel e) = Lx (NLet x);
-      (Lx (NLet x) - {x}) \<union>  chanSet V Ln x\<^sub>c x\<^sub>1 \<union> chanSet V Ln x\<^sub>c x\<^sub>2 = Ln (NLet x)
-    \<rbrakk> \<Longrightarrow>
-    static_chan_liveness V Ln Lx x\<^sub>c (LET x = \<lparr>x\<^sub>1, x\<^sub>2\<rparr> in e)
-  " |
-  Let_Left: "
-    \<lbrakk>
-      static_chan_liveness V Ln Lx x\<^sub>c e;
-      Ln (nodeLabel e) = Lx (NLet x);
-      (Lx (NLet x) - {x}) \<union> chanSet V Ln x\<^sub>c x\<^sub>a = Ln (NLet x)
-    \<rbrakk> \<Longrightarrow>
-    static_chan_liveness V Ln Lx x\<^sub>c (LET x = LEFT x\<^sub>a in e)
-  " |
-  Let_Right: "
-    \<lbrakk>
-      static_chan_liveness V Ln Lx x\<^sub>c e;
-      Ln (nodeLabel e) = Lx (NLet x);
-      (Lx (NLet x) - {x}) \<union> chanSet V Ln x\<^sub>c x\<^sub>a = Ln (NLet x)
-    \<rbrakk> \<Longrightarrow>
-    static_chan_liveness V Ln Lx x\<^sub>c (LET x = RIGHT x\<^sub>a in e)
-  " |
-  Let_Abs: "
-    \<lbrakk>
-      static_chan_liveness V Ln Lx x\<^sub>c e;
-      Ln (nodeLabel e) = Lx (NLet x);
-      static_chan_liveness V Ln Lx x\<^sub>c e\<^sub>b;
-      (Lx (NLet x) - {x}) \<union> (Ln (nodeLabel e\<^sub>b) - {x\<^sub>p}) = Ln (NLet x)
-    \<rbrakk> \<Longrightarrow>
-    static_chan_liveness V Ln Lx x\<^sub>c (LET x = FN f x\<^sub>p . e\<^sub>b  in e)
-  " |
-  Let_Spawn: "
-    \<lbrakk>
-      static_chan_liveness V Ln Lx x\<^sub>c e;
-      static_chan_liveness V Ln Lx x\<^sub>c e\<^sub>c;
-      Ln (nodeLabel e) \<union> Ln (nodeLabel e\<^sub>c) = Lx (NLet x);
-      (Lx (NLet x) - {x}) = Ln (NLet x)
-    \<rbrakk> \<Longrightarrow>
-    static_chan_liveness V Ln Lx x\<^sub>c (LET x = SPAWN e\<^sub>c in e)
-  " |
-  Let_Sync: "
-    \<lbrakk>
-      static_chan_liveness V Ln Lx x\<^sub>c e;
-      Ln (nodeLabel e) = Lx (NLet x);
-      (Lx (NLet x) - {x}) \<union> chanSet V Ln x\<^sub>c x\<^sub>e = Ln (NLet x)
-    \<rbrakk> \<Longrightarrow>
-    static_chan_liveness V Ln Lx x\<^sub>c (LET x = SYNC x\<^sub>e in e)
-  " |
-  Let_Fst: "
-    \<lbrakk>
-      static_chan_liveness V Ln Lx x\<^sub>c e;
-      Ln (nodeLabel e) = Lx (NLet x);
-      (Lx (NLet x) - {x}) \<union> chanSet V Ln x\<^sub>c x\<^sub>a = Ln (NLet x)
-    \<rbrakk> \<Longrightarrow>
-    static_chan_liveness V Ln Lx x\<^sub>c (LET x = FST x\<^sub>a in e)
-  " |
-  Let_Snd: "
-    \<lbrakk>
-      static_chan_liveness V Ln Lx x\<^sub>c e;
-      Ln (nodeLabel e) = Lx (NLet x);
-      (Lx (NLet x) - {x}) \<union> chanSet V Ln x\<^sub>c x\<^sub>a = Ln (NLet x)
-    \<rbrakk> \<Longrightarrow>
-    static_chan_liveness V Ln Lx x\<^sub>c (LET x = SND x\<^sub>a in e)
-  " |
-  Let_Case: "
-    \<lbrakk>
-      static_chan_liveness V Ln Lx x\<^sub>c e;
-      Ln (nodeLabel e) = Lx (NLet x);
-      static_chan_liveness V Ln Lx x\<^sub>c e\<^sub>l;
-      static_chan_liveness V Ln Lx x\<^sub>c e\<^sub>r;
-      (Lx (NLet x) - {x}) \<union> chanSet V Ln x\<^sub>c x\<^sub>s \<union> 
-         (Ln (nodeLabel e\<^sub>l) - {x\<^sub>l}) \<union> (Ln (nodeLabel e\<^sub>r) - {x\<^sub>r}) = Ln (NLet x)
-    \<rbrakk> \<Longrightarrow>
-    static_chan_liveness V Ln Lx x\<^sub>c (LET x = CASE x\<^sub>s LEFT x\<^sub>l |> e\<^sub>l RIGHT x\<^sub>r |> e\<^sub>r in e)
-  " |
-  Let_App: "
-    \<lbrakk>
-      static_chan_liveness V Ln Lx x\<^sub>c e;
-      Ln (nodeLabel e) = Lx (NLet x);
-      (Lx (NLet x) - {x}) \<union> chanSet V Ln x\<^sub>c f \<union> chanSet V Ln x\<^sub>c x\<^sub>a = Ln (NLet x)
-    \<rbrakk> \<Longrightarrow>
-    static_chan_liveness V Ln Lx x\<^sub>c (LET x = APP f x\<^sub>a in e)
+  Let: "
+    may_be_built_on_abstract_chan V x\<^sub>c x \<or> 
+    may_be_built_on_abstract_chan_exp V x\<^sub>c e \<Longrightarrow>
+    may_be_built_on_abstract_chan_exp V x\<^sub>c (LET x = b in e)
   "
 
-inductive maybe_static_send_node_label :: "abstract_value_env \<Rightarrow> exp \<Rightarrow> var \<Rightarrow> node_label \<Rightarrow> bool" where
+inductive may_be_static_send_node_label :: "abstract_value_env \<Rightarrow> exp \<Rightarrow> var \<Rightarrow> node_label \<Rightarrow> bool" where
   Sync: "
     {^Chan xC} \<subseteq> V xSC \<Longrightarrow>
     {^Send_Evt xSC xM} \<subseteq> V xE \<Longrightarrow>
     is_super_exp e (LET x = SYNC xE in e') \<Longrightarrow>
-    maybe_static_send_node_label V e xC (NLet x)
+    may_be_static_send_node_label V e xC (NLet x)
   "
 
-inductive maybe_static_recv_node_label :: "abstract_value_env \<Rightarrow> exp \<Rightarrow> var \<Rightarrow> node_label \<Rightarrow> bool" where
+inductive may_be_static_recv_node_label :: "abstract_value_env \<Rightarrow> exp \<Rightarrow> var \<Rightarrow> node_label \<Rightarrow> bool" where
   Sync: "
     {^Chan xC} \<subseteq> V xRC \<Longrightarrow>
     {^Recv_Evt xRC} \<subseteq> V xE \<Longrightarrow>
     is_super_exp e (LET x = SYNC xE in e') \<Longrightarrow>
-    maybe_static_recv_node_label V e xC (NLet x)
+    may_be_static_recv_node_label V e xC (NLet x)
   "
 
 
-inductive maybe_static_path :: "abstract_value_env \<Rightarrow> flow_set \<Rightarrow> label_map \<Rightarrow> var \<Rightarrow> node_label \<Rightarrow> (node_label \<Rightarrow> bool) \<Rightarrow> static_path \<Rightarrow> bool" where
+inductive may_be_static_path :: "abstract_value_env \<Rightarrow> flow_set \<Rightarrow> label_map \<Rightarrow> var \<Rightarrow> node_label \<Rightarrow> (node_label \<Rightarrow> bool) \<Rightarrow> static_path \<Rightarrow> bool" where
   Empty: "
     isEnd start \<Longrightarrow>
-    maybe_static_path V F Ln xC start isEnd []
+    may_be_static_path V F Ln xC start isEnd []
   " |
   Edge: "
     isEnd end \<Longrightarrow>
     (start, edge, end) \<in> F \<Longrightarrow>
-    maybe_static_path V F Ln xC start isEnd [(start, el)]
+    may_be_static_path V F Ln xC start isEnd [(start, el)]
   " |
   Step_Next: "
-    maybe_static_path V F Ln xC middle isEnd ((middle, edge') # path) \<Longrightarrow>
+    may_be_static_path V F Ln xC middle isEnd ((middle, edge') # path) \<Longrightarrow>
     (start, ENext, middle) \<in> F \<Longrightarrow>
-    maybe_static_path V F Ln xC start isEnd ((start, edge) # (middle, edge') # path)
+    may_be_static_path V F Ln xC start isEnd ((start, edge) # (middle, edge') # path)
   " |
   Step_Call: "
-    maybe_static_path V F Ln xC middle isEnd ((middle, edge') # path) \<Longrightarrow>
+    may_be_static_path V F Ln xC middle isEnd ((middle, edge') # path) \<Longrightarrow>
     (start, ECall, middle) \<in> F \<Longrightarrow>
-    maybe_static_path V F Ln xC start isEnd ((start, edge) # (middle, edge') # path)
+    may_be_static_path V F Ln xC start isEnd ((start, edge) # (middle, edge') # path)
   " |
   Step_Return: "
-    maybe_static_path V F Ln xC middle isEnd ((middle, edge') # path) \<Longrightarrow>
+    may_be_static_path V F Ln xC middle isEnd ((middle, edge') # path) \<Longrightarrow>
     (start, EReturn, middle) \<in> F \<Longrightarrow>
-    maybe_static_path V F Ln xC start isEnd ((start, edge) # (middle, edge') # path)
+    may_be_static_path V F Ln xC start isEnd ((start, edge) # (middle, edge') # path)
   " |
   Step_Send: "
-    maybe_static_path V F Ln xC middle isEnd ((middle, edge') # path) \<Longrightarrow>
-    static_built_on_chan V Ln xC xM \<Longrightarrow>
+    may_be_static_path V F Ln xC middle isEnd ((middle, edge') # path) \<Longrightarrow>
+    may_be_built_on_abstract_chan V xC xM \<Longrightarrow>
     (start, ESend xM, middle) \<in> F \<Longrightarrow>
-    maybe_static_path V F Ln xC start isEnd ((start, edge) # (middle, edge') # path)
+    may_be_static_path V F Ln xC start isEnd ((start, edge) # (middle, edge') # path)
   "
 
 
-inductive maybe_inclusive :: "static_path \<Rightarrow> static_path \<Rightarrow> bool" (infix "\<asymp>" 55) where
+inductive may_be_inclusive :: "static_path \<Rightarrow> static_path \<Rightarrow> bool" (infix "\<asymp>" 55) where
   Ordered: "
     prefix \<pi>\<^sub>1 \<pi>\<^sub>2 \<or> prefix \<pi>\<^sub>2 \<pi>\<^sub>1 \<Longrightarrow>
     \<pi>\<^sub>1 \<asymp> \<pi>\<^sub>2
@@ -254,10 +139,10 @@ inductive maybe_inclusive :: "static_path \<Rightarrow> static_path \<Rightarrow
     \<pi> @ (NLet x, ENext) # \<pi>\<^sub>1 \<asymp> \<pi> @ (NLet x, ESend xM) # \<pi>\<^sub>2
   "
 
-lemma maybe_inclusive_commut: "
+lemma may_be_inclusive_commut: "
   \<pi>\<^sub>1 \<asymp> \<pi>\<^sub>2 \<Longrightarrow> \<pi>\<^sub>2 \<asymp> \<pi>\<^sub>1
 "
- apply (erule maybe_inclusive.cases; auto)
+ apply (erule may_be_inclusive.cases; auto)
   apply (simp add: Ordered)
   apply (simp add: Ordered)
   apply (simp add: Spawn_Right)
@@ -267,10 +152,10 @@ lemma maybe_inclusive_commut: "
 done
 
 
-lemma maybe_inclusive_preserved_under_unordered_extension: "
+lemma may_be_inclusive_preserved_under_unordered_extension: "
   \<not> prefix \<pi>\<^sub>1 \<pi>\<^sub>2 \<Longrightarrow> \<not> prefix \<pi>\<^sub>2 \<pi>\<^sub>1 \<Longrightarrow> \<pi>\<^sub>1 \<asymp> \<pi>\<^sub>2 \<Longrightarrow> \<pi>\<^sub>1 @ [l] \<asymp> \<pi>\<^sub>2
 "
- apply (erule maybe_inclusive.cases; auto)
+ apply (erule may_be_inclusive.cases; auto)
   apply (simp add: Spawn_Left)
   apply (simp add: Spawn_Right)
   apply (simp add: Send_Left)
@@ -312,33 +197,29 @@ inductive every_two_static_paths  :: "(static_path \<Rightarrow> bool) \<Rightar
 
 inductive static_one_shot :: "abstract_value_env \<Rightarrow> exp \<Rightarrow> var \<Rightarrow> bool" where
   Sync: "
-    every_two_static_paths (maybe_static_path V F Ln xC (NLet xC) (maybe_static_send_node_label V e xC)) singular \<Longrightarrow>
-    static_chan_liveness V Ln Lx xC e \<Longrightarrow>
+    every_two_static_paths (may_be_static_path V F Ln xC (NLet xC) (may_be_static_send_node_label V e xC)) singular \<Longrightarrow>
     static_flow_set V F e \<Longrightarrow>
     static_one_shot V e xC 
   "
 
 inductive static_one_to_one :: "abstract_value_env \<Rightarrow> exp \<Rightarrow> var \<Rightarrow> bool" where
   Sync: "
-    every_two_static_paths (maybe_static_path V F Ln xC (NLet xC) (maybe_static_send_node_label V e xC)) noncompetitive \<Longrightarrow>
-    every_two_static_paths (maybe_static_path V F Ln xC (NLet xC) (maybe_static_recv_node_label V e xC)) noncompetitive \<Longrightarrow>
-    static_chan_liveness V Ln Lx xC e \<Longrightarrow>
+    every_two_static_paths (may_be_static_path V F Ln xC (NLet xC) (may_be_static_send_node_label V e xC)) noncompetitive \<Longrightarrow>
+    every_two_static_paths (may_be_static_path V F Ln xC (NLet xC) (may_be_static_recv_node_label V e xC)) noncompetitive \<Longrightarrow>
     static_flow_set V F e \<Longrightarrow>
     static_one_to_one V e xC 
   "
 
 inductive static_fan_out :: "abstract_value_env \<Rightarrow> exp \<Rightarrow> var \<Rightarrow> bool" where
   Sync: "
-    every_two_static_paths (maybe_static_path V F Ln xC (NLet xC) (maybe_static_send_node_label V e xC)) noncompetitive \<Longrightarrow>
-    static_chan_liveness V Ln Lx xC e \<Longrightarrow>
+    every_two_static_paths (may_be_static_path V F Ln xC (NLet xC) (may_be_static_send_node_label V e xC)) noncompetitive \<Longrightarrow>
     static_flow_set V F e \<Longrightarrow>
     static_fan_out V e xC 
   "
 
 inductive static_fan_in :: "abstract_value_env \<Rightarrow> exp \<Rightarrow> var \<Rightarrow> bool" where
   Sync: "
-    every_two_static_paths (maybe_static_path V F Ln xC (NLet xC) (maybe_static_recv_node_label V e xC)) noncompetitive \<Longrightarrow>
-    static_chan_liveness V Ln Lx xC e \<Longrightarrow>
+    every_two_static_paths (may_be_static_path V F Ln xC (NLet xC) (may_be_static_recv_node_label V e xC)) noncompetitive \<Longrightarrow>
     static_flow_set V F e \<Longrightarrow>
     static_fan_in V e xC 
   "
